@prefix dc11: <http://purl.org/dc/elements/1.1/> .
@prefix xsd: <http://www.w3.org/2001/XMLSchema#> .
@prefix rdfs: <http://www.w3.org/2000/01/rdf-schema#> .
@prefix rdf: <http://www.w3.org/1999/02/22-rdf-syntax-ns#> .

<https://edi3.org/mmt/vocab#>
  dc11:creator "EDI3"^^xsd:string ;
  dc11:date "2020-06-09"^^xsd:string ;
  dc11:description "MMT Vocabulary"^^xsd:string ;
  dc11:identifier "https://edi3.org/mmt/vocab#"^^xsd:string ;
  dc11:publisher "EDI3"^^xsd:string ;
  dc11:title "MMT Vocabulary"^^xsd:string ;
  rdfs:comment "MMT Vocabulary"^^xsd:string .

<https://edi3.org/mmt/vocab#AcademicQualification>
  a rdfs:Class ;
  rdfs:comment "An academic achievement that is officially recognized."^^xsd:string ;
  rdfs:label "AcademicQualification"^^xsd:string .

<https://edi3.org/mmt/vocab#AcademicQualificationAbbreviatedName>
  a rdf:Property ;
  rdfs:comment "The abbreviated name, expressed as text, of this academic qualification."^^xsd:string ;
  rdfs:domain "mmt:AcademicQualification"^^xsd:string ;
  rdfs:label "abbreviatedName"^^xsd:string ;
  rdfs:range "xsd:string"^^xsd:string .

<https://edi3.org/mmt/vocab#AcademicQualificationName>
  a rdf:Property ;
  rdfs:comment "A name, expressed as text, of this academic qualification."^^xsd:string ;
  rdfs:domain "mmt:AcademicQualification"^^xsd:string ;
  rdfs:label "name"^^xsd:string ;
  rdfs:range "xsd:string"^^xsd:string .

<https://edi3.org/mmt/vocab#AppliedChemicalTreatment>
  a rdfs:Class ;
  rdfs:comment "A process of applying a chemical, physical, or biological agent to an object."^^xsd:string ;
  rdfs:label "AppliedChemicalTreatment"^^xsd:string .

<https://edi3.org/mmt/vocab#AppliedChemicalTreatmentChemicalConcentrationMeasure>
  a rdf:Property ;
  rdfs:comment "A measure of the chemical concentration of this applied chemical treatment."^^xsd:string ;
  rdfs:domain "mmt:AppliedChemicalTreatment"^^xsd:string ;
  rdfs:label "chemicalConcentrationMeasure"^^xsd:string ;
  rdfs:range "xsd:decimal"^^xsd:string .

<https://edi3.org/mmt/vocab#AppliedChemicalTreatmentMethodName>
  a rdf:Property ;
  rdfs:comment "The name, expressed as text, of the method of this applied chemical treatment."^^xsd:string ;
  rdfs:domain "mmt:AppliedChemicalTreatment"^^xsd:string ;
  rdfs:label "methodName"^^xsd:string ;
  rdfs:range "xsd:string"^^xsd:string .

<https://edi3.org/mmt/vocab#AppliedChemicalTreatmentName>
  a rdf:Property ;
  rdfs:comment "A name, expressed as text, of this applied chemical treatment."^^xsd:string ;
  rdfs:domain "mmt:AppliedChemicalTreatment"^^xsd:string ;
  rdfs:label "name"^^xsd:string ;
  rdfs:range "xsd:string"^^xsd:string .

<https://edi3.org/mmt/vocab#AppliedChemicalTreatmentOccurrenceDateTime>
  a rdf:Property ;
  rdfs:comment "The date time of the occurrence of this applied chemical treatment."^^xsd:string ;
  rdfs:domain "mmt:AppliedChemicalTreatment"^^xsd:string ;
  rdfs:label "occurrenceDateTime"^^xsd:string ;
  rdfs:range "xsd:datetime"^^xsd:string .

<https://edi3.org/mmt/vocab#AssociatedTransportEquipment>
  a rdfs:Class ;
  rdfs:comment "A piece of transport equipment that is associated with another piece of transport equipment, such as a maritime container placed on a rail wagon for transportation."^^xsd:string ;
  rdfs:label "AssociatedTransportEquipment"^^xsd:string .

<https://edi3.org/mmt/vocab#AssociatedTransportEquipmentCharacteristicText>
  a rdf:Property ;
  rdfs:comment "The textual description of the characteristics, i.e. size and type, of this piece of associated transport equipment."^^xsd:string ;
  rdfs:domain "mmt:AssociatedTransportEquipment"^^xsd:string ;
  rdfs:label "characteristicText"^^xsd:string ;
  rdfs:range "xsd:string"^^xsd:string .

<https://edi3.org/mmt/vocab#AssociatedTransportEquipmentID>
  a rdf:Property ;
  rdfs:comment "A unique number, mark or name which identifies this associated piece of transport equipment."^^xsd:string ;
  rdfs:domain "mmt:AssociatedTransportEquipment"^^xsd:string ;
  rdfs:label "iD"^^xsd:string ;
  rdfs:range "xsd:ID"^^xsd:string .

<https://edi3.org/mmt/vocab#AttachedTransportEquipment>
  a rdfs:Class ;
  rdfs:comment "A piece of attached transport equipment, such as a chain or a tarpaulin."^^xsd:string ;
  rdfs:label "AttachedTransportEquipment"^^xsd:string .

<https://edi3.org/mmt/vocab#AttachedTransportEquipmentCharacteristicText>
  a rdf:Property ;
  rdfs:comment "The textual description of the characteristics, i.e. size and type, of this piece of attached transport equipment."^^xsd:string ;
  rdfs:domain "mmt:AttachedTransportEquipment"^^xsd:string ;
  rdfs:label "characteristicText"^^xsd:string ;
  rdfs:range "xsd:string"^^xsd:string .

<https://edi3.org/mmt/vocab#AttachedTransportEquipmentID>
  a rdf:Property ;
  rdfs:comment "A unique identifier of this piece of attached transport equipment."^^xsd:string ;
  rdfs:domain "mmt:AttachedTransportEquipment"^^xsd:string ;
  rdfs:label "iD"^^xsd:string ;
  rdfs:range "xsd:ID"^^xsd:string .

<https://edi3.org/mmt/vocab#AttachedTransportEquipmentUnitQuantity>
  a rdf:Property ;
  rdfs:comment "The number of units of attached transport equipment."^^xsd:string ;
  rdfs:domain "mmt:AttachedTransportEquipment"^^xsd:string ;
  rdfs:label "unitQuantity"^^xsd:string ;
  rdfs:range "xsd:decimal"^^xsd:string .

<https://edi3.org/mmt/vocab#AuthoritativeSignatoryPerson>
  a rdfs:Class ;
  rdfs:comment "A person who is authorized to sign a document, such as a customs officer or other government official."^^xsd:string ;
  rdfs:label "AuthoritativeSignatoryPerson"^^xsd:string .

<https://edi3.org/mmt/vocab#AuthoritativeSignatoryPersonName>
  a rdf:Property ;
  rdfs:comment "The name, expressed as text, of this authoritative signatory person."^^xsd:string ;
  rdfs:domain "mmt:AuthoritativeSignatoryPerson"^^xsd:string ;
  rdfs:label "name"^^xsd:string ;
  rdfs:range "xsd:string"^^xsd:string .

<https://edi3.org/mmt/vocab#CalculatedEmission>
  a rdfs:Class ;
  rdfs:comment "A calculation of the pollution (including noise, heat, and radiation etc.) discharged into the environment by a residential, commercial, or industrial facility or by a means of transport, such as a vessel, aircraft or truck."^^xsd:string ;
  rdfs:label "CalculatedEmission"^^xsd:string .

<https://edi3.org/mmt/vocab#CalculatedEmissionAffectedDistanceMeasure>
  a rdf:Property ;
  rdfs:comment "The affected distance over which this calculated emission is measured."^^xsd:string ;
  rdfs:domain "mmt:CalculatedEmission"^^xsd:string ;
  rdfs:label "affectedDistanceMeasure"^^xsd:string ;
  rdfs:range "xsd:decimal"^^xsd:string .

<https://edi3.org/mmt/vocab#CalculatedEmissionPollutionMeasure>
  a rdf:Property ;
  rdfs:comment "A measure of the pollution calculated for this emission."^^xsd:string ;
  rdfs:domain "mmt:CalculatedEmission"^^xsd:string ;
  rdfs:label "pollutionMeasure"^^xsd:string ;
  rdfs:range "xsd:decimal"^^xsd:string .

<https://edi3.org/mmt/vocab#CalculatedEmissionTypeCode>
  a rdf:Property ;
  rdfs:comment "The code specifying the type of this calculated emission."^^xsd:string ;
  rdfs:domain "mmt:CalculatedEmission"^^xsd:string ;
  rdfs:label "typeCode"^^xsd:string ;
  rdfs:range "xsd:token"^^xsd:string .

<https://edi3.org/mmt/vocab#CalculatedEmissionWeight>
  a rdf:Property ;
  rdfs:comment "A weight for which this calculated emission is measured."^^xsd:string ;
  rdfs:domain "mmt:CalculatedEmission"^^xsd:string ;
  rdfs:label "weight"^^xsd:string ;
  rdfs:range "xsd:decimal"^^xsd:string .

<https://edi3.org/mmt/vocab#CertificationTestSpecificationReport>
  a rdfs:Class ;
  rdfs:comment "A report that specifies a certification test and its attributes."^^xsd:string ;
  rdfs:label "CertificationTestSpecificationReport"^^xsd:string .

<https://edi3.org/mmt/vocab#CertificationTestSpecificationReportResultText>
  a rdf:Property ;
  rdfs:comment "A result, expressed as text, reported in this certification test specification report."^^xsd:string ;
  rdfs:domain "mmt:CertificationTestSpecificationReport"^^xsd:string ;
  rdfs:label "resultText"^^xsd:string ;
  rdfs:range "xsd:string"^^xsd:string .

<https://edi3.org/mmt/vocab#CertificationTestSpecificationReportStandardName>
  a rdf:Property ;
  rdfs:comment "The name, expressed as text, of the standard applicable for this certification test specification report."^^xsd:string ;
  rdfs:domain "mmt:CertificationTestSpecificationReport"^^xsd:string ;
  rdfs:label "standardName"^^xsd:string ;
  rdfs:range "xsd:string"^^xsd:string .

<https://edi3.org/mmt/vocab#CertificationTestSpecificationReportTestName>
  a rdf:Property ;
  rdfs:comment "A test name, expressed as text, for this certification test specification report."^^xsd:string ;
  rdfs:domain "mmt:CertificationTestSpecificationReport"^^xsd:string ;
  rdfs:label "testName"^^xsd:string ;
  rdfs:range "xsd:string"^^xsd:string .

<https://edi3.org/mmt/vocab#CertifiedAccreditation>
  a rdfs:Class ;
  rdfs:comment "A certified recognition that provides evidence of a level of competency in a given area, such as certifying a level of skill in a trade."^^xsd:string ;
  rdfs:label "CertifiedAccreditation"^^xsd:string .

<https://edi3.org/mmt/vocab#CertifiedAccreditationAccreditingBodyName>
  a rdf:Property ;
  rdfs:comment "The name of the accrediting body, expressed as text, for this certified accreditation."^^xsd:string ;
  rdfs:domain "mmt:CertifiedAccreditation"^^xsd:string ;
  rdfs:label "accreditingBodyName"^^xsd:string ;
  rdfs:range "xsd:string"^^xsd:string .

<https://edi3.org/mmt/vocab#CertifiedAccreditationAuthenticationMethodCode>
  a rdf:Property ;
  rdfs:comment "A code specifying an authentication method for this certified accreditation."^^xsd:string ;
  rdfs:domain "mmt:CertifiedAccreditation"^^xsd:string ;
  rdfs:label "authenticationMethodCode"^^xsd:string ;
  rdfs:range "xsd:token"^^xsd:string .

<https://edi3.org/mmt/vocab#CertifiedAccreditationCategoryCode>
  a rdf:Property ;
  rdfs:comment "The code specifying the category of this certified accreditation, such as driving or academic."^^xsd:string ;
  rdfs:domain "mmt:CertifiedAccreditation"^^xsd:string ;
  rdfs:label "categoryCode"^^xsd:string ;
  rdfs:range "xsd:token"^^xsd:string .

<https://edi3.org/mmt/vocab#CertifiedAccreditationDescription>
  a rdf:Property ;
  rdfs:comment "The textual description of this certified accreditation."^^xsd:string ;
  rdfs:domain "mmt:CertifiedAccreditation"^^xsd:string ;
  rdfs:label "description"^^xsd:string ;
  rdfs:range "xsd:string"^^xsd:string .

<https://edi3.org/mmt/vocab#CertifiedAccreditationExpiryDateTime>
  a rdf:Property ;
  rdfs:comment "The date, time, date time or other date time value when this certified accreditation expires."^^xsd:string ;
  rdfs:domain "mmt:CertifiedAccreditation"^^xsd:string ;
  rdfs:label "expiryDateTime"^^xsd:string ;
  rdfs:range "xsd:datetime"^^xsd:string .

<https://edi3.org/mmt/vocab#CertifiedAccreditationID>
  a rdf:Property ;
  rdfs:comment "An identifier for this certified accreditation."^^xsd:string ;
  rdfs:domain "mmt:CertifiedAccreditation"^^xsd:string ;
  rdfs:label "iD"^^xsd:string ;
  rdfs:range "xsd:ID"^^xsd:string .

<https://edi3.org/mmt/vocab#CertifiedAccreditationObtainedDateTime>
  a rdf:Property ;
  rdfs:comment "The date, time, date time or other date time value when this certified accreditation was obtained."^^xsd:string ;
  rdfs:domain "mmt:CertifiedAccreditation"^^xsd:string ;
  rdfs:label "obtainedDateTime"^^xsd:string ;
  rdfs:range "xsd:datetime"^^xsd:string .

<https://edi3.org/mmt/vocab#CertifiedAccreditationTypeCode>
  a rdf:Property ;
  rdfs:comment "The code specifying the type of this certified accreditation, such as a type of driving license."^^xsd:string ;
  rdfs:domain "mmt:CertifiedAccreditation"^^xsd:string ;
  rdfs:label "typeCode"^^xsd:string ;
  rdfs:range "xsd:token"^^xsd:string .

<https://edi3.org/mmt/vocab#CrossBorderCustomsValuation>
  a rdfs:Class ;
  rdfs:comment "A cross-border trade related assessment of the worth of an object, such as its monetary value, for customs purposes."^^xsd:string ;
  rdfs:label "CrossBorderCustomsValuation"^^xsd:string .

<https://edi3.org/mmt/vocab#CrossBorderCustomsValuationAddedAdjustmentAmount>
  a rdf:Property ;
  rdfs:comment "The monetary value of the adjustment added for this cross-border customs valuation."^^xsd:string ;
  rdfs:domain "mmt:CrossBorderCustomsValuation"^^xsd:string ;
  rdfs:label "addedAdjustmentAmount"^^xsd:string ;
  rdfs:range "http://schema.org/amount"^^xsd:string .

<https://edi3.org/mmt/vocab#CrossBorderCustomsValuationAddedAdjustmentPercent>
  a rdf:Property ;
  rdfs:comment "The adjustment added, expressed as a percentage, for this cross-border customs valuation."^^xsd:string ;
  rdfs:domain "mmt:CrossBorderCustomsValuation"^^xsd:string ;
  rdfs:label "addedAdjustmentPercent"^^xsd:string ;
  rdfs:range "xsd:decimal"^^xsd:string .

<https://edi3.org/mmt/vocab#CrossBorderCustomsValuationBuyerSellerRelationshipIndicator>
  a rdf:Property ;
  rdfs:comment "The indication of whether or not there is a relationship between the buyer and the seller, such as a financial relationship, for this cross-border customs valuation."^^xsd:string ;
  rdfs:domain "mmt:CrossBorderCustomsValuation"^^xsd:string ;
  rdfs:label "buyerSellerRelationshipIndicator"^^xsd:string ;
  rdfs:range "xsd:boolean"^^xsd:string .

<https://edi3.org/mmt/vocab#CrossBorderCustomsValuationBuyerSellerRelationshipPriceInfluenceIndicator>
  a rdf:Property ;
  rdfs:comment "The indication of whether or not the buyer seller relationship influences the price of the goods for this cross-border customs valuation."^^xsd:string ;
  rdfs:domain "mmt:CrossBorderCustomsValuation"^^xsd:string ;
  rdfs:label "buyerSellerRelationshipPriceInfluenceIndicator"^^xsd:string ;
  rdfs:range "xsd:boolean"^^xsd:string .

<https://edi3.org/mmt/vocab#CrossBorderCustomsValuationChargeApportionMethodCode>
  a rdf:Property ;
  rdfs:comment "The code specifying the method of the apportion of charges for this cross-border customs valuation."^^xsd:string ;
  rdfs:domain "mmt:CrossBorderCustomsValuation"^^xsd:string ;
  rdfs:label "chargeApportionMethodCode"^^xsd:string ;
  rdfs:range "xsd:token"^^xsd:string .

<https://edi3.org/mmt/vocab#CrossBorderCustomsValuationDeductedAdjustmentAmount>
  a rdf:Property ;
  rdfs:comment "The monetary value of the adjustment deducted for this cross-border customs valuation."^^xsd:string ;
  rdfs:domain "mmt:CrossBorderCustomsValuation"^^xsd:string ;
  rdfs:label "deductedAdjustmentAmount"^^xsd:string ;
  rdfs:range "http://schema.org/amount"^^xsd:string .

<https://edi3.org/mmt/vocab#CrossBorderCustomsValuationDeductedAdjustmentPercent>
  a rdf:Property ;
  rdfs:comment "The adjustment deducted, expressed as a percentage, for this cross-border customs valuation."^^xsd:string ;
  rdfs:domain "mmt:CrossBorderCustomsValuation"^^xsd:string ;
  rdfs:label "deductedAdjustmentPercent"^^xsd:string ;
  rdfs:range "xsd:decimal"^^xsd:string .

<https://edi3.org/mmt/vocab#CrossBorderCustomsValuationMethodCode>
  a rdf:Property ;
  rdfs:comment "The code specifying the method by which this cross-border customs valuation is determined."^^xsd:string ;
  rdfs:domain "mmt:CrossBorderCustomsValuation"^^xsd:string ;
  rdfs:label "methodCode"^^xsd:string ;
  rdfs:range "xsd:token"^^xsd:string .

<https://edi3.org/mmt/vocab#CrossBorderCustomsValuationOtherChargeAmount>
  a rdf:Property ;
  rdfs:comment "A monetary value added or subtracted from the total invoice price not previously taken into account for this cross-border customs valuation."^^xsd:string ;
  rdfs:domain "mmt:CrossBorderCustomsValuation"^^xsd:string ;
  rdfs:label "otherChargeAmount"^^xsd:string ;
  rdfs:range "http://schema.org/amount"^^xsd:string .

<https://edi3.org/mmt/vocab#CrossBorderCustomsValuationRoyaltyLicenceFeeIndicator>
  a rdf:Property ;
  rdfs:comment "The indication of whether or not there is a royalty or licence fee related to the goods for this cross-border customs valuation."^^xsd:string ;
  rdfs:domain "mmt:CrossBorderCustomsValuation"^^xsd:string ;
  rdfs:label "royaltyLicenceFeeIndicator"^^xsd:string ;
  rdfs:range "xsd:boolean"^^xsd:string .

<https://edi3.org/mmt/vocab#CrossBorderCustomsValuationSalePriceConditionIndicator>
  a rdf:Property ;
  rdfs:comment "The indication of whether or not there is a condition imposed on the sale price of the goods for this cross-border customs valuation."^^xsd:string ;
  rdfs:domain "mmt:CrossBorderCustomsValuation"^^xsd:string ;
  rdfs:label "salePriceConditionIndicator"^^xsd:string ;
  rdfs:range "xsd:boolean"^^xsd:string .

<https://edi3.org/mmt/vocab#CrossBorderCustomsValuationSaleRestrictionIndicator>
  a rdf:Property ;
  rdfs:comment "The indication of whether or not there is any restriction imposed on the sale of the goods for this cross-border customs valuation."^^xsd:string ;
  rdfs:domain "mmt:CrossBorderCustomsValuation"^^xsd:string ;
  rdfs:label "saleRestrictionIndicator"^^xsd:string ;
  rdfs:range "xsd:boolean"^^xsd:string .

<https://edi3.org/mmt/vocab#CrossBorderCustomsValuationTypeCode>
  a rdf:Property ;
  rdfs:comment "The code specifying the type of cross-border customs valuation."^^xsd:string ;
  rdfs:domain "mmt:CrossBorderCustomsValuation"^^xsd:string ;
  rdfs:label "typeCode"^^xsd:string ;
  rdfs:range "xsd:token"^^xsd:string .

<https://edi3.org/mmt/vocab#CrossBorderCustomsValuationWTOAdditionCode>
  a rdf:Property ;
  rdfs:comment "The code specifying any additions necessary under the World Trade Organization (WTO) Valuation Agreement used for the assessment of this cross-border customs valuation."^^xsd:string ;
  rdfs:domain "mmt:CrossBorderCustomsValuation"^^xsd:string ;
  rdfs:label "wTOAdditionCode"^^xsd:string ;
  rdfs:range "xsd:token"^^xsd:string .

<https://edi3.org/mmt/vocab#CrossBorderRegulatoryProcedure>
  a rdfs:Class ;
  rdfs:comment "A set of formal steps to satisfy a cross-border regulation, law or convention."^^xsd:string ;
  rdfs:label "CrossBorderRegulatoryProcedure"^^xsd:string .

<https://edi3.org/mmt/vocab#CrossBorderRegulatoryProcedureAcquisitionDateTime>
  a rdf:Property ;
  rdfs:comment "The date, time, date time, or other date time value of an acquisition for this cross-border regulatory procedure."^^xsd:string ;
  rdfs:domain "mmt:CrossBorderRegulatoryProcedure"^^xsd:string ;
  rdfs:label "acquisitionDateTime"^^xsd:string ;
  rdfs:range "xsd:datetime"^^xsd:string .

<https://edi3.org/mmt/vocab#CrossBorderRegulatoryProcedureAmendmentReasonCode>
  a rdf:Property ;
  rdfs:comment "A code specifying a reason for an amendment to this cross-border regulatory procedure."^^xsd:string ;
  rdfs:domain "mmt:CrossBorderRegulatoryProcedure"^^xsd:string ;
  rdfs:label "amendmentReasonCode"^^xsd:string ;
  rdfs:range "xsd:token"^^xsd:string .

<https://edi3.org/mmt/vocab#CrossBorderRegulatoryProcedureAnnualQuotaQuantity>
  a rdf:Property ;
  rdfs:comment "The annual quota quantity under this cross-border regulatory procedure."^^xsd:string ;
  rdfs:domain "mmt:CrossBorderRegulatoryProcedure"^^xsd:string ;
  rdfs:label "annualQuotaQuantity"^^xsd:string ;
  rdfs:range "xsd:decimal"^^xsd:string .

<https://edi3.org/mmt/vocab#CrossBorderRegulatoryProcedureCategoryCode>
  a rdf:Property ;
  rdfs:comment "A code specifying a category for this cross-border regulatory procedure, such as the appendices of the CITES Convention."^^xsd:string ;
  rdfs:domain "mmt:CrossBorderRegulatoryProcedure"^^xsd:string ;
  rdfs:label "categoryCode"^^xsd:string ;
  rdfs:range "xsd:token"^^xsd:string .

<https://edi3.org/mmt/vocab#CrossBorderRegulatoryProcedureCertificationBasisText>
  a rdf:Property ;
  rdfs:comment "A basis for a certification, expressed as text, for this cross-border regulatory procedure."^^xsd:string ;
  rdfs:domain "mmt:CrossBorderRegulatoryProcedure"^^xsd:string ;
  rdfs:label "certificationBasisText"^^xsd:string ;
  rdfs:range "xsd:string"^^xsd:string .

<https://edi3.org/mmt/vocab#CrossBorderRegulatoryProcedureControlRequirementIndicator>
  a rdf:Property ;
  rdfs:comment "The indication of whether or not a control is required for this cross-border regulatory procedure."^^xsd:string ;
  rdfs:domain "mmt:CrossBorderRegulatoryProcedure"^^xsd:string ;
  rdfs:label "controlRequirementIndicator"^^xsd:string ;
  rdfs:range "xsd:boolean"^^xsd:string .

<https://edi3.org/mmt/vocab#CrossBorderRegulatoryProcedureControlResultText>
  a rdf:Property ;
  rdfs:comment "A control result, expressed as text, for this cross-border regulatory procedure."^^xsd:string ;
  rdfs:domain "mmt:CrossBorderRegulatoryProcedure"^^xsd:string ;
  rdfs:label "controlResultText"^^xsd:string ;
  rdfs:range "xsd:string"^^xsd:string .

<https://edi3.org/mmt/vocab#CrossBorderRegulatoryProcedureControlStartDateConfirmationIndicator>
  a rdf:Property ;
  rdfs:comment "The indication of whether or not the start date of a control has been confirmed for this cross-border regulatory procedure."^^xsd:string ;
  rdfs:domain "mmt:CrossBorderRegulatoryProcedure"^^xsd:string ;
  rdfs:label "controlStartDateConfirmationIndicator"^^xsd:string ;
  rdfs:range "xsd:boolean"^^xsd:string .

<https://edi3.org/mmt/vocab#CrossBorderRegulatoryProcedureDeclarantAssignedDeclarationID>
  a rdf:Property ;
  rdfs:comment "The declarant assigned identifier of a declaration for this cross-border regulatory procedure."^^xsd:string ;
  rdfs:domain "mmt:CrossBorderRegulatoryProcedure"^^xsd:string ;
  rdfs:label "declarantAssignedDeclarationID"^^xsd:string ;
  rdfs:range "xsd:ID"^^xsd:string .

<https://edi3.org/mmt/vocab#CrossBorderRegulatoryProcedureDeferredPaymentMethodIndicator>
  a rdf:Property ;
  rdfs:comment "The indication of whether or not the deferred payment method is applicable to this cross-border regulatory procedure."^^xsd:string ;
  rdfs:domain "mmt:CrossBorderRegulatoryProcedure"^^xsd:string ;
  rdfs:label "deferredPaymentMethodIndicator"^^xsd:string ;
  rdfs:range "xsd:boolean"^^xsd:string .

<https://edi3.org/mmt/vocab#CrossBorderRegulatoryProcedureDeferredTotalChargeAmount>
  a rdf:Property ;
  rdfs:comment "A monetary value of the total charges, including tariff and non-tariff charges, deferred for this cross-border regulatory procedure."^^xsd:string ;
  rdfs:domain "mmt:CrossBorderRegulatoryProcedure"^^xsd:string ;
  rdfs:label "deferredTotalChargeAmount"^^xsd:string ;
  rdfs:range "http://schema.org/amount"^^xsd:string .

<https://edi3.org/mmt/vocab#CrossBorderRegulatoryProcedureExportLicenceControlClassificationID>
  a rdf:Property ;
  rdfs:comment "The identifier of the export licence classification for control purposes relevant to this cross-border regulatory procedure, such as per the Wassenaar agreement concerning trade in weapons and dual-use goods and technologies."^^xsd:string ;
  rdfs:domain "mmt:CrossBorderRegulatoryProcedure"^^xsd:string ;
  rdfs:label "exportLicenceControlClassificationID"^^xsd:string ;
  rdfs:range "xsd:ID"^^xsd:string .

<https://edi3.org/mmt/vocab#CrossBorderRegulatoryProcedureGoodsStatusCode>
  a rdf:Property ;
  rdfs:comment "The code specifying the goods status for this cross-border regulatory procedure."^^xsd:string ;
  rdfs:domain "mmt:CrossBorderRegulatoryProcedure"^^xsd:string ;
  rdfs:label "goodsStatusCode"^^xsd:string ;
  rdfs:range "xsd:token"^^xsd:string .

<https://edi3.org/mmt/vocab#CrossBorderRegulatoryProcedureGuaranteeCode>
  a rdf:Property ;
  rdfs:comment "The code specifying an undertaking given in cash, bond or as a written guarantee to ensure that an obligation will be fulfilled for this cross-border regulatory procedure."^^xsd:string ;
  rdfs:domain "mmt:CrossBorderRegulatoryProcedure"^^xsd:string ;
  rdfs:label "guaranteeCode"^^xsd:string ;
  rdfs:range "xsd:token"^^xsd:string .

<https://edi3.org/mmt/vocab#CrossBorderRegulatoryProcedureGuaranteeText>
  a rdf:Property ;
  rdfs:comment "The undertaking, expressed as text, given in cash, bond or as a written guarantee to ensure that an obligation will be fulfilled for this cross-border regulatory procedure."^^xsd:string ;
  rdfs:domain "mmt:CrossBorderRegulatoryProcedure"^^xsd:string ;
  rdfs:label "guaranteeText"^^xsd:string ;
  rdfs:range "xsd:string"^^xsd:string .

<https://edi3.org/mmt/vocab#CrossBorderRegulatoryProcedureImmediatePayableTotalChargeAmount>
  a rdf:Property ;
  rdfs:comment "A monetary value of the total charges, including tariff and non-tariff charges, immediately payable for this cross-border regulatory procedure."^^xsd:string ;
  rdfs:domain "mmt:CrossBorderRegulatoryProcedure"^^xsd:string ;
  rdfs:label "immediatePayableTotalChargeAmount"^^xsd:string ;
  rdfs:range "http://schema.org/amount"^^xsd:string .

<https://edi3.org/mmt/vocab#CrossBorderRegulatoryProcedureNonTariffChargeAmount>
  a rdf:Property ;
  rdfs:comment "A monetary value of all non-tariff charges for this cross-border regulatory procedure."^^xsd:string ;
  rdfs:domain "mmt:CrossBorderRegulatoryProcedure"^^xsd:string ;
  rdfs:label "nonTariffChargeAmount"^^xsd:string ;
  rdfs:range "http://schema.org/amount"^^xsd:string .

<https://edi3.org/mmt/vocab#CrossBorderRegulatoryProcedureOriginCriteriaText>
  a rdf:Property ;
  rdfs:comment "The origin criteria, expressed as text, for this cross-border regulatory procedure."^^xsd:string ;
  rdfs:domain "mmt:CrossBorderRegulatoryProcedure"^^xsd:string ;
  rdfs:label "originCriteriaText"^^xsd:string ;
  rdfs:range "xsd:string"^^xsd:string .

<https://edi3.org/mmt/vocab#CrossBorderRegulatoryProcedurePaymentMethodCode>
  a rdf:Property ;
  rdfs:comment "The code specifying the payment method for this cross-border regulatory procedure, such as by deferred payment method."^^xsd:string ;
  rdfs:domain "mmt:CrossBorderRegulatoryProcedure"^^xsd:string ;
  rdfs:label "paymentMethodCode"^^xsd:string ;
  rdfs:range "PaymentMethodType_Сode"^^xsd:string .

<https://edi3.org/mmt/vocab#CrossBorderRegulatoryProcedurePerformanceDateTime>
  a rdf:Property ;
  rdfs:comment "A date, time, date time, or other date time value on which this cross-border regulatory procedure was, or will be, performed."^^xsd:string ;
  rdfs:domain "mmt:CrossBorderRegulatoryProcedure"^^xsd:string ;
  rdfs:label "performanceDateTime"^^xsd:string ;
  rdfs:range "xsd:datetime"^^xsd:string .

<https://edi3.org/mmt/vocab#CrossBorderRegulatoryProcedurePreviousProcedureTypeCode>
  a rdf:Property ;
  rdfs:comment "A code specifying a type of previous procedure for this cross-border regulatory procedure."^^xsd:string ;
  rdfs:domain "mmt:CrossBorderRegulatoryProcedure"^^xsd:string ;
  rdfs:label "previousProcedureTypeCode"^^xsd:string ;
  rdfs:range "xsd:token"^^xsd:string .

<https://edi3.org/mmt/vocab#CrossBorderRegulatoryProcedureQuotaID>
  a rdf:Property ;
  rdfs:comment "A quota identifier for this cross-border regulatory procedure."^^xsd:string ;
  rdfs:domain "mmt:CrossBorderRegulatoryProcedure"^^xsd:string ;
  rdfs:label "quotaID"^^xsd:string ;
  rdfs:range "xsd:ID"^^xsd:string .

<https://edi3.org/mmt/vocab#CrossBorderRegulatoryProcedureRegisteredDeferredPaymentPayerID>
  a rdf:Property ;
  rdfs:comment "The identifier of the registered deferred payment payer for this cross-border regulatory procedure."^^xsd:string ;
  rdfs:domain "mmt:CrossBorderRegulatoryProcedure"^^xsd:string ;
  rdfs:label "registeredDeferredPaymentPayerID"^^xsd:string ;
  rdfs:range "xsd:ID"^^xsd:string .

<https://edi3.org/mmt/vocab#CrossBorderRegulatoryProcedureRemark>
  a rdf:Property ;
  rdfs:comment "A remark, expressed as text, for this cross-border regulatory procedure."^^xsd:string ;
  rdfs:domain "mmt:CrossBorderRegulatoryProcedure"^^xsd:string ;
  rdfs:label "remark"^^xsd:string ;
  rdfs:range "xsd:string"^^xsd:string .

<https://edi3.org/mmt/vocab#CrossBorderRegulatoryProcedureRequestOverrideCode>
  a rdf:Property ;
  rdfs:comment "A code specifying a request, including a reason, to override previously submitted information for this cross-border regulatory procedure, such as due to an error condition."^^xsd:string ;
  rdfs:domain "mmt:CrossBorderRegulatoryProcedure"^^xsd:string ;
  rdfs:label "requestOverrideCode"^^xsd:string ;
  rdfs:range "xsd:token"^^xsd:string .

<https://edi3.org/mmt/vocab#CrossBorderRegulatoryProcedureResponsibleAgencyActionCode>
  a rdf:Property ;
  rdfs:comment "A code specifying an action for a responsible agency in this cross-border regulatory procedure."^^xsd:string ;
  rdfs:domain "mmt:CrossBorderRegulatoryProcedure"^^xsd:string ;
  rdfs:label "responsibleAgencyActionCode"^^xsd:string ;
  rdfs:range "GovernmentActionType_Сode"^^xsd:string .

<https://edi3.org/mmt/vocab#CrossBorderRegulatoryProcedureResponsibleAgencyCode>
  a rdf:Property ;
  rdfs:comment "The code specifying the agency responsible for this cross-border regulatory procedure."^^xsd:string ;
  rdfs:domain "mmt:CrossBorderRegulatoryProcedure"^^xsd:string ;
  rdfs:label "responsibleAgencyCode"^^xsd:string ;
  rdfs:range "ResponsibleAgencyType_Сode"^^xsd:string .

<https://edi3.org/mmt/vocab#CrossBorderRegulatoryProcedureResponsibleAgencyInvolvementCode>
  a rdf:Property ;
  rdfs:comment "A code specifying a responsible agency involved in this cross-border regulatory procedure."^^xsd:string ;
  rdfs:domain "mmt:CrossBorderRegulatoryProcedure"^^xsd:string ;
  rdfs:label "responsibleAgencyInvolvementCode"^^xsd:string ;
  rdfs:range "ResponsibleAgencyInvolvementType_Сode"^^xsd:string .

<https://edi3.org/mmt/vocab#CrossBorderRegulatoryProcedureTariffAmount>
  a rdf:Property ;
  rdfs:comment "A monetary value of a tariff for this cross-border regulatory procedure."^^xsd:string ;
  rdfs:domain "mmt:CrossBorderRegulatoryProcedure"^^xsd:string ;
  rdfs:label "tariffAmount"^^xsd:string ;
  rdfs:range "http://schema.org/amount"^^xsd:string .

<https://edi3.org/mmt/vocab#CrossBorderRegulatoryProcedureTariffDeductionQuantity>
  a rdf:Property ;
  rdfs:comment "A quantity to be deducted from the tariff quantity for this cross-border regulatory procedure."^^xsd:string ;
  rdfs:domain "mmt:CrossBorderRegulatoryProcedure"^^xsd:string ;
  rdfs:label "tariffDeductionQuantity"^^xsd:string ;
  rdfs:range "xsd:decimal"^^xsd:string .

<https://edi3.org/mmt/vocab#CrossBorderRegulatoryProcedureTariffQuantity>
  a rdf:Property ;
  rdfs:comment "A tariff quantity for this cross-border regulatory procedure."^^xsd:string ;
  rdfs:domain "mmt:CrossBorderRegulatoryProcedure"^^xsd:string ;
  rdfs:label "tariffQuantity"^^xsd:string ;
  rdfs:range "xsd:decimal"^^xsd:string .

<https://edi3.org/mmt/vocab#CrossBorderRegulatoryProcedureTotalChargeAmount>
  a rdf:Property ;
  rdfs:comment "A monetary value of the total charges, including tariff and non-tariff charges, for this cross-border regulatory procedure."^^xsd:string ;
  rdfs:domain "mmt:CrossBorderRegulatoryProcedure"^^xsd:string ;
  rdfs:label "totalChargeAmount"^^xsd:string ;
  rdfs:range "http://schema.org/amount"^^xsd:string .

<https://edi3.org/mmt/vocab#CrossBorderRegulatoryProcedureTotalConsignmentValueAmount>
  a rdf:Property ;
  rdfs:comment "The total monetary value for a consignment for this cross-border regulatory procedure."^^xsd:string ;
  rdfs:domain "mmt:CrossBorderRegulatoryProcedure"^^xsd:string ;
  rdfs:label "totalConsignmentValueAmount"^^xsd:string ;
  rdfs:range "http://schema.org/amount"^^xsd:string .

<https://edi3.org/mmt/vocab#CrossBorderRegulatoryProcedureTransactionNatureCode>
  a rdf:Property ;
  rdfs:comment "A code specifying the nature of a transaction for this cross-border regulatory procedure."^^xsd:string ;
  rdfs:domain "mmt:CrossBorderRegulatoryProcedure"^^xsd:string ;
  rdfs:label "transactionNatureCode"^^xsd:string ;
  rdfs:range "xsd:token"^^xsd:string .

<https://edi3.org/mmt/vocab#CrossBorderRegulatoryProcedureTransportMovementTypeCode>
  a rdf:Property ;
  rdfs:comment "A code specifying the transport movement type, such as import, export, transit, for this cross-border regulatory procedure."^^xsd:string ;
  rdfs:domain "mmt:CrossBorderRegulatoryProcedure"^^xsd:string ;
  rdfs:label "transportMovementTypeCode"^^xsd:string ;
  rdfs:range "TransportMovementType_Сode"^^xsd:string .

<https://edi3.org/mmt/vocab#CrossBorderRegulatoryProcedureTypeCode>
  a rdf:Property ;
  rdfs:comment "A code specifying a type of cross-border regulatory procedure."^^xsd:string ;
  rdfs:domain "mmt:CrossBorderRegulatoryProcedure"^^xsd:string ;
  rdfs:label "typeCode"^^xsd:string ;
  rdfs:range "xsd:token"^^xsd:string .

<https://edi3.org/mmt/vocab#CrossBorderRegulatoryProcedureUsedToDateQuotaQuantity>
  a rdf:Property ;
  rdfs:comment "The quantity of the quota used to date under this cross-border regulatory procedure."^^xsd:string ;
  rdfs:domain "mmt:CrossBorderRegulatoryProcedure"^^xsd:string ;
  rdfs:label "usedToDateQuotaQuantity"^^xsd:string ;
  rdfs:range "xsd:decimal"^^xsd:string .

<https://edi3.org/mmt/vocab#CrossBorderRegulatoryProcedureValuationBasisAmount>
  a rdf:Property ;
  rdfs:comment "The monetary value of the basis on which the valuation is, or will be, calculated for this cross-border regulatory procedure."^^xsd:string ;
  rdfs:domain "mmt:CrossBorderRegulatoryProcedure"^^xsd:string ;
  rdfs:label "valuationBasisAmount"^^xsd:string ;
  rdfs:range "http://schema.org/amount"^^xsd:string .

<https://edi3.org/mmt/vocab#DeliveryInstructions>
  a rdfs:Class ;
  rdfs:comment "Delivery information of an instructive nature."^^xsd:string ;
  rdfs:label "DeliveryInstructions"^^xsd:string .

<https://edi3.org/mmt/vocab#DeliveryInstructionsDescription>
  a rdf:Property ;
  rdfs:comment "A textual description of these delivery instructions."^^xsd:string ;
  rdfs:domain "mmt:DeliveryInstructions"^^xsd:string ;
  rdfs:label "description"^^xsd:string ;
  rdfs:range "xsd:string"^^xsd:string .

<https://edi3.org/mmt/vocab#DeliveryInstructionsDescriptionCode>
  a rdf:Property ;
  rdfs:comment "The code specifying a description of these delivery instructions."^^xsd:string ;
  rdfs:domain "mmt:DeliveryInstructions"^^xsd:string ;
  rdfs:label "descriptionCode"^^xsd:string ;
  rdfs:range "xsd:token"^^xsd:string .

<https://edi3.org/mmt/vocab#DisposalInstructions>
  a rdfs:Class ;
  rdfs:comment "A set of instructions detailing how to properly dispose of a material."^^xsd:string ;
  rdfs:label "DisposalInstructions"^^xsd:string .

<https://edi3.org/mmt/vocab#DisposalInstructionsDescription>
  a rdf:Property ;
  rdfs:comment "A textual description of these disposal instructions."^^xsd:string ;
  rdfs:domain "mmt:DisposalInstructions"^^xsd:string ;
  rdfs:label "description"^^xsd:string ;
  rdfs:range "xsd:string"^^xsd:string .

<https://edi3.org/mmt/vocab#DisposalInstructionsMaterialID>
  a rdf:Property ;
  rdfs:comment "The identifier of the material to which these disposal instructions apply."^^xsd:string ;
  rdfs:domain "mmt:DisposalInstructions"^^xsd:string ;
  rdfs:label "materialID"^^xsd:string ;
  rdfs:range "xsd:ID"^^xsd:string .

<https://edi3.org/mmt/vocab#DisposalInstructionsRecyclingDescriptionCode>
  a rdf:Property ;
  rdfs:comment "A code describing recycling in these disposal instructions."^^xsd:string ;
  rdfs:domain "mmt:DisposalInstructions"^^xsd:string ;
  rdfs:label "recyclingDescriptionCode"^^xsd:string ;
  rdfs:range "xsd:token"^^xsd:string .

<https://edi3.org/mmt/vocab#DisposalInstructionsRecyclingProcedureText>
  a rdf:Property ;
  rdfs:comment "A recycling procedure, expressed as text, for these disposal instructions."^^xsd:string ;
  rdfs:domain "mmt:DisposalInstructions"^^xsd:string ;
  rdfs:label "recyclingProcedureText"^^xsd:string ;
  rdfs:range "xsd:string"^^xsd:string .

<https://edi3.org/mmt/vocab#DistinctChemical>
  a rdfs:Class ;
  rdfs:comment "Any clearly defined substance having a defined molecular composition."^^xsd:string ;
  rdfs:label "DistinctChemical"^^xsd:string .

<https://edi3.org/mmt/vocab#DistinctChemicalCommonName>
  a rdf:Property ;
  rdfs:comment "A common name, expressed as text, for this distinct chemical."^^xsd:string ;
  rdfs:domain "mmt:DistinctChemical"^^xsd:string ;
  rdfs:label "commonName"^^xsd:string ;
  rdfs:range "xsd:string"^^xsd:string .

<https://edi3.org/mmt/vocab#DistinctChemicalFamilyName>
  a rdf:Property ;
  rdfs:comment "The family name expressed as text for this distinct chemical."^^xsd:string ;
  rdfs:domain "mmt:DistinctChemical"^^xsd:string ;
  rdfs:label "familyName"^^xsd:string ;
  rdfs:range "xsd:string"^^xsd:string .

<https://edi3.org/mmt/vocab#DistinctChemicalFormulaDescription>
  a rdf:Property ;
  rdfs:comment "The textual description of the formula for this distinct chemical."^^xsd:string ;
  rdfs:domain "mmt:DistinctChemical"^^xsd:string ;
  rdfs:label "formulaDescription"^^xsd:string ;
  rdfs:range "xsd:string"^^xsd:string .

<https://edi3.org/mmt/vocab#DistinctChemicalMolecularWeight>
  a rdf:Property ;
  rdfs:comment "The measure of the molecular weight (in grams) for this distinct chemical."^^xsd:string ;
  rdfs:domain "mmt:DistinctChemical"^^xsd:string ;
  rdfs:label "molecularWeight"^^xsd:string ;
  rdfs:range "xsd:decimal"^^xsd:string .

<https://edi3.org/mmt/vocab#DistinctChemicalScientificName>
  a rdf:Property ;
  rdfs:comment "The scientific name, expressed as text, for this distinct chemical."^^xsd:string ;
  rdfs:domain "mmt:DistinctChemical"^^xsd:string ;
  rdfs:label "scientificName"^^xsd:string ;
  rdfs:range "xsd:string"^^xsd:string .

<https://edi3.org/mmt/vocab#DistinctChemicalSynonymName>
  a rdf:Property ;
  rdfs:comment "A synonym name, expressed as text, for this distinct chemical."^^xsd:string ;
  rdfs:domain "mmt:DistinctChemical"^^xsd:string ;
  rdfs:label "synonymName"^^xsd:string ;
  rdfs:range "xsd:string"^^xsd:string .

<https://edi3.org/mmt/vocab#DistinctChemicalTypeCode>
  a rdf:Property ;
  rdfs:comment "The code specifying the type of distinct chemical."^^xsd:string ;
  rdfs:domain "mmt:DistinctChemical"^^xsd:string ;
  rdfs:label "typeCode"^^xsd:string ;
  rdfs:range "xsd:token"^^xsd:string .

<https://edi3.org/mmt/vocab#DocumentContextParameter>
  a rdfs:Class ;
  rdfs:comment "A feature that is fixed for a particular document context."^^xsd:string ;
  rdfs:label "DocumentContextParameter"^^xsd:string .

<https://edi3.org/mmt/vocab#DocumentContextParameterID>
  a rdf:Property ;
  rdfs:comment "The unique identifier of this document context parameter."^^xsd:string ;
  rdfs:domain "mmt:DocumentContextParameter"^^xsd:string ;
  rdfs:label "iD"^^xsd:string ;
  rdfs:range "xsd:ID"^^xsd:string .

<https://edi3.org/mmt/vocab#DocumentContextParameterValueText>
  a rdf:Property ;
  rdfs:comment "The value, expressed as text, of this document context parameter."^^xsd:string ;
  rdfs:domain "mmt:DocumentContextParameter"^^xsd:string ;
  rdfs:label "valueText"^^xsd:string ;
  rdfs:range "xsd:string"^^xsd:string .

<https://edi3.org/mmt/vocab#DocumentLineDocument>
  a rdfs:Class ;
  rdfs:comment "A collection of data for a line on a piece of written, printed or electronic matter that provides information or evidence."^^xsd:string ;
  rdfs:label "DocumentLineDocument"^^xsd:string .

<https://edi3.org/mmt/vocab#DocumentLineDocumentLineID>
  a rdf:Property ;
  rdfs:comment "The unique identifier of this document line."^^xsd:string ;
  rdfs:domain "mmt:DocumentLineDocument"^^xsd:string ;
  rdfs:label "lineID"^^xsd:string ;
  rdfs:range "xsd:ID"^^xsd:string .

<https://edi3.org/mmt/vocab#DocumentLineDocumentStatusCode>
  a rdf:Property ;
  rdfs:comment "The code specifying the status of this document line."^^xsd:string ;
  rdfs:domain "mmt:DocumentLineDocument"^^xsd:string ;
  rdfs:label "statusCode"^^xsd:string ;
  rdfs:range "ActionType_Сode"^^xsd:string .

<https://edi3.org/mmt/vocab#DocumentAuthentication>
  a rdfs:Class ;
  rdfs:comment "A proof that a document is genuine."^^xsd:string ;
  rdfs:label "DocumentAuthentication"^^xsd:string .

<https://edi3.org/mmt/vocab#DocumentAuthenticationActualDateTime>
  a rdf:Property ;
  rdfs:comment "The actual date, time, date time, or other date time value of this document authentication."^^xsd:string ;
  rdfs:domain "mmt:DocumentAuthentication"^^xsd:string ;
  rdfs:label "actualDateTime"^^xsd:string ;
  rdfs:range "xsd:datetime"^^xsd:string .

<https://edi3.org/mmt/vocab#DocumentAuthenticationGovernmentActionTypeCode>
  a rdf:Property ;
  rdfs:comment "The code specifying the type of document authentication."^^xsd:string ;
  rdfs:domain "mmt:DocumentAuthentication"^^xsd:string ;
  rdfs:label "governmentActionTypeCode"^^xsd:string ;
  rdfs:range "GovernmentActionType_Сode"^^xsd:string .

<https://edi3.org/mmt/vocab#DocumentAuthenticationID>
  a rdf:Property ;
  rdfs:comment "A unique identifier for this document authentication."^^xsd:string ;
  rdfs:domain "mmt:DocumentAuthentication"^^xsd:string ;
  rdfs:label "iD"^^xsd:string ;
  rdfs:range "xsd:ID"^^xsd:string .

<https://edi3.org/mmt/vocab#DocumentAuthenticationRepresentationTypeCode>
  a rdf:Property ;
  rdfs:comment "The code specifying the type of representation of this document authentication, such as direct or indirect."^^xsd:string ;
  rdfs:domain "mmt:DocumentAuthentication"^^xsd:string ;
  rdfs:label "representationTypeCode"^^xsd:string ;
  rdfs:range "xsd:token"^^xsd:string .

<https://edi3.org/mmt/vocab#DocumentAuthenticationSignatoryText>
  a rdf:Property ;
  rdfs:comment "The signatory, expressed as text, for this document authentication."^^xsd:string ;
  rdfs:domain "mmt:DocumentAuthentication"^^xsd:string ;
  rdfs:label "signatoryText"^^xsd:string ;
  rdfs:range "xsd:string"^^xsd:string .

<https://edi3.org/mmt/vocab#DocumentAuthenticationStatement>
  a rdf:Property ;
  rdfs:comment "The statement, expressed as text, for this document authentication."^^xsd:string ;
  rdfs:domain "mmt:DocumentAuthentication"^^xsd:string ;
  rdfs:label "statement"^^xsd:string ;
  rdfs:range "xsd:string"^^xsd:string .

<https://edi3.org/mmt/vocab#DocumentAuthenticationStatementCode>
  a rdf:Property ;
  rdfs:comment "The code specifying the statement for this document authentication."^^xsd:string ;
  rdfs:domain "mmt:DocumentAuthentication"^^xsd:string ;
  rdfs:label "statementCode"^^xsd:string ;
  rdfs:range "xsd:token"^^xsd:string .

<https://edi3.org/mmt/vocab#DocumentClause>
  a rdfs:Class ;
  rdfs:comment "A distinct article or provision in a document, which requires compliance."^^xsd:string ;
  rdfs:label "DocumentClause"^^xsd:string .

<https://edi3.org/mmt/vocab#DocumentClauseContentText>
  a rdf:Property ;
  rdfs:comment "Content, expressed as text, of this document clause."^^xsd:string ;
  rdfs:domain "mmt:DocumentClause"^^xsd:string ;
  rdfs:label "contentText"^^xsd:string ;
  rdfs:range "xsd:string"^^xsd:string .

<https://edi3.org/mmt/vocab#DocumentClauseID>
  a rdf:Property ;
  rdfs:comment "The unique identifier of this document clause."^^xsd:string ;
  rdfs:domain "mmt:DocumentClause"^^xsd:string ;
  rdfs:label "iD"^^xsd:string ;
  rdfs:range "xsd:ID"^^xsd:string .

<https://edi3.org/mmt/vocab#DocumentVersion>
  a rdfs:Class ;
  rdfs:comment "A specific variant of a document."^^xsd:string ;
  rdfs:label "DocumentVersion"^^xsd:string .

<https://edi3.org/mmt/vocab#DocumentVersionID>
  a rdf:Property ;
  rdfs:comment "The unique identifier for this document version."^^xsd:string ;
  rdfs:domain "mmt:DocumentVersion"^^xsd:string ;
  rdfs:label "iD"^^xsd:string ;
  rdfs:range "xsd:ID"^^xsd:string .

<https://edi3.org/mmt/vocab#DocumentVersionIssueDateTime>
  a rdf:Property ;
  rdfs:comment "The date, time, date and time or other date time value of issue of this document version."^^xsd:string ;
  rdfs:domain "mmt:DocumentVersion"^^xsd:string ;
  rdfs:label "issueDateTime"^^xsd:string ;
  rdfs:range "xsd:datetime"^^xsd:string .

<https://edi3.org/mmt/vocab#DocumentVersionName>
  a rdf:Property ;
  rdfs:comment "The name, expressed as text, of this document version."^^xsd:string ;
  rdfs:domain "mmt:DocumentVersion"^^xsd:string ;
  rdfs:label "name"^^xsd:string ;
  rdfs:range "xsd:string"^^xsd:string .

<https://edi3.org/mmt/vocab#ExchangedDocumentContext>
  a rdfs:Class ;
  rdfs:comment "The scenario or setting of an exchanged document, such as its business process application context."^^xsd:string ;
  rdfs:label "ExchangedDocumentContext"^^xsd:string .

<https://edi3.org/mmt/vocab#ExchangedDocumentContextTestIndicator>
  a rdf:Property ;
  rdfs:comment "The indication of whether or not this exchanged document context is a test."^^xsd:string ;
  rdfs:domain "mmt:ExchangedDocumentContext"^^xsd:string ;
  rdfs:label "testIndicator"^^xsd:string ;
  rdfs:range "xsd:boolean"^^xsd:string .

<https://edi3.org/mmt/vocab#ExchangedDocumentContextTransactionID>
  a rdf:Property ;
  rdfs:comment "The identifier of a specified transaction in this exchanged document context."^^xsd:string ;
  rdfs:domain "mmt:ExchangedDocumentContext"^^xsd:string ;
  rdfs:label "transactionID"^^xsd:string ;
  rdfs:range "xsd:ID"^^xsd:string .

<https://edi3.org/mmt/vocab#ExchangedDeclaration>
  a rdfs:Class ;
  rdfs:comment "A collection of data for a piece of written, printed or electronic matter that is exchanged between two parties as a formal declaration."^^xsd:string ;
  rdfs:label "ExchangedDeclaration"^^xsd:string .

<https://edi3.org/mmt/vocab#ExchangedDeclarationCurrencyExchangeRate>
  a rdf:Property ;
  rdfs:comment "The rate of currency exchange in this exchanged declaration."^^xsd:string ;
  rdfs:domain "mmt:ExchangedDeclaration"^^xsd:string ;
  rdfs:label "currencyExchangeRate"^^xsd:string ;
  rdfs:range "xsd:decimal"^^xsd:string .

<https://edi3.org/mmt/vocab#ExchangedDeclarationCustomsValueAmount>
  a rdf:Property ;
  rdfs:comment "The monetary value specified for customs purposes in this exchanged declaration."^^xsd:string ;
  rdfs:domain "mmt:ExchangedDeclaration"^^xsd:string ;
  rdfs:label "customsValueAmount"^^xsd:string ;
  rdfs:range "http://schema.org/amount"^^xsd:string .

<https://edi3.org/mmt/vocab#ExchangedDeclarationFormattedIssueDateTime>
  a rdf:Property ;
  rdfs:comment "The date, time, date time or other date time value for the issuance of this exchanged declaration."^^xsd:string ;
  rdfs:domain "mmt:ExchangedDeclaration"^^xsd:string ;
  rdfs:label "formattedIssueDateTime"^^xsd:string ;
  rdfs:range "xsd:datetime"^^xsd:string .

<https://edi3.org/mmt/vocab#ExchangedDeclarationFormattedJurisdictionEntryDateTime>
  a rdf:Property ;
  rdfs:comment "The date, time, date time or other date time value when the items which are a subject of this exchanged declaration enter a jurisdiction, such as the actual date of arrival of a means of transport."^^xsd:string ;
  rdfs:domain "mmt:ExchangedDeclaration"^^xsd:string ;
  rdfs:label "formattedJurisdictionEntryDateTime"^^xsd:string ;
  rdfs:range "xsd:datetime"^^xsd:string .

<https://edi3.org/mmt/vocab#ExchangedDeclarationGrossWeight>
  a rdf:Property ;
  rdfs:comment "The gross weight measure specified in this exchanged declaration."^^xsd:string ;
  rdfs:domain "mmt:ExchangedDeclaration"^^xsd:string ;
  rdfs:label "grossWeight"^^xsd:string ;
  rdfs:range "xsd:decimal"^^xsd:string .

<https://edi3.org/mmt/vocab#ExchangedDeclarationID>
  a rdf:Property ;
  rdfs:comment "An identifier for this exchanged declaration."^^xsd:string ;
  rdfs:domain "mmt:ExchangedDeclaration"^^xsd:string ;
  rdfs:label "iD"^^xsd:string ;
  rdfs:range "xsd:ID"^^xsd:string .

<https://edi3.org/mmt/vocab#ExchangedDeclarationProcedureCode>
  a rdf:Property ;
  rdfs:comment "A code specifying a procedure for this exchanged declaration."^^xsd:string ;
  rdfs:domain "mmt:ExchangedDeclaration"^^xsd:string ;
  rdfs:label "procedureCode"^^xsd:string ;
  rdfs:range "xsd:token"^^xsd:string .

<https://edi3.org/mmt/vocab#ExchangedDeclarationSpecificCircumstanceCode>
  a rdf:Property ;
  rdfs:comment "The code specifying a specific circumstance in this exchanged declaration."^^xsd:string ;
  rdfs:domain "mmt:ExchangedDeclaration"^^xsd:string ;
  rdfs:label "specificCircumstanceCode"^^xsd:string ;
  rdfs:range "xsd:token"^^xsd:string .

<https://edi3.org/mmt/vocab#ExchangedDeclarationStatisticalValueAmount>
  a rdf:Property ;
  rdfs:comment "The monetary value specified for statistical purposes in this exchanged declaration."^^xsd:string ;
  rdfs:domain "mmt:ExchangedDeclaration"^^xsd:string ;
  rdfs:label "statisticalValueAmount"^^xsd:string ;
  rdfs:range "http://schema.org/amount"^^xsd:string .

<https://edi3.org/mmt/vocab#ExchangedDeclarationTotalInvoiceAmount>
  a rdf:Property ;
  rdfs:comment "The total invoice monetary value specified in this exchanged declaration."^^xsd:string ;
  rdfs:domain "mmt:ExchangedDeclaration"^^xsd:string ;
  rdfs:label "totalInvoiceAmount"^^xsd:string ;
  rdfs:range "http://schema.org/amount"^^xsd:string .

<https://edi3.org/mmt/vocab#ExchangedDeclarationTotalPackageQuantity>
  a rdf:Property ;
  rdfs:comment "The total package quantity specified in this exchanged declaration."^^xsd:string ;
  rdfs:domain "mmt:ExchangedDeclaration"^^xsd:string ;
  rdfs:label "totalPackageQuantity"^^xsd:string ;
  rdfs:range "xsd:decimal"^^xsd:string .

<https://edi3.org/mmt/vocab#ExchangedDeclarationTypeCode>
  a rdf:Property ;
  rdfs:comment "The code specifying the type of this exchanged declaration."^^xsd:string ;
  rdfs:domain "mmt:ExchangedDeclaration"^^xsd:string ;
  rdfs:label "typeCode"^^xsd:string ;
  rdfs:range "DocumentNameType_Сode"^^xsd:string .

<https://edi3.org/mmt/vocab#ExchangedDeclarationVersionID>
  a rdf:Property ;
  rdfs:comment "The identifier for the version of this exchanged declaration."^^xsd:string ;
  rdfs:domain "mmt:ExchangedDeclaration"^^xsd:string ;
  rdfs:label "versionID"^^xsd:string ;
  rdfs:range "xsd:ID"^^xsd:string .

<https://edi3.org/mmt/vocab#ExchangedDocument>
  a rdfs:Class ;
  rdfs:comment "A collection of data for a piece of written, printed or electronic matter that is exchanged between two or more parties."^^xsd:string ;
  rdfs:label "ExchangedDocument"^^xsd:string .

<https://edi3.org/mmt/vocab#ExchangedDocumentAcceptanceDateTime>
  a rdf:Property ;
  rdfs:comment "The date, time, date time, or other date time value for the acceptance of this exchanged document."^^xsd:string ;
  rdfs:domain "mmt:ExchangedDocument"^^xsd:string ;
  rdfs:label "acceptanceDateTime"^^xsd:string ;
  rdfs:range "xsd:datetime"^^xsd:string .

<https://edi3.org/mmt/vocab#ExchangedDocumentAmendmentPurposeCode>
  a rdf:Property ;
  rdfs:comment "A code specifying a purpose of an amendment to this exchanged document."^^xsd:string ;
  rdfs:domain "mmt:ExchangedDocument"^^xsd:string ;
  rdfs:label "amendmentPurposeCode"^^xsd:string ;
  rdfs:range "xsd:token"^^xsd:string .

<https://edi3.org/mmt/vocab#ExchangedDocumentCancellationDateTime>
  a rdf:Property ;
  rdfs:comment "The date, time, date time, or other date time value of a cancellation of the exchanged document."^^xsd:string ;
  rdfs:domain "mmt:ExchangedDocument"^^xsd:string ;
  rdfs:label "cancellationDateTime"^^xsd:string ;
  rdfs:range "xsd:datetime"^^xsd:string .

<https://edi3.org/mmt/vocab#ExchangedDocumentCategoryCode>
  a rdf:Property ;
  rdfs:comment "The code specifying a category for this exchanged document."^^xsd:string ;
  rdfs:domain "mmt:ExchangedDocument"^^xsd:string ;
  rdfs:label "categoryCode"^^xsd:string ;
  rdfs:range "xsd:token"^^xsd:string .

<https://edi3.org/mmt/vocab#ExchangedDocumentCopyIndicator>
  a rdf:Property ;
  rdfs:comment "The indication of whether or not this exchanged document is a copy."^^xsd:string ;
  rdfs:domain "mmt:ExchangedDocument"^^xsd:string ;
  rdfs:label "copyIndicator"^^xsd:string ;
  rdfs:range "xsd:boolean"^^xsd:string .

<https://edi3.org/mmt/vocab#ExchangedDocumentCopyIssuedQuantity>
  a rdf:Property ;
  rdfs:comment "The number of copies issued of this exchanged document."^^xsd:string ;
  rdfs:domain "mmt:ExchangedDocument"^^xsd:string ;
  rdfs:label "copyIssuedQuantity"^^xsd:string ;
  rdfs:range "xsd:decimal"^^xsd:string .

<https://edi3.org/mmt/vocab#ExchangedDocumentCopyRequiredQuantity>
  a rdf:Property ;
  rdfs:comment "The number of copies required of this exchanged document."^^xsd:string ;
  rdfs:domain "mmt:ExchangedDocument"^^xsd:string ;
  rdfs:label "copyRequiredQuantity"^^xsd:string ;
  rdfs:range "xsd:decimal"^^xsd:string .

<https://edi3.org/mmt/vocab#ExchangedDocumentCreationDateTime>
  a rdf:Property ;
  rdfs:comment "The date, time, date time, or other date time value of a creation of this exchanged document."^^xsd:string ;
  rdfs:domain "mmt:ExchangedDocument"^^xsd:string ;
  rdfs:label "creationDateTime"^^xsd:string ;
  rdfs:range "xsd:datetime"^^xsd:string .

<https://edi3.org/mmt/vocab#ExchangedDocumentCustomsID>
  a rdf:Property ;
  rdfs:comment "A unique identifier, for customs purposes, for this exchanged document."^^xsd:string ;
  rdfs:domain "mmt:ExchangedDocument"^^xsd:string ;
  rdfs:label "customsID"^^xsd:string ;
  rdfs:range "xsd:ID"^^xsd:string .

<https://edi3.org/mmt/vocab#ExchangedDocumentID>
  a rdf:Property ;
  rdfs:comment "The unique identifier of this exchanged document."^^xsd:string ;
  rdfs:domain "mmt:ExchangedDocument"^^xsd:string ;
  rdfs:label "iD"^^xsd:string ;
  rdfs:range "xsd:ID"^^xsd:string .

<https://edi3.org/mmt/vocab#ExchangedDocumentIssueDateTime>
  a rdf:Property ;
  rdfs:comment "The date, time, date time or other date time value for the issuance of this exchanged document."^^xsd:string ;
  rdfs:domain "mmt:ExchangedDocument"^^xsd:string ;
  rdfs:label "issueDateTime"^^xsd:string ;
  rdfs:range "xsd:datetime"^^xsd:string .

<https://edi3.org/mmt/vocab#ExchangedDocumentLanguageCode>
  a rdf:Property ;
  rdfs:comment "A unique identifier for a language used in this exchanged document."^^xsd:string ;
  rdfs:domain "mmt:ExchangedDocument"^^xsd:string ;
  rdfs:label "languageCode"^^xsd:string ;
  rdfs:range "xsd:ID"^^xsd:string .

<https://edi3.org/mmt/vocab#ExchangedDocumentName>
  a rdf:Property ;
  rdfs:comment "A name, expressed as text, of this exchanged document."^^xsd:string ;
  rdfs:domain "mmt:ExchangedDocument"^^xsd:string ;
  rdfs:label "name"^^xsd:string ;
  rdfs:range "xsd:string"^^xsd:string .

<https://edi3.org/mmt/vocab#ExchangedDocumentOriginalIssuedQuantity>
  a rdf:Property ;
  rdfs:comment "The number of originals issued of this exchanged document."^^xsd:string ;
  rdfs:domain "mmt:ExchangedDocument"^^xsd:string ;
  rdfs:label "originalIssuedQuantity"^^xsd:string ;
  rdfs:range "xsd:decimal"^^xsd:string .

<https://edi3.org/mmt/vocab#ExchangedDocumentOriginalRequiredQuantity>
  a rdf:Property ;
  rdfs:comment "The number of originals required of this exchanged document."^^xsd:string ;
  rdfs:domain "mmt:ExchangedDocument"^^xsd:string ;
  rdfs:label "originalRequiredQuantity"^^xsd:string ;
  rdfs:range "xsd:decimal"^^xsd:string .

<https://edi3.org/mmt/vocab#ExchangedDocumentPurposeCode>
  a rdf:Property ;
  rdfs:comment "A code specifying the purpose of this exchanged document, such as request or reminder."^^xsd:string ;
  rdfs:domain "mmt:ExchangedDocument"^^xsd:string ;
  rdfs:label "purposeCode"^^xsd:string ;
  rdfs:range "MessageFunctionType_Сode"^^xsd:string .

<https://edi3.org/mmt/vocab#ExchangedDocumentRecipientAssignedID>
  a rdf:Property ;
  rdfs:comment "A unique recipient assigned identifier for this exchanged document."^^xsd:string ;
  rdfs:domain "mmt:ExchangedDocument"^^xsd:string ;
  rdfs:label "recipientAssignedID"^^xsd:string ;
  rdfs:range "xsd:ID"^^xsd:string .

<https://edi3.org/mmt/vocab#ExchangedDocumentRejectionResponseDateTime>
  a rdf:Property ;
  rdfs:comment "A date, time, date time, or other date time value of a rejection response of the exchanged document."^^xsd:string ;
  rdfs:domain "mmt:ExchangedDocument"^^xsd:string ;
  rdfs:label "rejectionResponseDateTime"^^xsd:string ;
  rdfs:range "xsd:datetime"^^xsd:string .

<https://edi3.org/mmt/vocab#ExchangedDocumentRemark>
  a rdf:Property ;
  rdfs:comment "A remark, expressed as text, regarding this exchanged document."^^xsd:string ;
  rdfs:domain "mmt:ExchangedDocument"^^xsd:string ;
  rdfs:label "remark"^^xsd:string ;
  rdfs:range "xsd:string"^^xsd:string .

<https://edi3.org/mmt/vocab#ExchangedDocumentResponseDateTime>
  a rdf:Property ;
  rdfs:comment "A date, time, date time, or other date time value of a response of the exchanged document."^^xsd:string ;
  rdfs:domain "mmt:ExchangedDocument"^^xsd:string ;
  rdfs:label "responseDateTime"^^xsd:string ;
  rdfs:range "xsd:datetime"^^xsd:string .

<https://edi3.org/mmt/vocab#ExchangedDocumentResponseRequestTypeCode>
  a rdf:Property ;
  rdfs:comment "A code specifying a type of response requested for this exchanged document."^^xsd:string ;
  rdfs:domain "mmt:ExchangedDocument"^^xsd:string ;
  rdfs:label "responseRequestTypeCode"^^xsd:string ;
  rdfs:range "xsd:token"^^xsd:string .

<https://edi3.org/mmt/vocab#ExchangedDocumentRevisionDateTime>
  a rdf:Property ;
  rdfs:comment "The date, time, date time or other date time value for the revision of this exchanged document."^^xsd:string ;
  rdfs:domain "mmt:ExchangedDocument"^^xsd:string ;
  rdfs:label "revisionDateTime"^^xsd:string ;
  rdfs:range "xsd:datetime"^^xsd:string .

<https://edi3.org/mmt/vocab#ExchangedDocumentSenderAssignedID>
  a rdf:Property ;
  rdfs:comment "A unique sender assigned identifier for this exchanged document."^^xsd:string ;
  rdfs:domain "mmt:ExchangedDocument"^^xsd:string ;
  rdfs:label "senderAssignedID"^^xsd:string ;
  rdfs:range "xsd:ID"^^xsd:string .

<https://edi3.org/mmt/vocab#ExchangedDocumentStatusCode>
  a rdf:Property ;
  rdfs:comment "The code specifying the status of this exchanged document."^^xsd:string ;
  rdfs:domain "mmt:ExchangedDocument"^^xsd:string ;
  rdfs:label "statusCode"^^xsd:string ;
  rdfs:range "DocumentStatusType_Сode"^^xsd:string .

<https://edi3.org/mmt/vocab#ExchangedDocumentSubmissionDateTime>
  a rdf:Property ;
  rdfs:comment "The date, time, date time or other date time value for the formal submission of this exchanged document to a receiver by a sender."^^xsd:string ;
  rdfs:domain "mmt:ExchangedDocument"^^xsd:string ;
  rdfs:label "submissionDateTime"^^xsd:string ;
  rdfs:range "xsd:datetime"^^xsd:string .

<https://edi3.org/mmt/vocab#ExchangedDocumentTraderAssignedID>
  a rdf:Property ;
  rdfs:comment "A unique trader assigned identifier for this exchanged document."^^xsd:string ;
  rdfs:domain "mmt:ExchangedDocument"^^xsd:string ;
  rdfs:label "traderAssignedID"^^xsd:string ;
  rdfs:range "xsd:ID"^^xsd:string .

<https://edi3.org/mmt/vocab#ExchangedDocumentTypeCode>
  a rdf:Property ;
  rdfs:comment "The code specifying the type of exchanged document."^^xsd:string ;
  rdfs:domain "mmt:ExchangedDocument"^^xsd:string ;
  rdfs:label "typeCode"^^xsd:string ;
  rdfs:range "DocumentNameType_Сode"^^xsd:string .

<https://edi3.org/mmt/vocab#ExchangedDocumentVersionID>
  a rdf:Property ;
  rdfs:comment "The unique identifier for the version of this exchanged document."^^xsd:string ;
  rdfs:domain "mmt:ExchangedDocument"^^xsd:string ;
  rdfs:label "versionID"^^xsd:string ;
  rdfs:range "xsd:ID"^^xsd:string .

<https://edi3.org/mmt/vocab#FinancialAdjustment>
  a rdfs:Class ;
  rdfs:comment "A correction or modification to reflect actual financial conditions."^^xsd:string ;
  rdfs:label "FinancialAdjustment"^^xsd:string .

<https://edi3.org/mmt/vocab#FinancialAdjustmentActualAmount>
  a rdf:Property ;
  rdfs:comment "An actual monetary value added or subtracted as a result of this financial adjustment."^^xsd:string ;
  rdfs:domain "mmt:FinancialAdjustment"^^xsd:string ;
  rdfs:label "actualAmount"^^xsd:string ;
  rdfs:range "http://schema.org/amount"^^xsd:string .

<https://edi3.org/mmt/vocab#FinancialAdjustmentActualDateTime>
  a rdf:Property ;
  rdfs:comment "The actual date, time, date time, or other date time value of this financial adjustment."^^xsd:string ;
  rdfs:domain "mmt:FinancialAdjustment"^^xsd:string ;
  rdfs:label "actualDateTime"^^xsd:string ;
  rdfs:range "xsd:datetime"^^xsd:string .

<https://edi3.org/mmt/vocab#FinancialAdjustmentActualQuantity>
  a rdf:Property ;
  rdfs:comment "The actual quantity added or subtracted as a result of this financial adjustment."^^xsd:string ;
  rdfs:domain "mmt:FinancialAdjustment"^^xsd:string ;
  rdfs:label "actualQuantity"^^xsd:string ;
  rdfs:range "xsd:decimal"^^xsd:string .

<https://edi3.org/mmt/vocab#FinancialAdjustmentReasonCode>
  a rdf:Property ;
  rdfs:comment "A code specifying a reason for this financial adjustment."^^xsd:string ;
  rdfs:domain "mmt:FinancialAdjustment"^^xsd:string ;
  rdfs:label "reasonCode"^^xsd:string ;
  rdfs:range "xsd:token"^^xsd:string .

<https://edi3.org/mmt/vocab#FinancialAdjustmentReasonText>
  a rdf:Property ;
  rdfs:comment "A reason, expressed as text, for this financial adjustment."^^xsd:string ;
  rdfs:domain "mmt:FinancialAdjustment"^^xsd:string ;
  rdfs:label "reasonText"^^xsd:string ;
  rdfs:range "xsd:string"^^xsd:string .

<https://edi3.org/mmt/vocab#GeographicalCoordinate>
  a rdfs:Class ;
  rdfs:comment "A set of geographical coordinates of a specific point such as the longitude, latitude and altitude."^^xsd:string ;
  rdfs:label "GeographicalCoordinate"^^xsd:string .

<https://edi3.org/mmt/vocab#GeographicalCoordinateAltimetricSystemID>
  a rdf:Property ;
  rdfs:comment "The unique identifier of the system used for measuring the altitude."^^xsd:string ;
  rdfs:domain "mmt:GeographicalCoordinate"^^xsd:string ;
  rdfs:label "altimetricSystemID"^^xsd:string ;
  rdfs:range "xsd:ID"^^xsd:string .

<https://edi3.org/mmt/vocab#GeographicalCoordinateAltitude>
  a rdf:Property ;
  rdfs:comment "The measure of the altitude that reflects the vertical elevation of an object above a surface for this geographical coordinate (Reference ISO 6709)."^^xsd:string ;
  rdfs:domain "mmt:GeographicalCoordinate"^^xsd:string ;
  rdfs:label "altitude"^^xsd:string ;
  rdfs:range "xsd:decimal"^^xsd:string .

<https://edi3.org/mmt/vocab#GeographicalCoordinateID>
  a rdf:Property ;
  rdfs:comment "The unique identifier for this geographical coordinate."^^xsd:string ;
  rdfs:domain "mmt:GeographicalCoordinate"^^xsd:string ;
  rdfs:label "iD"^^xsd:string ;
  rdfs:range "xsd:ID"^^xsd:string .

<https://edi3.org/mmt/vocab#GeographicalCoordinateLatitude>
  a rdf:Property ;
  rdfs:comment "The measure of the latitude as an angular distance north or south from the Equator meridian to the meridian of a specific place for this geographical coordinate (Reference ISO 6709)."^^xsd:string ;
  rdfs:domain "mmt:GeographicalCoordinate"^^xsd:string ;
  rdfs:label "latitude"^^xsd:string ;
  rdfs:range "xsd:decimal"^^xsd:string .

<https://edi3.org/mmt/vocab#GeographicalCoordinateLatitudeDirectionIndicator>
  a rdf:Property ;
  rdfs:comment "The indication of whether the latitude compass direction from the Equator meridian to the meridian of a specific place is North (+) or South (-)  (Reference ISO 6709)."^^xsd:string ;
  rdfs:domain "mmt:GeographicalCoordinate"^^xsd:string ;
  rdfs:label "latitudeDirectionIndicator"^^xsd:string ;
  rdfs:range "xsd:boolean"^^xsd:string .

<https://edi3.org/mmt/vocab#GeographicalCoordinateLongitude>
  a rdf:Property ;
  rdfs:comment "The measure of the longitude as an angular distance east or west from the Greenwich meridian to the meridian of a specific place (Reference ISO 6709)."^^xsd:string ;
  rdfs:domain "mmt:GeographicalCoordinate"^^xsd:string ;
  rdfs:label "longitude"^^xsd:string ;
  rdfs:range "xsd:decimal"^^xsd:string .

<https://edi3.org/mmt/vocab#GeographicalCoordinateLongitudeDirectionIndicator>
  a rdf:Property ;
  rdfs:comment "The indication of whether the longitude as a compass direction from the Greenwich meridian to the meridian of a specific place is East (+) or West (-) for this geographical coordinate (Reference ISO 6709)."^^xsd:string ;
  rdfs:domain "mmt:GeographicalCoordinate"^^xsd:string ;
  rdfs:label "longitudeDirectionIndicator"^^xsd:string ;
  rdfs:range "xsd:boolean"^^xsd:string .

<https://edi3.org/mmt/vocab#GeographicalCoordinateSystemID>
  a rdf:Property ;
  rdfs:comment "The unique identifier of the reference system used for measuring a geographical coordinate."^^xsd:string ;
  rdfs:domain "mmt:GeographicalCoordinate"^^xsd:string ;
  rdfs:label "systemID"^^xsd:string ;
  rdfs:range "xsd:ID"^^xsd:string .

<https://edi3.org/mmt/vocab#GovernmentRegistration>
  a rdfs:Class ;
  rdfs:comment "The recording of items or details for a governmental purpose."^^xsd:string ;
  rdfs:label "GovernmentRegistration"^^xsd:string .

<https://edi3.org/mmt/vocab#GovernmentRegistrationCategoryCode>
  a rdf:Property ;
  rdfs:comment "A code specifying a category of this government registration."^^xsd:string ;
  rdfs:domain "mmt:GovernmentRegistration"^^xsd:string ;
  rdfs:label "categoryCode"^^xsd:string ;
  rdfs:range "xsd:token"^^xsd:string .

<https://edi3.org/mmt/vocab#GovernmentRegistrationCountryCode>
  a rdf:Property ;
  rdfs:comment "The identifier of the country for this government registration."^^xsd:string ;
  rdfs:domain "mmt:GovernmentRegistration"^^xsd:string ;
  rdfs:label "countryCode"^^xsd:string ;
  rdfs:range "xsd:ID"^^xsd:string .

<https://edi3.org/mmt/vocab#GovernmentRegistrationCountrySubDivisionCode>
  a rdf:Property ;
  rdfs:comment "The identifier of the country sub-division for this registration."^^xsd:string ;
  rdfs:domain "mmt:GovernmentRegistration"^^xsd:string ;
  rdfs:label "countrySubDivisionCode"^^xsd:string ;
  rdfs:range "xsd:ID"^^xsd:string .

<https://edi3.org/mmt/vocab#GovernmentRegistrationID>
  a rdf:Property ;
  rdfs:comment "An identifier for this government registration."^^xsd:string ;
  rdfs:domain "mmt:GovernmentRegistration"^^xsd:string ;
  rdfs:label "iD"^^xsd:string ;
  rdfs:range "xsd:ID"^^xsd:string .

<https://edi3.org/mmt/vocab#GovernmentRegistrationLastRegisteredYear>
  a rdf:Property ;
  rdfs:comment "The last registered year of this government registration."^^xsd:string ;
  rdfs:domain "mmt:GovernmentRegistration"^^xsd:string ;
  rdfs:label "lastRegisteredYear"^^xsd:string ;
  rdfs:range "xsd:datetime"^^xsd:string .

<https://edi3.org/mmt/vocab#GovernmentRegistrationLicenceID>
  a rdf:Property ;
  rdfs:comment "The identifier of a licence for this government registration."^^xsd:string ;
  rdfs:domain "mmt:GovernmentRegistration"^^xsd:string ;
  rdfs:label "licenceID"^^xsd:string ;
  rdfs:range "xsd:ID"^^xsd:string .

<https://edi3.org/mmt/vocab#GovernmentRegistrationRecordedDate>
  a rdf:Property ;
  rdfs:comment "The date that this government registration was recorded."^^xsd:string ;
  rdfs:domain "mmt:GovernmentRegistration"^^xsd:string ;
  rdfs:label "recordedDate"^^xsd:string ;
  rdfs:range "xsd:date"^^xsd:string .

<https://edi3.org/mmt/vocab#GovernmentRegistrationTypeCode>
  a rdf:Property ;
  rdfs:comment "A code specifying a type of government registration."^^xsd:string ;
  rdfs:domain "mmt:GovernmentRegistration"^^xsd:string ;
  rdfs:label "typeCode"^^xsd:string ;
  rdfs:range "xsd:token"^^xsd:string .

<https://edi3.org/mmt/vocab#GovernmentRegistrationVersionID>
  a rdf:Property ;
  rdfs:comment "The identifier of the version of this government registration."^^xsd:string ;
  rdfs:domain "mmt:GovernmentRegistration"^^xsd:string ;
  rdfs:label "versionID"^^xsd:string ;
  rdfs:range "xsd:ID"^^xsd:string .

<https://edi3.org/mmt/vocab#HandlingInstructions>
  a rdfs:Class ;
  rdfs:comment "Handling information of an instructive nature."^^xsd:string ;
  rdfs:label "HandlingInstructions"^^xsd:string .

<https://edi3.org/mmt/vocab#HandlingInstructionsDescription>
  a rdf:Property ;
  rdfs:comment "A textual description of these handling instructions."^^xsd:string ;
  rdfs:domain "mmt:HandlingInstructions"^^xsd:string ;
  rdfs:label "description"^^xsd:string ;
  rdfs:range "xsd:string"^^xsd:string .

<https://edi3.org/mmt/vocab#HandlingInstructionsDescriptionCode>
  a rdf:Property ;
  rdfs:comment "A code specifying a description of these handling instructions."^^xsd:string ;
  rdfs:domain "mmt:HandlingInstructions"^^xsd:string ;
  rdfs:label "descriptionCode"^^xsd:string ;
  rdfs:range "xsd:token"^^xsd:string .

<https://edi3.org/mmt/vocab#HandlingInstructionsMaximumStackabilityQuantity>
  a rdf:Property ;
  rdfs:comment "The maximum number of units which can be stacked on top of each other according to these handling instructions."^^xsd:string ;
  rdfs:domain "mmt:HandlingInstructions"^^xsd:string ;
  rdfs:label "maximumStackabilityQuantity"^^xsd:string ;
  rdfs:range "xsd:decimal"^^xsd:string .

<https://edi3.org/mmt/vocab#HandlingInstructionsMaximumStackabilityWeight>
  a rdf:Property ;
  rdfs:comment "The maximum stackability weight applicable to these handling instructions."^^xsd:string ;
  rdfs:domain "mmt:HandlingInstructions"^^xsd:string ;
  rdfs:label "maximumStackabilityWeight"^^xsd:string ;
  rdfs:range "xsd:decimal"^^xsd:string .

<https://edi3.org/mmt/vocab#HandlingInstructionsMaximumStorageHumidity>
  a rdf:Property ;
  rdfs:comment "The measure of the maximum storage humidity applicable to these handling instructions."^^xsd:string ;
  rdfs:domain "mmt:HandlingInstructions"^^xsd:string ;
  rdfs:label "maximumStorageHumidity"^^xsd:string ;
  rdfs:range "xsd:decimal"^^xsd:string .

<https://edi3.org/mmt/vocab#HandlingInstructionsMinimumStorageHumidity>
  a rdf:Property ;
  rdfs:comment "The measure of the minimum storage humidity applicable to these handling instructions."^^xsd:string ;
  rdfs:domain "mmt:HandlingInstructions"^^xsd:string ;
  rdfs:label "minimumStorageHumidity"^^xsd:string ;
  rdfs:range "xsd:decimal"^^xsd:string .

<https://edi3.org/mmt/vocab#HaulageInstructions>
  a rdfs:Class ;
  rdfs:comment "Instructions related to the action or process of conveyance."^^xsd:string ;
  rdfs:label "HaulageInstructions"^^xsd:string .

<https://edi3.org/mmt/vocab#HaulageInstructionsDescription>
  a rdf:Property ;
  rdfs:comment "The textual description of these haulage instructions."^^xsd:string ;
  rdfs:domain "mmt:HaulageInstructions"^^xsd:string ;
  rdfs:label "description"^^xsd:string ;
  rdfs:range "xsd:string"^^xsd:string .

<https://edi3.org/mmt/vocab#HaulageInstructionsDescriptionCode>
  a rdf:Property ;
  rdfs:comment "The code specifying the description of these haulage instructions."^^xsd:string ;
  rdfs:domain "mmt:HaulageInstructions"^^xsd:string ;
  rdfs:label "descriptionCode"^^xsd:string ;
  rdfs:range "xsd:token"^^xsd:string .

<https://edi3.org/mmt/vocab#HeaderTradeAgreement>
  a rdfs:Class ;
  rdfs:comment "The contractual terms of a header trade agreement."^^xsd:string ;
  rdfs:label "HeaderTradeAgreement"^^xsd:string .

<https://edi3.org/mmt/vocab#HeaderTradeAgreementBuyerReferenceText>
  a rdf:Property ;
  rdfs:comment "A buyer reference, expressed as text, for this header trade agreement."^^xsd:string ;
  rdfs:domain "mmt:HeaderTradeAgreement"^^xsd:string ;
  rdfs:label "buyerReferenceText"^^xsd:string ;
  rdfs:range "xsd:string"^^xsd:string .

<https://edi3.org/mmt/vocab#HeaderTradeAgreementDeliveryPriorityCode>
  a rdf:Property ;
  rdfs:comment "The code specifying the delivery priority for this header trade agreement."^^xsd:string ;
  rdfs:domain "mmt:HeaderTradeAgreement"^^xsd:string ;
  rdfs:label "deliveryPriorityCode"^^xsd:string ;
  rdfs:range "PriorityDescriptionType_Сode"^^xsd:string .

<https://edi3.org/mmt/vocab#HeaderTradeAgreementReferenceText>
  a rdf:Property ;
  rdfs:comment "A reference, expressed as text, for this header trade agreement."^^xsd:string ;
  rdfs:domain "mmt:HeaderTradeAgreement"^^xsd:string ;
  rdfs:label "referenceText"^^xsd:string ;
  rdfs:range "xsd:string"^^xsd:string .

<https://edi3.org/mmt/vocab#HeaderTradeDelivery>
  a rdfs:Class ;
  rdfs:comment "Shipping arrangements and movement of products and or services including despatch and delivery at a header level."^^xsd:string ;
  rdfs:label "HeaderTradeDelivery"^^xsd:string .

<https://edi3.org/mmt/vocab#HeaderTradeDeliveryAgreedQuantity>
  a rdf:Property ;
  rdfs:comment "The quantity, at header level, agreed for this trade delivery."^^xsd:string ;
  rdfs:domain "mmt:HeaderTradeDelivery"^^xsd:string ;
  rdfs:label "agreedQuantity"^^xsd:string ;
  rdfs:range "xsd:decimal"^^xsd:string .

<https://edi3.org/mmt/vocab#HeaderTradeDeliveryDespatchedQuantity>
  a rdf:Property ;
  rdfs:comment "The quantity, at header level, despatched in this trade delivery."^^xsd:string ;
  rdfs:domain "mmt:HeaderTradeDelivery"^^xsd:string ;
  rdfs:label "despatchedQuantity"^^xsd:string ;
  rdfs:range "xsd:decimal"^^xsd:string .

<https://edi3.org/mmt/vocab#HeaderTradeDeliveryFinalDeliveryIndicator>
  a rdf:Property ;
  rdfs:comment "The indication, at header level, of whether or not this trade delivery is the final delivery."^^xsd:string ;
  rdfs:domain "mmt:HeaderTradeDelivery"^^xsd:string ;
  rdfs:label "finalDeliveryIndicator"^^xsd:string ;
  rdfs:range "xsd:boolean"^^xsd:string .

<https://edi3.org/mmt/vocab#HeaderTradeDeliveryID>
  a rdf:Property ;
  rdfs:comment "The identifier, at header level, for this trade delivery."^^xsd:string ;
  rdfs:domain "mmt:HeaderTradeDelivery"^^xsd:string ;
  rdfs:label "iD"^^xsd:string ;
  rdfs:range "xsd:ID"^^xsd:string .

<https://edi3.org/mmt/vocab#HeaderTradeDeliveryPartialDeliveryAllowedIndicator>
  a rdf:Property ;
  rdfs:comment "The indication, at header level, of whether or not this trade delivery can be partially delivered."^^xsd:string ;
  rdfs:domain "mmt:HeaderTradeDelivery"^^xsd:string ;
  rdfs:label "partialDeliveryAllowedIndicator"^^xsd:string ;
  rdfs:range "xsd:boolean"^^xsd:string .

<https://edi3.org/mmt/vocab#HeaderTradeDeliveryPickUpAvailabilityDateTime>
  a rdf:Property ;
  rdfs:comment "The formatted date, time, date time, or other date time value, at header level, when this trade delivery is available for pick-up."^^xsd:string ;
  rdfs:domain "mmt:HeaderTradeDelivery"^^xsd:string ;
  rdfs:label "pickUpAvailabilityDateTime"^^xsd:string ;
  rdfs:range "xsd:datetime"^^xsd:string .

<https://edi3.org/mmt/vocab#HeaderTradeDeliveryRemainingRequestedQuantity>
  a rdf:Property ;
  rdfs:comment "The remaining quantity, at header level, requested for this trade delivery."^^xsd:string ;
  rdfs:domain "mmt:HeaderTradeDelivery"^^xsd:string ;
  rdfs:label "remainingRequestedQuantity"^^xsd:string ;
  rdfs:range "xsd:decimal"^^xsd:string .

<https://edi3.org/mmt/vocab#HeaderTradeDeliveryRequestedQuantity>
  a rdf:Property ;
  rdfs:comment "The quantity, at header level, requested for this trade delivery."^^xsd:string ;
  rdfs:domain "mmt:HeaderTradeDelivery"^^xsd:string ;
  rdfs:label "requestedQuantity"^^xsd:string ;
  rdfs:range "xsd:decimal"^^xsd:string .

<https://edi3.org/mmt/vocab#HeaderTradeSettlement>
  a rdfs:Class ;
  rdfs:comment "The information, at a header level, that enables the reconciliation of a financial transaction, with the item(s) that the financial transaction is intended to settle, such as a commercial invoice."^^xsd:string ;
  rdfs:label "HeaderTradeSettlement"^^xsd:string .

<https://edi3.org/mmt/vocab#HeaderTradeSettlementCreditReasonCode>
  a rdf:Property ;
  rdfs:comment "The code specifying the reason for a credit being given in this header trade settlement."^^xsd:string ;
  rdfs:domain "mmt:HeaderTradeSettlement"^^xsd:string ;
  rdfs:label "creditReasonCode"^^xsd:string ;
  rdfs:range "xsd:token"^^xsd:string .

<https://edi3.org/mmt/vocab#HeaderTradeSettlementCreditReasonText>
  a rdf:Property ;
  rdfs:comment "A textual description of the reason for a credit being given in this header trade settlement."^^xsd:string ;
  rdfs:domain "mmt:HeaderTradeSettlement"^^xsd:string ;
  rdfs:label "creditReasonText"^^xsd:string ;
  rdfs:range "xsd:string"^^xsd:string .

<https://edi3.org/mmt/vocab#HeaderTradeSettlementDuePayableAmount>
  a rdf:Property ;
  rdfs:comment "A monetary value that is an exact amount due and payable for this header trade settlement, such as the amount due to the creditor."^^xsd:string ;
  rdfs:domain "mmt:HeaderTradeSettlement"^^xsd:string ;
  rdfs:label "duePayableAmount"^^xsd:string ;
  rdfs:range "http://schema.org/amount"^^xsd:string .

<https://edi3.org/mmt/vocab#HeaderTradeSettlementInvoiceCurrencyCode>
  a rdf:Property ;
  rdfs:comment "The code specifying the invoice currency for this header trade settlement."^^xsd:string ;
  rdfs:domain "mmt:HeaderTradeSettlement"^^xsd:string ;
  rdfs:label "invoiceCurrencyCode"^^xsd:string ;
  rdfs:range "ISO4217_Code"^^xsd:string .

<https://edi3.org/mmt/vocab#HeaderTradeSettlementInvoiceDateTime>
  a rdf:Property ;
  rdfs:comment "The date, time, date time or other date time value of the invoice in this header trade settlement."^^xsd:string ;
  rdfs:domain "mmt:HeaderTradeSettlement"^^xsd:string ;
  rdfs:label "invoiceDateTime"^^xsd:string ;
  rdfs:range "xsd:datetime"^^xsd:string .

<https://edi3.org/mmt/vocab#HeaderTradeSettlementInvoiceIssuerReferenceText>
  a rdf:Property ;
  rdfs:comment "The invoice issuer reference, expressed as text, for this header trade settlement."^^xsd:string ;
  rdfs:domain "mmt:HeaderTradeSettlement"^^xsd:string ;
  rdfs:label "invoiceIssuerReferenceText"^^xsd:string ;
  rdfs:range "xsd:string"^^xsd:string .

<https://edi3.org/mmt/vocab#HeaderTradeSettlementNextInvoiceDateTime>
  a rdf:Property ;
  rdfs:comment "A date, time, date time or other date time value of a next invoice or invoices in this header trade settlement."^^xsd:string ;
  rdfs:domain "mmt:HeaderTradeSettlement"^^xsd:string ;
  rdfs:label "nextInvoiceDateTime"^^xsd:string ;
  rdfs:range "xsd:datetime"^^xsd:string .

<https://edi3.org/mmt/vocab#HeaderTradeSettlementPriceCurrencyCode>
  a rdf:Property ;
  rdfs:comment "The code specifying the price currency for this header trade settlement."^^xsd:string ;
  rdfs:domain "mmt:HeaderTradeSettlement"^^xsd:string ;
  rdfs:label "priceCurrencyCode"^^xsd:string ;
  rdfs:range "ISO4217_Code"^^xsd:string .

<https://edi3.org/mmt/vocab#HeaderTradeSettlementTaxCurrencyCode>
  a rdf:Property ;
  rdfs:comment "The code specifying the tax currency for this header trade settlement."^^xsd:string ;
  rdfs:domain "mmt:HeaderTradeSettlement"^^xsd:string ;
  rdfs:label "taxCurrencyCode"^^xsd:string ;
  rdfs:range "ISO4217_Code"^^xsd:string .

<https://edi3.org/mmt/vocab#IdentifiedFault>
  a rdfs:Class ;
  rdfs:comment "An identified defect or fault."^^xsd:string ;
  rdfs:label "IdentifiedFault"^^xsd:string .

<https://edi3.org/mmt/vocab#IdentifiedFaultDescription>
  a rdf:Property ;
  rdfs:comment "A textual description of this identified fault."^^xsd:string ;
  rdfs:domain "mmt:IdentifiedFault"^^xsd:string ;
  rdfs:label "description"^^xsd:string ;
  rdfs:range "xsd:string"^^xsd:string .

<https://edi3.org/mmt/vocab#IdentifiedFaultIDCode>
  a rdf:Property ;
  rdfs:comment "A code specifying an identified fault."^^xsd:string ;
  rdfs:domain "mmt:IdentifiedFault"^^xsd:string ;
  rdfs:label "iDCode"^^xsd:string ;
  rdfs:range "xsd:token"^^xsd:string .

<https://edi3.org/mmt/vocab#InstructedTemperature>
  a rdfs:Class ;
  rdfs:comment "Temperature settings instructed for storage or movement of goods."^^xsd:string ;
  rdfs:label "InstructedTemperature"^^xsd:string .

<https://edi3.org/mmt/vocab#InstructedTemperatureMaximumValue>
  a rdf:Property ;
  rdfs:comment "The measure of the maximum value of this instructed temperature."^^xsd:string ;
  rdfs:domain "mmt:InstructedTemperature"^^xsd:string ;
  rdfs:label "maximumValue"^^xsd:string ;
  rdfs:range "xsd:decimal"^^xsd:string .

<https://edi3.org/mmt/vocab#InstructedTemperatureMinimumValue>
  a rdf:Property ;
  rdfs:comment "The measure of the minimum value of this instructed temperature."^^xsd:string ;
  rdfs:domain "mmt:InstructedTemperature"^^xsd:string ;
  rdfs:label "minimumValue"^^xsd:string ;
  rdfs:range "xsd:decimal"^^xsd:string .

<https://edi3.org/mmt/vocab#LegalOrganization>
  a rdfs:Class ;
  rdfs:comment "An organization set up on a legal basis as a business, government body, department, charity, or financial institution."^^xsd:string ;
  rdfs:label "LegalOrganization"^^xsd:string .

<https://edi3.org/mmt/vocab#LegalOrganizationBusinessTypeCode>
  a rdf:Property ;
  rdfs:comment "A code specifying the type of business of this legally set up organization."^^xsd:string ;
  rdfs:domain "mmt:LegalOrganization"^^xsd:string ;
  rdfs:label "businessTypeCode"^^xsd:string ;
  rdfs:range "xsd:token"^^xsd:string .

<https://edi3.org/mmt/vocab#LegalOrganizationEstablishedDateTime>
  a rdf:Property ;
  rdfs:comment "The date, time, date time, or other date time value when this legally set up organization was established."^^xsd:string ;
  rdfs:domain "mmt:LegalOrganization"^^xsd:string ;
  rdfs:label "establishedDateTime"^^xsd:string ;
  rdfs:range "xsd:datetime"^^xsd:string .

<https://edi3.org/mmt/vocab#LegalOrganizationID>
  a rdf:Property ;
  rdfs:comment "A unique identifier for this legally set up organization."^^xsd:string ;
  rdfs:domain "mmt:LegalOrganization"^^xsd:string ;
  rdfs:label "iD"^^xsd:string ;
  rdfs:range "xsd:ID"^^xsd:string .

<https://edi3.org/mmt/vocab#LegalOrganizationLegalClassificationCode>
  a rdf:Property ;
  rdfs:comment "The code specifying the legal classification of this organization, such as Incorporated (Inc), Limited Liability Corporation (LLC) or non-profit."^^xsd:string ;
  rdfs:domain "mmt:LegalOrganization"^^xsd:string ;
  rdfs:label "legalClassificationCode"^^xsd:string ;
  rdfs:range "xsd:token"^^xsd:string .

<https://edi3.org/mmt/vocab#LegalOrganizationName>
  a rdf:Property ;
  rdfs:comment "A name, expressed as text, of this legally set up organization."^^xsd:string ;
  rdfs:domain "mmt:LegalOrganization"^^xsd:string ;
  rdfs:label "name"^^xsd:string ;
  rdfs:range "xsd:string"^^xsd:string .

<https://edi3.org/mmt/vocab#LegalOrganizationTradingName>
  a rdf:Property ;
  rdfs:comment "The trading business name, expressed as text, of this legally set up organization."^^xsd:string ;
  rdfs:domain "mmt:LegalOrganization"^^xsd:string ;
  rdfs:label "tradingName"^^xsd:string ;
  rdfs:range "xsd:string"^^xsd:string .

<https://edi3.org/mmt/vocab#LegalOrganizationTypeCode>
  a rdf:Property ;
  rdfs:comment "A code specifying a type of legally set up organization."^^xsd:string ;
  rdfs:domain "mmt:LegalOrganization"^^xsd:string ;
  rdfs:label "typeCode"^^xsd:string ;
  rdfs:range "xsd:token"^^xsd:string .

<https://edi3.org/mmt/vocab#LegalRegistration>
  a rdfs:Class ;
  rdfs:comment "The recording of items or details for a specific legal purpose."^^xsd:string ;
  rdfs:label "LegalRegistration"^^xsd:string .

<https://edi3.org/mmt/vocab#LegalRegistrationCountryCode>
  a rdf:Property ;
  rdfs:comment "An identifier of the country in which this legal registration is valid."^^xsd:string ;
  rdfs:domain "mmt:LegalRegistration"^^xsd:string ;
  rdfs:label "countryCode"^^xsd:string ;
  rdfs:range "xsd:ID"^^xsd:string .

<https://edi3.org/mmt/vocab#LegalRegistrationID>
  a rdf:Property ;
  rdfs:comment "A unique identifier for this legal registration."^^xsd:string ;
  rdfs:domain "mmt:LegalRegistration"^^xsd:string ;
  rdfs:label "iD"^^xsd:string ;
  rdfs:range "xsd:ID"^^xsd:string .

<https://edi3.org/mmt/vocab#LegalRegistrationLastRegisteredYear>
  a rdf:Property ;
  rdfs:comment "The last year in which this legal registration was registered."^^xsd:string ;
  rdfs:domain "mmt:LegalRegistration"^^xsd:string ;
  rdfs:label "lastRegisteredYear"^^xsd:string ;
  rdfs:range "xsd:datetime"^^xsd:string .

<https://edi3.org/mmt/vocab#LegalRegistrationTypeCode>
  a rdf:Property ;
  rdfs:comment "A code specifying the type of this legal registration."^^xsd:string ;
  rdfs:domain "mmt:LegalRegistration"^^xsd:string ;
  rdfs:label "typeCode"^^xsd:string ;
  rdfs:range "xsd:token"^^xsd:string .

<https://edi3.org/mmt/vocab#LineTradeAgreement>
  a rdfs:Class ;
  rdfs:comment "The contractual terms of a line trade agreement."^^xsd:string ;
  rdfs:label "LineTradeAgreement"^^xsd:string .

<https://edi3.org/mmt/vocab#LineTradeDelivery>
  a rdfs:Class ;
  rdfs:comment "Shipping arrangements and movement of products and or services including despatch and delivery at a line level."^^xsd:string ;
  rdfs:label "LineTradeDelivery"^^xsd:string .

<https://edi3.org/mmt/vocab#LineTradeDeliveryDespatchedQuantity>
  a rdf:Property ;
  rdfs:comment "The quantity, at line level, despatched for this trade delivery."^^xsd:string ;
  rdfs:domain "mmt:LineTradeDelivery"^^xsd:string ;
  rdfs:label "despatchedQuantity"^^xsd:string ;
  rdfs:range "xsd:decimal"^^xsd:string .

<https://edi3.org/mmt/vocab#LineTradeDeliveryGrossVolume>
  a rdf:Property ;
  rdfs:comment "The measure, at line level, of the gross volume of this trade delivery."^^xsd:string ;
  rdfs:domain "mmt:LineTradeDelivery"^^xsd:string ;
  rdfs:label "grossVolume"^^xsd:string ;
  rdfs:range "xsd:decimal"^^xsd:string .

<https://edi3.org/mmt/vocab#LineTradeDeliveryGrossWeight>
  a rdf:Property ;
  rdfs:comment "The measure, at line level, of the gross weight (mass) of this line trade delivery."^^xsd:string ;
  rdfs:domain "mmt:LineTradeDelivery"^^xsd:string ;
  rdfs:label "grossWeight"^^xsd:string ;
  rdfs:range "xsd:decimal"^^xsd:string .

<https://edi3.org/mmt/vocab#LineTradeDeliveryNetWeight>
  a rdf:Property ;
  rdfs:comment "The measure, at line level, of the net weight (mass) of this trade delivery."^^xsd:string ;
  rdfs:domain "mmt:LineTradeDelivery"^^xsd:string ;
  rdfs:label "netWeight"^^xsd:string ;
  rdfs:range "xsd:decimal"^^xsd:string .

<https://edi3.org/mmt/vocab#LineTradeDeliveryPackageQuantity>
  a rdf:Property ;
  rdfs:comment "The number of packages, at line level, in this trade delivery."^^xsd:string ;
  rdfs:domain "mmt:LineTradeDelivery"^^xsd:string ;
  rdfs:label "packageQuantity"^^xsd:string ;
  rdfs:range "xsd:decimal"^^xsd:string .

<https://edi3.org/mmt/vocab#LineTradeDeliveryUltimateShipToDeliveryDateTime>
  a rdf:Property ;
  rdfs:comment "The formatted date, time, date time, or other date time value, at line level, when this trade delivery is delivered to the ultimate ship to party."^^xsd:string ;
  rdfs:domain "mmt:LineTradeDelivery"^^xsd:string ;
  rdfs:label "ultimateShipToDeliveryDateTime"^^xsd:string ;
  rdfs:range "xsd:datetime"^^xsd:string .

<https://edi3.org/mmt/vocab#LineTradeSettlement>
  a rdfs:Class ;
  rdfs:comment "The information, at a line level, that enables the reconciliation of a financial transaction with the item(s) that the financial transaction is intended to settle, for example a commercial invoice."^^xsd:string ;
  rdfs:label "LineTradeSettlement"^^xsd:string .

<https://edi3.org/mmt/vocab#LocationParty>
  a rdfs:Class ;
  rdfs:comment "An individual, a group, or a body having a role related to a location."^^xsd:string ;
  rdfs:label "LocationParty"^^xsd:string .

<https://edi3.org/mmt/vocab#LocationPartyCountryCode>
  a rdf:Property ;
  rdfs:comment "A unique country identifier for this location party."^^xsd:string ;
  rdfs:domain "mmt:LocationParty"^^xsd:string ;
  rdfs:label "countryCode"^^xsd:string ;
  rdfs:range "xsd:ID"^^xsd:string .

<https://edi3.org/mmt/vocab#LocationPartyID>
  a rdf:Property ;
  rdfs:comment "A unique identifier of this location party."^^xsd:string ;
  rdfs:domain "mmt:LocationParty"^^xsd:string ;
  rdfs:label "iD"^^xsd:string ;
  rdfs:range "xsd:ID"^^xsd:string .

<https://edi3.org/mmt/vocab#LocationPartyName>
  a rdf:Property ;
  rdfs:comment "A name, expressed as text, for this location party."^^xsd:string ;
  rdfs:domain "mmt:LocationParty"^^xsd:string ;
  rdfs:label "name"^^xsd:string ;
  rdfs:range "xsd:string"^^xsd:string .

<https://edi3.org/mmt/vocab#LocationPartyRoleCode>
  a rdf:Property ;
  rdfs:comment "A code specifying a role of this location party."^^xsd:string ;
  rdfs:domain "mmt:LocationParty"^^xsd:string ;
  rdfs:label "roleCode"^^xsd:string ;
  rdfs:range "xsd:token"^^xsd:string .

<https://edi3.org/mmt/vocab#LogisticsConvoy>
  a rdfs:Class ;
  rdfs:comment "A number of means of transport following each other with a common logistics purpose."^^xsd:string ;
  rdfs:label "LogisticsConvoy"^^xsd:string .

<https://edi3.org/mmt/vocab#LogisticsConvoyMaximumWidth>
  a rdf:Property ;
  rdfs:comment "The maximum width measure for this logistics convoy."^^xsd:string ;
  rdfs:domain "mmt:LogisticsConvoy"^^xsd:string ;
  rdfs:label "maximumWidth"^^xsd:string ;
  rdfs:range "xsd:decimal"^^xsd:string .

<https://edi3.org/mmt/vocab#LogisticsConvoyNumberOfTransportMeans>
  a rdf:Property ;
  rdfs:comment "The number of means of transport in this logistics convoy."^^xsd:string ;
  rdfs:domain "mmt:LogisticsConvoy"^^xsd:string ;
  rdfs:label "numberOfTransportMeans"^^xsd:string ;
  rdfs:range "xsd:decimal"^^xsd:string .

<https://edi3.org/mmt/vocab#LogisticsConvoyOverallLength>
  a rdf:Property ;
  rdfs:comment "The overall length measure of this logistics convoy."^^xsd:string ;
  rdfs:domain "mmt:LogisticsConvoy"^^xsd:string ;
  rdfs:label "overallLength"^^xsd:string ;
  rdfs:range "xsd:decimal"^^xsd:string .

<https://edi3.org/mmt/vocab#LogisticsLabel>
  a rdfs:Class ;
  rdfs:comment "A label used for identifying goods for logistics purposes, such as a barcode, a radio frequency tag or a Vehicle Identification Number (VIN)."^^xsd:string ;
  rdfs:label "LogisticsLabel"^^xsd:string .

<https://edi3.org/mmt/vocab#LogisticsLabelID>
  a rdf:Property ;
  rdfs:comment "The unique identifier of this logistics label."^^xsd:string ;
  rdfs:domain "mmt:LogisticsLabel"^^xsd:string ;
  rdfs:label "iD"^^xsd:string ;
  rdfs:range "xsd:ID"^^xsd:string .

<https://edi3.org/mmt/vocab#LogisticsLabelSeriesEndID>
  a rdf:Property ;
  rdfs:comment "The unique identifier of the end of a series of logistics labels."^^xsd:string ;
  rdfs:domain "mmt:LogisticsLabel"^^xsd:string ;
  rdfs:label "seriesEndID"^^xsd:string ;
  rdfs:range "xsd:ID"^^xsd:string .

<https://edi3.org/mmt/vocab#LogisticsLabelSeriesStartID>
  a rdf:Property ;
  rdfs:comment "The unique identifier of the start of a series of logistics labels."^^xsd:string ;
  rdfs:domain "mmt:LogisticsLabel"^^xsd:string ;
  rdfs:label "seriesStartID"^^xsd:string ;
  rdfs:range "xsd:ID"^^xsd:string .

<https://edi3.org/mmt/vocab#LogisticsLocation>
  a rdfs:Class ;
  rdfs:comment "A logistics related physical location or place."^^xsd:string ;
  rdfs:label "LogisticsLocation"^^xsd:string .

<https://edi3.org/mmt/vocab#LogisticsLocationCountryCode>
  a rdf:Property ;
  rdfs:comment "The unique identifier of a country for this logistics location."^^xsd:string ;
  rdfs:domain "mmt:LogisticsLocation"^^xsd:string ;
  rdfs:label "countryCode"^^xsd:string ;
  rdfs:range "ISO3166_Code"^^xsd:string .

<https://edi3.org/mmt/vocab#LogisticsLocationCountryName>
  a rdf:Property ;
  rdfs:comment "The country name, expressed as text, of this logistics location."^^xsd:string ;
  rdfs:domain "mmt:LogisticsLocation"^^xsd:string ;
  rdfs:label "countryName"^^xsd:string ;
  rdfs:range "xsd:string"^^xsd:string .

<https://edi3.org/mmt/vocab#LogisticsLocationDescription>
  a rdf:Property ;
  rdfs:comment "A textual description of this logistics related location."^^xsd:string ;
  rdfs:domain "mmt:LogisticsLocation"^^xsd:string ;
  rdfs:label "description"^^xsd:string ;
  rdfs:range "xsd:string"^^xsd:string .

<https://edi3.org/mmt/vocab#LogisticsLocationID>
  a rdf:Property ;
  rdfs:comment "A unique identifier for this logistics related location, such as a United Nations Location Code (UNLOCODE) or GS1 Global Location Number (GLN)."^^xsd:string ;
  rdfs:domain "mmt:LogisticsLocation"^^xsd:string ;
  rdfs:label "iD"^^xsd:string ;
  rdfs:range "xsd:ID"^^xsd:string .

<https://edi3.org/mmt/vocab#LogisticsLocationName>
  a rdf:Property ;
  rdfs:comment "A name, expressed as text, of this logistics related location."^^xsd:string ;
  rdfs:domain "mmt:LogisticsLocation"^^xsd:string ;
  rdfs:label "name"^^xsd:string ;
  rdfs:range "xsd:string"^^xsd:string .

<https://edi3.org/mmt/vocab#LogisticsLocationTypeCode>
  a rdf:Property ;
  rdfs:comment "A code specifying the type of this logistics related location."^^xsd:string ;
  rdfs:domain "mmt:LogisticsLocation"^^xsd:string ;
  rdfs:label "typeCode"^^xsd:string ;
  rdfs:range "LocationFunctionType_Сode"^^xsd:string .

<https://edi3.org/mmt/vocab#LogisticsPackage>
  a rdfs:Class ;
  rdfs:comment "A self-contained wrapping or container within which goods can be contained for logistics purposes, such as a box or a barrel which can be filled, partially filled or empty."^^xsd:string ;
  rdfs:label "LogisticsPackage"^^xsd:string .

<https://edi3.org/mmt/vocab#LogisticsPackageGrossVolume>
  a rdf:Property ;
  rdfs:comment "The measure of the gross volume of this logistics package."^^xsd:string ;
  rdfs:domain "mmt:LogisticsPackage"^^xsd:string ;
  rdfs:label "grossVolume"^^xsd:string ;
  rdfs:range "xsd:decimal"^^xsd:string .

<https://edi3.org/mmt/vocab#LogisticsPackageGrossWeight>
  a rdf:Property ;
  rdfs:comment "The measure of the gross weight (mass) of this logistics package and its contents."^^xsd:string ;
  rdfs:domain "mmt:LogisticsPackage"^^xsd:string ;
  rdfs:label "grossWeight"^^xsd:string ;
  rdfs:range "xsd:decimal"^^xsd:string .

<https://edi3.org/mmt/vocab#LogisticsPackageID>
  a rdf:Property ;
  rdfs:comment "The unique identifier for this logistics package."^^xsd:string ;
  rdfs:domain "mmt:LogisticsPackage"^^xsd:string ;
  rdfs:label "iD"^^xsd:string ;
  rdfs:range "xsd:ID"^^xsd:string .

<https://edi3.org/mmt/vocab#LogisticsPackageItemQuantity>
  a rdf:Property ;
  rdfs:comment "The number of logistics packages at this level."^^xsd:string ;
  rdfs:domain "mmt:LogisticsPackage"^^xsd:string ;
  rdfs:label "itemQuantity"^^xsd:string ;
  rdfs:range "xsd:decimal"^^xsd:string .

<https://edi3.org/mmt/vocab#LogisticsPackageLevelCode>
  a rdf:Property ;
  rdfs:comment "The code specifying the level of this logistics package."^^xsd:string ;
  rdfs:domain "mmt:LogisticsPackage"^^xsd:string ;
  rdfs:label "levelCode"^^xsd:string ;
  rdfs:range "PackagingLevelType_Сode"^^xsd:string .

<https://edi3.org/mmt/vocab#LogisticsPackageNetWeight>
  a rdf:Property ;
  rdfs:comment "The measure of the net weight of this logistics package, i.e. the weight (mass) of the contents."^^xsd:string ;
  rdfs:domain "mmt:LogisticsPackage"^^xsd:string ;
  rdfs:label "netWeight"^^xsd:string ;
  rdfs:range "xsd:decimal"^^xsd:string .

<https://edi3.org/mmt/vocab#LogisticsPackageReturnableIndicator>
  a rdf:Property ;
  rdfs:comment "The indication of whether or not this logistics package is returnable."^^xsd:string ;
  rdfs:domain "mmt:LogisticsPackage"^^xsd:string ;
  rdfs:label "returnableIndicator"^^xsd:string ;
  rdfs:range "xsd:boolean"^^xsd:string .

<https://edi3.org/mmt/vocab#LogisticsPackageSequenceNumber>
  a rdf:Property ;
  rdfs:comment "The sequence number of this logistics package."^^xsd:string ;
  rdfs:domain "mmt:LogisticsPackage"^^xsd:string ;
  rdfs:label "sequenceNumber"^^xsd:string ;
  rdfs:range "xsd:decimal"^^xsd:string .

<https://edi3.org/mmt/vocab#LogisticsPackageSeriesEndID>
  a rdf:Property ;
  rdfs:comment "The unique identifier of the end of a series of packages within this logistics package."^^xsd:string ;
  rdfs:domain "mmt:LogisticsPackage"^^xsd:string ;
  rdfs:label "seriesEndID"^^xsd:string ;
  rdfs:range "xsd:ID"^^xsd:string .

<https://edi3.org/mmt/vocab#LogisticsPackageSeriesStartID>
  a rdf:Property ;
  rdfs:comment "The unique start identifier of a series of packages within this logistics package."^^xsd:string ;
  rdfs:domain "mmt:LogisticsPackage"^^xsd:string ;
  rdfs:label "seriesStartID"^^xsd:string ;
  rdfs:range "xsd:ID"^^xsd:string .

<https://edi3.org/mmt/vocab#LogisticsPackageTypeCode>
  a rdf:Property ;
  rdfs:comment "The code specifying the type of logistics package."^^xsd:string ;
  rdfs:domain "mmt:LogisticsPackage"^^xsd:string ;
  rdfs:label "typeCode"^^xsd:string ;
  rdfs:range "PackageType_Сode"^^xsd:string .

<https://edi3.org/mmt/vocab#LogisticsPackageTypeText>
  a rdf:Property ;
  rdfs:comment "The type, expressed as text, of this logistics package."^^xsd:string ;
  rdfs:domain "mmt:LogisticsPackage"^^xsd:string ;
  rdfs:label "typeText"^^xsd:string ;
  rdfs:range "xsd:string"^^xsd:string .

<https://edi3.org/mmt/vocab#LogisticsRegulatedGoods>
  a rdfs:Class ;
  rdfs:comment "Articles of trade or commerce which are subject to, or controlled by a rule, regulation, or law at a particular point during their logistics lifecycle."^^xsd:string ;
  rdfs:label "LogisticsRegulatedGoods"^^xsd:string .

<https://edi3.org/mmt/vocab#LogisticsSeal>
  a rdfs:Class ;
  rdfs:comment "A device used to secure an object and protect it from unauthorized entry or tampering during transport or other logistics operations."^^xsd:string ;
  rdfs:label "LogisticsSeal"^^xsd:string .

<https://edi3.org/mmt/vocab#LogisticsSealConditionCode>
  a rdf:Property ;
  rdfs:comment "A code specifying a condition of this logistics seal."^^xsd:string ;
  rdfs:domain "mmt:LogisticsSeal"^^xsd:string ;
  rdfs:label "conditionCode"^^xsd:string ;
  rdfs:range "SealConditionType_Сode"^^xsd:string .

<https://edi3.org/mmt/vocab#LogisticsSealID>
  a rdf:Property ;
  rdfs:comment "A unique identifier for this logistics seal."^^xsd:string ;
  rdfs:domain "mmt:LogisticsSeal"^^xsd:string ;
  rdfs:label "iD"^^xsd:string ;
  rdfs:range "xsd:ID"^^xsd:string .

<https://edi3.org/mmt/vocab#LogisticsSealSealingPartyRoleCode>
  a rdf:Property ;
  rdfs:comment "The code specifying the role of the party responsible for the sealing of this logistics seal."^^xsd:string ;
  rdfs:domain "mmt:LogisticsSeal"^^xsd:string ;
  rdfs:label "sealingPartyRoleCode"^^xsd:string ;
  rdfs:range "SealingPartyRoleType_Сode"^^xsd:string .

<https://edi3.org/mmt/vocab#LogisticsSealTypeCode>
  a rdf:Property ;
  rdfs:comment "The code specifying the type of logistics seal."^^xsd:string ;
  rdfs:domain "mmt:LogisticsSeal"^^xsd:string ;
  rdfs:label "typeCode"^^xsd:string ;
  rdfs:range "SealType_Сode"^^xsd:string .

<https://edi3.org/mmt/vocab#LogisticsServiceCharge>
  a rdfs:Class ;
  rdfs:comment "A charge made for a logistics related service."^^xsd:string ;
  rdfs:label "LogisticsServiceCharge"^^xsd:string .

<https://edi3.org/mmt/vocab#LogisticsServiceChargeAppliedAmount>
  a rdf:Property ;
  rdfs:comment "A monetary value applied to this logistics service charge."^^xsd:string ;
  rdfs:domain "mmt:LogisticsServiceCharge"^^xsd:string ;
  rdfs:label "appliedAmount"^^xsd:string ;
  rdfs:range "http://schema.org/amount"^^xsd:string .

<https://edi3.org/mmt/vocab#LogisticsServiceChargeCalculationBasisCode>
  a rdf:Property ;
  rdfs:comment "The code specifying a basis on which this logistics service charge is to be calculated, such as by volume or per unit."^^xsd:string ;
  rdfs:domain "mmt:LogisticsServiceCharge"^^xsd:string ;
  rdfs:label "calculationBasisCode"^^xsd:string ;
  rdfs:range "FreightChargeQuantityUnitBasisType_Сode"^^xsd:string .

<https://edi3.org/mmt/vocab#LogisticsServiceChargeCategoryCode>
  a rdf:Property ;
  rdfs:comment "The code specifying the category of this logistics service charge [Reference United Nations Code List (UNCL) 5237]."^^xsd:string ;
  rdfs:domain "mmt:LogisticsServiceCharge"^^xsd:string ;
  rdfs:label "categoryCode"^^xsd:string ;
  rdfs:range "TransportServiceCategoryType_Сode"^^xsd:string .

<https://edi3.org/mmt/vocab#LogisticsServiceChargeChargeCategoryCode>
  a rdf:Property ;
  rdfs:comment "The code specifying the category of charge for this logistics service charge."^^xsd:string ;
  rdfs:domain "mmt:LogisticsServiceCharge"^^xsd:string ;
  rdfs:label "chargeCategoryCode"^^xsd:string ;
  rdfs:range "xsd:token"^^xsd:string .

<https://edi3.org/mmt/vocab#LogisticsServiceChargeDescription>
  a rdf:Property ;
  rdfs:comment "A textual description of this logistics service charge."^^xsd:string ;
  rdfs:domain "mmt:LogisticsServiceCharge"^^xsd:string ;
  rdfs:label "description"^^xsd:string ;
  rdfs:range "xsd:string"^^xsd:string .

<https://edi3.org/mmt/vocab#LogisticsServiceChargeDisbursementAmount>
  a rdf:Property ;
  rdfs:comment "A monetary value of a disbursement for this logistics service charge."^^xsd:string ;
  rdfs:domain "mmt:LogisticsServiceCharge"^^xsd:string ;
  rdfs:label "disbursementAmount"^^xsd:string ;
  rdfs:range "http://schema.org/amount"^^xsd:string .

<https://edi3.org/mmt/vocab#LogisticsServiceChargeFreightInvoiceTypeCode>
  a rdf:Property ;
  rdfs:comment "A code specifying a type of freight invoice of this logistics service charge."^^xsd:string ;
  rdfs:domain "mmt:LogisticsServiceCharge"^^xsd:string ;
  rdfs:label "freightInvoiceTypeCode"^^xsd:string ;
  rdfs:range "xsd:token"^^xsd:string .

<https://edi3.org/mmt/vocab#LogisticsServiceChargeID>
  a rdf:Property ;
  rdfs:comment "The unique identifier for this logistics service charge."^^xsd:string ;
  rdfs:domain "mmt:LogisticsServiceCharge"^^xsd:string ;
  rdfs:label "iD"^^xsd:string ;
  rdfs:range "FreightCostType_Сode"^^xsd:string .

<https://edi3.org/mmt/vocab#LogisticsServiceChargePayingPartyRoleCode>
  a rdf:Property ;
  rdfs:comment "The code specifying the role of the party responsible for paying this logistics service charge."^^xsd:string ;
  rdfs:domain "mmt:LogisticsServiceCharge"^^xsd:string ;
  rdfs:label "payingPartyRoleCode"^^xsd:string ;
  rdfs:range "xsd:token"^^xsd:string .

<https://edi3.org/mmt/vocab#LogisticsServiceChargePaymentArrangementCode>
  a rdf:Property ;
  rdfs:comment "The code specifying the payment arrangement for this logistics service charge [Reference United Nations Code List (UNCL) 4237]."^^xsd:string ;
  rdfs:domain "mmt:LogisticsServiceCharge"^^xsd:string ;
  rdfs:label "paymentArrangementCode"^^xsd:string ;
  rdfs:range "TransportPaymentArrangementType_Сode"^^xsd:string .

<https://edi3.org/mmt/vocab#LogisticsServiceChargeServiceCategoryCode>
  a rdf:Property ;
  rdfs:comment "The code specifying the category of service for this logistics service charge."^^xsd:string ;
  rdfs:domain "mmt:LogisticsServiceCharge"^^xsd:string ;
  rdfs:label "serviceCategoryCode"^^xsd:string ;
  rdfs:range "xsd:token"^^xsd:string .

<https://edi3.org/mmt/vocab#LogisticsServiceChargeTariffClassCode>
  a rdf:Property ;
  rdfs:comment "The code specifying the tariff class for this logistics service charge which represents an entry in a table of fixed charges [Reference United Nations Code List (UNCL) 5243]."^^xsd:string ;
  rdfs:domain "mmt:LogisticsServiceCharge"^^xsd:string ;
  rdfs:label "tariffClassCode"^^xsd:string ;
  rdfs:range "FreightChargeTariffType_Сode"^^xsd:string .

<https://edi3.org/mmt/vocab#LogisticsServiceChargeTransportPaymentMethodCode>
  a rdf:Property ;
  rdfs:comment "The code specifying the transport payment method for this logistics service charge."^^xsd:string ;
  rdfs:domain "mmt:LogisticsServiceCharge"^^xsd:string ;
  rdfs:label "transportPaymentMethodCode"^^xsd:string ;
  rdfs:range "xsd:token"^^xsd:string .

<https://edi3.org/mmt/vocab#LogisticsShippingMarks>
  a rdfs:Class ;
  rdfs:comment "Physical markings or labels on individual packages or transport units for logistics purposes."^^xsd:string ;
  rdfs:label "LogisticsShippingMarks"^^xsd:string .

<https://edi3.org/mmt/vocab#LogisticsShippingMarksMarkingInstructionCode>
  a rdf:Property ;
  rdfs:comment "A code specifying a marking instruction for these logistics shipping marks."^^xsd:string ;
  rdfs:domain "mmt:LogisticsShippingMarks"^^xsd:string ;
  rdfs:label "markingInstructionCode"^^xsd:string ;
  rdfs:range "MarkingInstructionType_Сode"^^xsd:string .

<https://edi3.org/mmt/vocab#LogisticsShippingMarksMarkingText>
  a rdf:Property ;
  rdfs:comment "Marking, expressed as text, for these logistics shipping marks."^^xsd:string ;
  rdfs:domain "mmt:LogisticsShippingMarks"^^xsd:string ;
  rdfs:label "markingText"^^xsd:string ;
  rdfs:range "xsd:string"^^xsd:string .

<https://edi3.org/mmt/vocab#LogisticsStatus>
  a rdfs:Class ;
  rdfs:comment "The information relevant to a condition or a position related to logistics."^^xsd:string ;
  rdfs:label "LogisticsStatus"^^xsd:string .

<https://edi3.org/mmt/vocab#LogisticsStatusConditionCode>
  a rdf:Property ;
  rdfs:comment "The code specifying this logistics status condition [UNECE Recommendation 24]."^^xsd:string ;
  rdfs:domain "mmt:LogisticsStatus"^^xsd:string ;
  rdfs:label "conditionCode"^^xsd:string ;
  rdfs:range "TransportStatusType_Сode"^^xsd:string .

<https://edi3.org/mmt/vocab#LogisticsStatusDescription>
  a rdf:Property ;
  rdfs:comment "The textual description of this logistics status."^^xsd:string ;
  rdfs:domain "mmt:LogisticsStatus"^^xsd:string ;
  rdfs:label "description"^^xsd:string ;
  rdfs:range "xsd:string"^^xsd:string .

<https://edi3.org/mmt/vocab#LogisticsStatusReasonCode>
  a rdf:Property ;
  rdfs:comment "A code specifying a reason for this logistics status [UNECE Recommendation 24]."^^xsd:string ;
  rdfs:domain "mmt:LogisticsStatus"^^xsd:string ;
  rdfs:label "reasonCode"^^xsd:string ;
  rdfs:range "TransportStatusType_Сode"^^xsd:string .

<https://edi3.org/mmt/vocab#LogisticsStatusReasonText>
  a rdf:Property ;
  rdfs:comment "A reason, expressed as text, for this logistics status."^^xsd:string ;
  rdfs:domain "mmt:LogisticsStatus"^^xsd:string ;
  rdfs:label "reasonText"^^xsd:string ;
  rdfs:range "xsd:string"^^xsd:string .

<https://edi3.org/mmt/vocab#LogisticsStatusReferenceDateTime>
  a rdf:Property ;
  rdfs:comment "The reference date, time, date time or other date time value for this logistics status."^^xsd:string ;
  rdfs:domain "mmt:LogisticsStatus"^^xsd:string ;
  rdfs:label "referenceDateTime"^^xsd:string ;
  rdfs:range "xsd:datetime"^^xsd:string .

<https://edi3.org/mmt/vocab#LogisticsStatusSequenceNumber>
  a rdf:Property ;
  rdfs:comment "The sequence number of this logistics status, such as within a status report."^^xsd:string ;
  rdfs:domain "mmt:LogisticsStatus"^^xsd:string ;
  rdfs:label "sequenceNumber"^^xsd:string ;
  rdfs:range "xsd:decimal"^^xsd:string .

<https://edi3.org/mmt/vocab#LogisticsTransportEquipment>
  a rdfs:Class ;
  rdfs:comment "A piece of equipment used to hold, protect or secure cargo for logistics purposes."^^xsd:string ;
  rdfs:label "LogisticsTransportEquipment"^^xsd:string .

<https://edi3.org/mmt/vocab#LogisticsTransportEquipmentAccompaniedIndicator>
  a rdf:Property ;
  rdfs:comment "The indication of whether or not this piece of logistics transport equipment is accompanied, such as by a transport means."^^xsd:string ;
  rdfs:domain "mmt:LogisticsTransportEquipment"^^xsd:string ;
  rdfs:label "accompaniedIndicator"^^xsd:string ;
  rdfs:range "xsd:boolean"^^xsd:string .

<https://edi3.org/mmt/vocab#LogisticsTransportEquipmentAirFlowMeasure>
  a rdf:Property ;
  rdfs:comment "The measure of the air flow for this piece of logistics transport equipment."^^xsd:string ;
  rdfs:domain "mmt:LogisticsTransportEquipment"^^xsd:string ;
  rdfs:label "airFlowMeasure"^^xsd:string ;
  rdfs:range "xsd:decimal"^^xsd:string .

<https://edi3.org/mmt/vocab#LogisticsTransportEquipmentCarrierAssignedBookingID>
  a rdf:Property ;
  rdfs:comment "A carrier assigned booking identifier for this piece of logistics transport equipment."^^xsd:string ;
  rdfs:domain "mmt:LogisticsTransportEquipment"^^xsd:string ;
  rdfs:label "carrierAssignedBookingID"^^xsd:string ;
  rdfs:range "xsd:ID"^^xsd:string .

<https://edi3.org/mmt/vocab#LogisticsTransportEquipmentCategoryCode>
  a rdf:Property ;
  rdfs:comment "The code specifying the category for this piece of logistics transport equipment, such as container or trailer."^^xsd:string ;
  rdfs:domain "mmt:LogisticsTransportEquipment"^^xsd:string ;
  rdfs:label "categoryCode"^^xsd:string ;
  rdfs:range "TransportEquipmentCategoryType_Сode"^^xsd:string .

<https://edi3.org/mmt/vocab#LogisticsTransportEquipmentCharacteristicText>
  a rdf:Property ;
  rdfs:comment "The characteristic or characteristics, expressed as text, of a piece of logistics transport equipment, such as its size and type."^^xsd:string ;
  rdfs:domain "mmt:LogisticsTransportEquipment"^^xsd:string ;
  rdfs:label "characteristicText"^^xsd:string ;
  rdfs:range "xsd:string"^^xsd:string .

<https://edi3.org/mmt/vocab#LogisticsTransportEquipmentContainedConsignmentQuantity>
  a rdf:Property ;
  rdfs:comment "The number of consignments contained in this piece of logistics transport equipment."^^xsd:string ;
  rdfs:domain "mmt:LogisticsTransportEquipment"^^xsd:string ;
  rdfs:label "containedConsignmentQuantity"^^xsd:string ;
  rdfs:range "xsd:decimal"^^xsd:string .

<https://edi3.org/mmt/vocab#LogisticsTransportEquipmentDamageRemark>
  a rdf:Property ;
  rdfs:comment "A damage remark, expressed as text, for this piece of logistics transport equipment."^^xsd:string ;
  rdfs:domain "mmt:LogisticsTransportEquipment"^^xsd:string ;
  rdfs:label "damageRemark"^^xsd:string ;
  rdfs:range "xsd:string"^^xsd:string .

<https://edi3.org/mmt/vocab#LogisticsTransportEquipmentFullEmptyCode>
  a rdf:Property ;
  rdfs:comment "The code specifying the used capacity of this piece of logistics transport equipment, such as full or empty."^^xsd:string ;
  rdfs:domain "mmt:LogisticsTransportEquipment"^^xsd:string ;
  rdfs:label "fullEmptyCode"^^xsd:string ;
  rdfs:range "TransportEquipmentFullnessType_Сode"^^xsd:string .

<https://edi3.org/mmt/vocab#LogisticsTransportEquipmentGrossVolume>
  a rdf:Property ;
  rdfs:comment "The measure of the gross volume of this piece of logistics transport equipment."^^xsd:string ;
  rdfs:domain "mmt:LogisticsTransportEquipment"^^xsd:string ;
  rdfs:label "grossVolume"^^xsd:string ;
  rdfs:range "xsd:decimal"^^xsd:string .

<https://edi3.org/mmt/vocab#LogisticsTransportEquipmentGrossWeight>
  a rdf:Property ;
  rdfs:comment "The measure of the gross weight (mass) of this piece of logistics transport equipment which is the weight (mass) including loaded goods, packing and transport equipment."^^xsd:string ;
  rdfs:domain "mmt:LogisticsTransportEquipment"^^xsd:string ;
  rdfs:label "grossWeight"^^xsd:string ;
  rdfs:range "xsd:decimal"^^xsd:string .

<https://edi3.org/mmt/vocab#LogisticsTransportEquipmentHaulageArrangementCode>
  a rdf:Property ;
  rdfs:comment "The code specifying the arrangement for the haulage of this piece of logistics transport equipment."^^xsd:string ;
  rdfs:domain "mmt:LogisticsTransportEquipment"^^xsd:string ;
  rdfs:label "haulageArrangementCode"^^xsd:string ;
  rdfs:range "TransportEquipmentHaulageArrangementsType_Сode"^^xsd:string .

<https://edi3.org/mmt/vocab#LogisticsTransportEquipmentHumidityPercent>
  a rdf:Property ;
  rdfs:comment "The percent of the humidity (moisture content) within this piece of logistics transport equipment."^^xsd:string ;
  rdfs:domain "mmt:LogisticsTransportEquipment"^^xsd:string ;
  rdfs:label "humidityPercent"^^xsd:string ;
  rdfs:range "xsd:decimal"^^xsd:string .

<https://edi3.org/mmt/vocab#LogisticsTransportEquipmentID>
  a rdf:Property ;
  rdfs:comment "The unique identifier of this piece of logistics transport equipment."^^xsd:string ;
  rdfs:domain "mmt:LogisticsTransportEquipment"^^xsd:string ;
  rdfs:label "iD"^^xsd:string ;
  rdfs:range "xsd:ID"^^xsd:string .

<https://edi3.org/mmt/vocab#LogisticsTransportEquipmentInformation>
  a rdf:Property ;
  rdfs:comment "Information, expressed as text, for this piece of logistics transport equipment."^^xsd:string ;
  rdfs:domain "mmt:LogisticsTransportEquipment"^^xsd:string ;
  rdfs:label "information"^^xsd:string ;
  rdfs:range "xsd:string"^^xsd:string .

<https://edi3.org/mmt/vocab#LogisticsTransportEquipmentLegalStatusCode>
  a rdf:Property ;
  rdfs:comment "The code specifying the legal status of this piece of logistics transport equipment with respect to a specific law such as the \"Container Convention Code\"."^^xsd:string ;
  rdfs:domain "mmt:LogisticsTransportEquipment"^^xsd:string ;
  rdfs:label "legalStatusCode"^^xsd:string ;
  rdfs:range "TransportEquipmentMovementLegalStatusType_Сode"^^xsd:string .

<https://edi3.org/mmt/vocab#LogisticsTransportEquipmentLoadedPackageQuantity>
  a rdf:Property ;
  rdfs:comment "The number of packages loaded into or onto this piece of logistics transport equipment."^^xsd:string ;
  rdfs:domain "mmt:LogisticsTransportEquipment"^^xsd:string ;
  rdfs:label "loadedPackageQuantity"^^xsd:string ;
  rdfs:range "xsd:decimal"^^xsd:string .

<https://edi3.org/mmt/vocab#LogisticsTransportEquipmentLoadingLength>
  a rdf:Property ;
  rdfs:comment "The measure of the loading length of this piece of logistics transport equipment."^^xsd:string ;
  rdfs:domain "mmt:LogisticsTransportEquipment"^^xsd:string ;
  rdfs:label "loadingLength"^^xsd:string ;
  rdfs:range "xsd:decimal"^^xsd:string .

<https://edi3.org/mmt/vocab#LogisticsTransportEquipmentLoadingRemark>
  a rdf:Property ;
  rdfs:comment "A loading remark, expressed as text, for this piece of logistics transport equipment."^^xsd:string ;
  rdfs:domain "mmt:LogisticsTransportEquipment"^^xsd:string ;
  rdfs:label "loadingRemark"^^xsd:string ;
  rdfs:range "xsd:string"^^xsd:string .

<https://edi3.org/mmt/vocab#LogisticsTransportEquipmentLoadingSequenceNumber>
  a rdf:Property ;
  rdfs:comment "The sequence number differentiating this piece of logistics transport equipment from others during loading."^^xsd:string ;
  rdfs:domain "mmt:LogisticsTransportEquipment"^^xsd:string ;
  rdfs:label "loadingSequenceNumber"^^xsd:string ;
  rdfs:range "xsd:decimal"^^xsd:string .

<https://edi3.org/mmt/vocab#LogisticsTransportEquipmentNetWeight>
  a rdf:Property ;
  rdfs:comment "The measure of the net weight (mass) of this piece of logistics transport equipment."^^xsd:string ;
  rdfs:domain "mmt:LogisticsTransportEquipment"^^xsd:string ;
  rdfs:label "netWeight"^^xsd:string ;
  rdfs:range "xsd:decimal"^^xsd:string .

<https://edi3.org/mmt/vocab#LogisticsTransportEquipmentOperationalStatusCode>
  a rdf:Property ;
  rdfs:comment "The code specifying the operational status for this piece of logistics transport equipment, such as to be repaired or to be shifted."^^xsd:string ;
  rdfs:domain "mmt:LogisticsTransportEquipment"^^xsd:string ;
  rdfs:label "operationalStatusCode"^^xsd:string ;
  rdfs:range "TransportEquipmentOperationalStatusType_Сode"^^xsd:string .

<https://edi3.org/mmt/vocab#LogisticsTransportEquipmentPowerSupplyConnectorQuantity>
  a rdf:Property ;
  rdfs:comment "The number of power supply connectors for this piece of logistics transport equipment."^^xsd:string ;
  rdfs:domain "mmt:LogisticsTransportEquipment"^^xsd:string ;
  rdfs:label "powerSupplyConnectorQuantity"^^xsd:string ;
  rdfs:range "xsd:decimal"^^xsd:string .

<https://edi3.org/mmt/vocab#LogisticsTransportEquipmentPowerSupplyTypeCode>
  a rdf:Property ;
  rdfs:comment "The code specifying the type of power supply for this piece of logistics transport equipment, such as diesel fuel or electricity."^^xsd:string ;
  rdfs:domain "mmt:LogisticsTransportEquipment"^^xsd:string ;
  rdfs:label "powerSupplyTypeCode"^^xsd:string ;
  rdfs:range "xsd:token"^^xsd:string .

<https://edi3.org/mmt/vocab#LogisticsTransportEquipmentPowerSupplyTypeText>
  a rdf:Property ;
  rdfs:comment "The type of power supply, expressed as text, for this piece of logistics transport equipment, such as diesel fuel or electricity."^^xsd:string ;
  rdfs:domain "mmt:LogisticsTransportEquipment"^^xsd:string ;
  rdfs:label "powerSupplyTypeText"^^xsd:string ;
  rdfs:range "xsd:string"^^xsd:string .

<https://edi3.org/mmt/vocab#LogisticsTransportEquipmentReleaseID>
  a rdf:Property ;
  rdfs:comment "The release identifier for this piece of logistics transport equipment."^^xsd:string ;
  rdfs:domain "mmt:LogisticsTransportEquipment"^^xsd:string ;
  rdfs:label "releaseID"^^xsd:string ;
  rdfs:range "xsd:ID"^^xsd:string .

<https://edi3.org/mmt/vocab#LogisticsTransportEquipmentReleaseRestrictionText>
  a rdf:Property ;
  rdfs:comment "The release restriction, expressed as text, for this piece of logistics transport equipment."^^xsd:string ;
  rdfs:domain "mmt:LogisticsTransportEquipment"^^xsd:string ;
  rdfs:label "releaseRestrictionText"^^xsd:string ;
  rdfs:range "xsd:string"^^xsd:string .

<https://edi3.org/mmt/vocab#LogisticsTransportEquipmentRequiredLaneLength>
  a rdf:Property ;
  rdfs:comment "The measure of the length required in a lane for this piece of logistics transport equipment."^^xsd:string ;
  rdfs:domain "mmt:LogisticsTransportEquipment"^^xsd:string ;
  rdfs:label "requiredLaneLength"^^xsd:string ;
  rdfs:range "xsd:decimal"^^xsd:string .

<https://edi3.org/mmt/vocab#LogisticsTransportEquipmentReturnableIndicator>
  a rdf:Property ;
  rdfs:comment "The indication of whether or not this piece of logistics transport equipment is returnable."^^xsd:string ;
  rdfs:domain "mmt:LogisticsTransportEquipment"^^xsd:string ;
  rdfs:label "returnableIndicator"^^xsd:string ;
  rdfs:range "xsd:boolean"^^xsd:string .

<https://edi3.org/mmt/vocab#LogisticsTransportEquipmentSealQuantity>
  a rdf:Property ;
  rdfs:comment "The quantity of seals for this piece of logistics transport equipment."^^xsd:string ;
  rdfs:domain "mmt:LogisticsTransportEquipment"^^xsd:string ;
  rdfs:label "sealQuantity"^^xsd:string ;
  rdfs:range "xsd:decimal"^^xsd:string .

<https://edi3.org/mmt/vocab#LogisticsTransportEquipmentSealedIndicator>
  a rdf:Property ;
  rdfs:comment "The indication of whether or not this piece of logistics transport equipment is sealed."^^xsd:string ;
  rdfs:domain "mmt:LogisticsTransportEquipment"^^xsd:string ;
  rdfs:label "sealedIndicator"^^xsd:string ;
  rdfs:range "xsd:boolean"^^xsd:string .

<https://edi3.org/mmt/vocab#LogisticsTransportEquipmentSequenceNumber>
  a rdf:Property ;
  rdfs:comment "The sequence number differentiating this piece of logistics transport equipment from others in a set of transport equipment."^^xsd:string ;
  rdfs:domain "mmt:LogisticsTransportEquipment"^^xsd:string ;
  rdfs:label "sequenceNumber"^^xsd:string ;
  rdfs:range "xsd:decimal"^^xsd:string .

<https://edi3.org/mmt/vocab#LogisticsTransportEquipmentSizeTypeCode>
  a rdf:Property ;
  rdfs:comment "The code specifying the characteristic or characteristics of this piece of logistics transport equipment, such as the ISO 6346 transport equipment size and type code."^^xsd:string ;
  rdfs:domain "mmt:LogisticsTransportEquipment"^^xsd:string ;
  rdfs:label "sizeTypeCode"^^xsd:string ;
  rdfs:range "EquipmentSizeTypeDescriptionType_Сode"^^xsd:string .

<https://edi3.org/mmt/vocab#LogisticsTransportEquipmentSupplierPartyRoleCode>
  a rdf:Property ;
  rdfs:comment "The code specifying the role of the party responsible for supplying this piece of logistics transport equipment, such as the carrier or the buyer."^^xsd:string ;
  rdfs:domain "mmt:LogisticsTransportEquipment"^^xsd:string ;
  rdfs:label "supplierPartyRoleCode"^^xsd:string ;
  rdfs:range "EquipmentSupplierType_Сode"^^xsd:string .

<https://edi3.org/mmt/vocab#LogisticsTransportEquipmentTareWeight>
  a rdf:Property ;
  rdfs:comment "The measure of the tare weight (mass) of this piece of logistics transport equipment which is the weight (mass) including permanent equipment but excluding goods and loose accessories."^^xsd:string ;
  rdfs:domain "mmt:LogisticsTransportEquipment"^^xsd:string ;
  rdfs:label "tareWeight"^^xsd:string ;
  rdfs:range "xsd:decimal"^^xsd:string .

<https://edi3.org/mmt/vocab#LogisticsTransportEquipmentTransportMovementStatusCode>
  a rdf:Property ;
  rdfs:comment "The code specifying the transport movement status for this piece of logistics transport equipment, such as for export, for import, or for transhipment."^^xsd:string ;
  rdfs:domain "mmt:LogisticsTransportEquipment"^^xsd:string ;
  rdfs:label "transportMovementStatusCode"^^xsd:string ;
  rdfs:range "TransportEquipmentMovementStatusType_Сode"^^xsd:string .

<https://edi3.org/mmt/vocab#LogisticsTransportEquipmentUnitQuantity>
  a rdf:Property ;
  rdfs:comment "The number of units of this type of logistics transport equipment."^^xsd:string ;
  rdfs:domain "mmt:LogisticsTransportEquipment"^^xsd:string ;
  rdfs:label "unitQuantity"^^xsd:string ;
  rdfs:range "xsd:decimal"^^xsd:string .

<https://edi3.org/mmt/vocab#LogisticsTransportEquipmentUnloadingSequenceNumber>
  a rdf:Property ;
  rdfs:comment "The sequence number differentiating this piece of logistics transport equipment from others during unloading."^^xsd:string ;
  rdfs:domain "mmt:LogisticsTransportEquipment"^^xsd:string ;
  rdfs:label "unloadingSequenceNumber"^^xsd:string ;
  rdfs:range "xsd:decimal"^^xsd:string .

<https://edi3.org/mmt/vocab#LogisticsTransportMeans>
  a rdfs:Class ;
  rdfs:comment "The devices used to convey goods or other objects from place to place during logistics cargo movements."^^xsd:string ;
  rdfs:label "LogisticsTransportMeans"^^xsd:string .

<https://edi3.org/mmt/vocab#LogisticsTransportMeansAftDraughtLevelMeasure>
  a rdf:Property ;
  rdfs:comment "The draught level measured at the aft end of this transport means."^^xsd:string ;
  rdfs:domain "mmt:LogisticsTransportMeans"^^xsd:string ;
  rdfs:label "aftDraughtLevelMeasure"^^xsd:string ;
  rdfs:range "xsd:decimal"^^xsd:string .

<https://edi3.org/mmt/vocab#LogisticsTransportMeansCargoGrossWeight>
  a rdf:Property ;
  rdfs:comment "The measure of the total gross weight (mass) of all cargo loaded onto this logistics means of transport, including packaging but excluding any associated transport equipment."^^xsd:string ;
  rdfs:domain "mmt:LogisticsTransportMeans"^^xsd:string ;
  rdfs:label "cargoGrossWeight"^^xsd:string ;
  rdfs:range "xsd:decimal"^^xsd:string .

<https://edi3.org/mmt/vocab#LogisticsTransportMeansConferenceCode>
  a rdf:Property ;
  rdfs:comment "The code specifying the conference for this logistics means of transport."^^xsd:string ;
  rdfs:domain "mmt:LogisticsTransportMeans"^^xsd:string ;
  rdfs:label "conferenceCode"^^xsd:string ;
  rdfs:range "xsd:token"^^xsd:string .

<https://edi3.org/mmt/vocab#LogisticsTransportMeansDraughtLevelMeasure>
  a rdf:Property ;
  rdfs:comment "The measure of the draught level of this logistics means of transport."^^xsd:string ;
  rdfs:domain "mmt:LogisticsTransportMeans"^^xsd:string ;
  rdfs:label "draughtLevelMeasure"^^xsd:string ;
  rdfs:range "xsd:decimal"^^xsd:string .

<https://edi3.org/mmt/vocab#LogisticsTransportMeansDriverAccompaniedIndicator>
  a rdf:Property ;
  rdfs:comment "The indication of whether or not this logistics means of transport is accompanied by a driver."^^xsd:string ;
  rdfs:domain "mmt:LogisticsTransportMeans"^^xsd:string ;
  rdfs:label "driverAccompaniedIndicator"^^xsd:string ;
  rdfs:range "xsd:boolean"^^xsd:string .

<https://edi3.org/mmt/vocab#LogisticsTransportMeansForwardDraughtLevelMeasure>
  a rdf:Property ;
  rdfs:comment "The draught level measured at the fore end of this transport means."^^xsd:string ;
  rdfs:domain "mmt:LogisticsTransportMeans"^^xsd:string ;
  rdfs:label "forwardDraughtLevelMeasure"^^xsd:string ;
  rdfs:range "xsd:decimal"^^xsd:string .

<https://edi3.org/mmt/vocab#LogisticsTransportMeansGrossWeight>
  a rdf:Property ;
  rdfs:comment "The measure of the gross weight (mass) of this logistics means of transport including cargo, such as the measure of the overall size of a vessel determined in accordance with the provisions of the International Convention on Tonnage Measurement of Ships, 1969."^^xsd:string ;
  rdfs:domain "mmt:LogisticsTransportMeans"^^xsd:string ;
  rdfs:label "grossWeight"^^xsd:string ;
  rdfs:range "xsd:decimal"^^xsd:string .

<https://edi3.org/mmt/vocab#LogisticsTransportMeansHelipadIndicator>
  a rdf:Property ;
  rdfs:comment "The indication of whether or not there is a helipad on this logistics means of transport."^^xsd:string ;
  rdfs:domain "mmt:LogisticsTransportMeans"^^xsd:string ;
  rdfs:label "helipadIndicator"^^xsd:string ;
  rdfs:range "xsd:boolean"^^xsd:string .

<https://edi3.org/mmt/vocab#LogisticsTransportMeansID>
  a rdf:Property ;
  rdfs:comment "An identifier of this logistics means of transport, such as the International Maritime Organization number of a vessel."^^xsd:string ;
  rdfs:domain "mmt:LogisticsTransportMeans"^^xsd:string ;
  rdfs:label "iD"^^xsd:string ;
  rdfs:range "xsd:ID"^^xsd:string .

<https://edi3.org/mmt/vocab#LogisticsTransportMeansISPSSecurityLevelCode>
  a rdf:Property ;
  rdfs:comment "The code specifying the International Ship and Port facility Security (ISPS) level assigned to this logistics means of transport."^^xsd:string ;
  rdfs:domain "mmt:LogisticsTransportMeans"^^xsd:string ;
  rdfs:label "iSPSSecurityLevelCode"^^xsd:string ;
  rdfs:range "xsd:token"^^xsd:string .

<https://edi3.org/mmt/vocab#LogisticsTransportMeansLength>
  a rdf:Property ;
  rdfs:comment "The measure of the length of this logistics means of transport."^^xsd:string ;
  rdfs:domain "mmt:LogisticsTransportMeans"^^xsd:string ;
  rdfs:label "length"^^xsd:string ;
  rdfs:range "xsd:decimal"^^xsd:string .

<https://edi3.org/mmt/vocab#LogisticsTransportMeansLoadedCargoMeasure>
  a rdf:Property ;
  rdfs:comment "The measure of the cargo loaded onto this logistics means of transport, such as the number of barrels of oil or other quantity of breakbulk cargo."^^xsd:string ;
  rdfs:domain "mmt:LogisticsTransportMeans"^^xsd:string ;
  rdfs:label "loadedCargoMeasure"^^xsd:string ;
  rdfs:range "xsd:decimal"^^xsd:string .

<https://edi3.org/mmt/vocab#LogisticsTransportMeansManoeuvringSpeed>
  a rdf:Property ;
  rdfs:comment "The manoeuvring speed measured for this logistics means of transport."^^xsd:string ;
  rdfs:domain "mmt:LogisticsTransportMeans"^^xsd:string ;
  rdfs:label "manoeuvringSpeed"^^xsd:string ;
  rdfs:range "xsd:decimal"^^xsd:string .

<https://edi3.org/mmt/vocab#LogisticsTransportMeansName>
  a rdf:Property ;
  rdfs:comment "The name, expressed as text, of this logistics means of transport."^^xsd:string ;
  rdfs:domain "mmt:LogisticsTransportMeans"^^xsd:string ;
  rdfs:label "name"^^xsd:string ;
  rdfs:range "xsd:string"^^xsd:string .

<https://edi3.org/mmt/vocab#LogisticsTransportMeansNetWeight>
  a rdf:Property ;
  rdfs:comment "The measure of the net weight (mass) of this logistics means of transport, such as the net tonnage of a vessel determined in accordance with the provisions of the International Convention on Tonnage Measurement of Ships, 1969."^^xsd:string ;
  rdfs:domain "mmt:LogisticsTransportMeans"^^xsd:string ;
  rdfs:label "netWeight"^^xsd:string ;
  rdfs:range "xsd:decimal"^^xsd:string .

<https://edi3.org/mmt/vocab#LogisticsTransportMeansRequiredLaneLength>
  a rdf:Property ;
  rdfs:comment "The measure of the external length required in a lane for this logistics transport means."^^xsd:string ;
  rdfs:domain "mmt:LogisticsTransportMeans"^^xsd:string ;
  rdfs:label "requiredLaneLength"^^xsd:string ;
  rdfs:range "xsd:decimal"^^xsd:string .

<https://edi3.org/mmt/vocab#LogisticsTransportMeansSequenceNumber>
  a rdf:Property ;
  rdfs:comment "The sequence number differentiating this logistics transport means from others."^^xsd:string ;
  rdfs:domain "mmt:LogisticsTransportMeans"^^xsd:string ;
  rdfs:label "sequenceNumber"^^xsd:string ;
  rdfs:range "xsd:decimal"^^xsd:string .

<https://edi3.org/mmt/vocab#LogisticsTransportMeansTypeCode>
  a rdf:Property ;
  rdfs:comment "The code specifying the type of logistics means of transport (Reference UNECE Recommendation 28)."^^xsd:string ;
  rdfs:domain "mmt:LogisticsTransportMeans"^^xsd:string ;
  rdfs:label "typeCode"^^xsd:string ;
  rdfs:range "TransportMeansType_Сode"^^xsd:string .

<https://edi3.org/mmt/vocab#LogisticsTransportMeansTypeText>
  a rdf:Property ;
  rdfs:comment "The type, expressed as text, of this logistics means of transport."^^xsd:string ;
  rdfs:domain "mmt:LogisticsTransportMeans"^^xsd:string ;
  rdfs:label "typeText"^^xsd:string ;
  rdfs:range "xsd:string"^^xsd:string .

<https://edi3.org/mmt/vocab#LogisticsTransportMeansWasteReportingExemptionIndicator>
  a rdf:Property ;
  rdfs:comment "The indication of whether or not there is a waste reporting exemption for this logistics means of transport."^^xsd:string ;
  rdfs:domain "mmt:LogisticsTransportMeans"^^xsd:string ;
  rdfs:label "wasteReportingExemptionIndicator"^^xsd:string ;
  rdfs:range "xsd:boolean"^^xsd:string .

<https://edi3.org/mmt/vocab#LogisticsTransportMovement>
  a rdfs:Class ;
  rdfs:comment "The conveyance (physical carriage) of goods or other objects used for logistics transport purposes."^^xsd:string ;
  rdfs:label "LogisticsTransportMovement"^^xsd:string .

<https://edi3.org/mmt/vocab#LogisticsTransportMovementBorderCrossingDateTime>
  a rdf:Property ;
  rdfs:comment "A date, time, date time or other date time value when this logistics transport movement crosses a border."^^xsd:string ;
  rdfs:domain "mmt:LogisticsTransportMovement"^^xsd:string ;
  rdfs:label "borderCrossingDateTime"^^xsd:string ;
  rdfs:range "xsd:datetime"^^xsd:string .

<https://edi3.org/mmt/vocab#LogisticsTransportMovementCargoDescription>
  a rdf:Property ;
  rdfs:comment "The textual description of the cargo for this logistics transport movement."^^xsd:string ;
  rdfs:domain "mmt:LogisticsTransportMovement"^^xsd:string ;
  rdfs:label "cargoDescription"^^xsd:string ;
  rdfs:range "xsd:string"^^xsd:string .

<https://edi3.org/mmt/vocab#LogisticsTransportMovementClosingDateTime>
  a rdf:Property ;
  rdfs:comment "The date, time, date time, or other date time value by which cargo should be loaded onto the means of transport for the departure of this logistics transport movement."^^xsd:string ;
  rdfs:domain "mmt:LogisticsTransportMovement"^^xsd:string ;
  rdfs:label "closingDateTime"^^xsd:string ;
  rdfs:range "xsd:datetime"^^xsd:string .

<https://edi3.org/mmt/vocab#LogisticsTransportMovementConsignmentQuantity>
  a rdf:Property ;
  rdfs:comment "The number of consignments in this logistics transport movement."^^xsd:string ;
  rdfs:domain "mmt:LogisticsTransportMovement"^^xsd:string ;
  rdfs:label "consignmentQuantity"^^xsd:string ;
  rdfs:range "xsd:decimal"^^xsd:string .

<https://edi3.org/mmt/vocab#LogisticsTransportMovementCrewQuantity>
  a rdf:Property ;
  rdfs:comment "The number of crew members for this logistics transport movement."^^xsd:string ;
  rdfs:domain "mmt:LogisticsTransportMovement"^^xsd:string ;
  rdfs:label "crewQuantity"^^xsd:string ;
  rdfs:range "xsd:decimal"^^xsd:string .

<https://edi3.org/mmt/vocab#LogisticsTransportMovementDangerousGoodsIndicator>
  a rdf:Property ;
  rdfs:comment "The indication of whether or not dangerous goods are carried for this logistics transport movement."^^xsd:string ;
  rdfs:domain "mmt:LogisticsTransportMovement"^^xsd:string ;
  rdfs:label "dangerousGoodsIndicator"^^xsd:string ;
  rdfs:range "xsd:boolean"^^xsd:string .

<https://edi3.org/mmt/vocab#LogisticsTransportMovementID>
  a rdf:Property ;
  rdfs:comment "The unique identifier for this logistics transport movement, such as a voyage number, flight number, or trip number."^^xsd:string ;
  rdfs:domain "mmt:LogisticsTransportMovement"^^xsd:string ;
  rdfs:label "iD"^^xsd:string ;
  rdfs:range "xsd:ID"^^xsd:string .

<https://edi3.org/mmt/vocab#LogisticsTransportMovementInformation>
  a rdf:Property ;
  rdfs:comment "Information, expressed as text, for this logistics transport movement."^^xsd:string ;
  rdfs:domain "mmt:LogisticsTransportMovement"^^xsd:string ;
  rdfs:label "information"^^xsd:string ;
  rdfs:range "xsd:string"^^xsd:string .

<https://edi3.org/mmt/vocab#LogisticsTransportMovementManifestOnboardIndicator>
  a rdf:Property ;
  rdfs:comment "The indication of whether or not the manifest for this logistics transport movement is onboard."^^xsd:string ;
  rdfs:domain "mmt:LogisticsTransportMovement"^^xsd:string ;
  rdfs:label "manifestOnboardIndicator"^^xsd:string ;
  rdfs:range "xsd:boolean"^^xsd:string .

<https://edi3.org/mmt/vocab#LogisticsTransportMovementModeCode>
  a rdf:Property ;
  rdfs:comment "The code specifying the mode, such as by air, sea, rail, road or inland waterway, for this logistics transport movement."^^xsd:string ;
  rdfs:domain "mmt:LogisticsTransportMovement"^^xsd:string ;
  rdfs:label "modeCode"^^xsd:string ;
  rdfs:range "TransportModeType_Сode"^^xsd:string .

<https://edi3.org/mmt/vocab#LogisticsTransportMovementModeText>
  a rdf:Property ;
  rdfs:comment "The mode, expressed as text, of this logistics transport movement."^^xsd:string ;
  rdfs:domain "mmt:LogisticsTransportMovement"^^xsd:string ;
  rdfs:label "modeText"^^xsd:string ;
  rdfs:range "xsd:string"^^xsd:string .

<https://edi3.org/mmt/vocab#LogisticsTransportMovementPackageQuantity>
  a rdf:Property ;
  rdfs:comment "The number of packages in this logistics transport movement."^^xsd:string ;
  rdfs:domain "mmt:LogisticsTransportMovement"^^xsd:string ;
  rdfs:label "packageQuantity"^^xsd:string ;
  rdfs:range "xsd:decimal"^^xsd:string .

<https://edi3.org/mmt/vocab#LogisticsTransportMovementPassengerQuantity>
  a rdf:Property ;
  rdfs:comment "The number of passengers for this logistics transport movement."^^xsd:string ;
  rdfs:domain "mmt:LogisticsTransportMovement"^^xsd:string ;
  rdfs:label "passengerQuantity"^^xsd:string ;
  rdfs:range "xsd:decimal"^^xsd:string .

<https://edi3.org/mmt/vocab#LogisticsTransportMovementPilotageExemptionID>
  a rdf:Property ;
  rdfs:comment "The identifier of a pilotage exemption for this logistics transport movement."^^xsd:string ;
  rdfs:domain "mmt:LogisticsTransportMovement"^^xsd:string ;
  rdfs:label "pilotageExemptionID"^^xsd:string ;
  rdfs:range "xsd:ID"^^xsd:string .

<https://edi3.org/mmt/vocab#LogisticsTransportMovementSailingAdviceNotificationInformation>
  a rdf:Property ;
  rdfs:comment "Sailing advice notification information, expressed as text, for this logistics transport movement."^^xsd:string ;
  rdfs:domain "mmt:LogisticsTransportMovement"^^xsd:string ;
  rdfs:label "sailingAdviceNotificationInformation"^^xsd:string ;
  rdfs:range "xsd:string"^^xsd:string .

<https://edi3.org/mmt/vocab#LogisticsTransportMovementScheduledID>
  a rdf:Property ;
  rdfs:comment "A unique identifier for this logistics transport movement, such as a voyage number, flight number, or trip number, as stated in a schedule."^^xsd:string ;
  rdfs:domain "mmt:LogisticsTransportMovement"^^xsd:string ;
  rdfs:label "scheduledID"^^xsd:string ;
  rdfs:range "xsd:ID"^^xsd:string .

<https://edi3.org/mmt/vocab#LogisticsTransportMovementStageCode>
  a rdf:Property ;
  rdfs:comment "The code specifying the stage of this logistics transport movement."^^xsd:string ;
  rdfs:domain "mmt:LogisticsTransportMovement"^^xsd:string ;
  rdfs:label "stageCode"^^xsd:string ;
  rdfs:range "TransportMovementStageType_Сode"^^xsd:string .

<https://edi3.org/mmt/vocab#LogisticsTransportMovementStatusCode>
  a rdf:Property ;
  rdfs:comment "The code specifying a status for the logistics transport movement, such as estimated or final."^^xsd:string ;
  rdfs:domain "mmt:LogisticsTransportMovement"^^xsd:string ;
  rdfs:label "statusCode"^^xsd:string ;
  rdfs:range "StatusType_Сode"^^xsd:string .

<https://edi3.org/mmt/vocab#LogisticsTransportMovementStayID>
  a rdf:Property ;
  rdfs:comment "The unique identifier of a stay in a port, airport or other place of service for this logistics transport movement."^^xsd:string ;
  rdfs:domain "mmt:LogisticsTransportMovement"^^xsd:string ;
  rdfs:label "stayID"^^xsd:string ;
  rdfs:range "xsd:ID"^^xsd:string .

<https://edi3.org/mmt/vocab#LogisticsTransportMovementTerminalOperatorAssignedID>
  a rdf:Property ;
  rdfs:comment "A unique identifier for this logistics transport movement as assigned by a terminal operator."^^xsd:string ;
  rdfs:domain "mmt:LogisticsTransportMovement"^^xsd:string ;
  rdfs:label "terminalOperatorAssignedID"^^xsd:string ;
  rdfs:range "xsd:ID"^^xsd:string .

<https://edi3.org/mmt/vocab#LogisticsTransportMovementTradedParcelQuantity>
  a rdf:Property ;
  rdfs:comment "The number of traded parcels of cargo being transported in this logistics transport movement."^^xsd:string ;
  rdfs:domain "mmt:LogisticsTransportMovement"^^xsd:string ;
  rdfs:label "tradedParcelQuantity"^^xsd:string ;
  rdfs:range "xsd:decimal"^^xsd:string .

<https://edi3.org/mmt/vocab#LogisticsTransportMovementTradingConsolidatorAssignedID>
  a rdf:Property ;
  rdfs:comment "The unique identifier for this logistics transport movement as assigned by the trading consolidator."^^xsd:string ;
  rdfs:domain "mmt:LogisticsTransportMovement"^^xsd:string ;
  rdfs:label "tradingConsolidatorAssignedID"^^xsd:string ;
  rdfs:range "xsd:ID"^^xsd:string .

<https://edi3.org/mmt/vocab#LogisticsTransportMovementTransitDirectionCode>
  a rdf:Property ;
  rdfs:comment "The code specifying the transit direction of this logistics transport movement."^^xsd:string ;
  rdfs:domain "mmt:LogisticsTransportMovement"^^xsd:string ;
  rdfs:label "transitDirectionCode"^^xsd:string ;
  rdfs:range "TransportMeansDirectionType_Сode"^^xsd:string .

<https://edi3.org/mmt/vocab#LogisticsTransportMovementTransportEquipmentQuantity>
  a rdf:Property ;
  rdfs:comment "The number of pieces of transport equipment for this logistics transport movement."^^xsd:string ;
  rdfs:domain "mmt:LogisticsTransportMovement"^^xsd:string ;
  rdfs:label "transportEquipmentQuantity"^^xsd:string ;
  rdfs:range "xsd:decimal"^^xsd:string .

<https://edi3.org/mmt/vocab#MaterialGoodsCharacteristic>
  a rdfs:Class ;
  rdfs:comment "A distinctive feature of a material contained within physical goods."^^xsd:string ;
  rdfs:label "MaterialGoodsCharacteristic"^^xsd:string .

<https://edi3.org/mmt/vocab#MaterialGoodsCharacteristicConstituentPercent>
  a rdf:Property ;
  rdfs:comment "The percentage presence of the material within the goods for this material goods characteristic."^^xsd:string ;
  rdfs:domain "mmt:MaterialGoodsCharacteristic"^^xsd:string ;
  rdfs:label "constituentPercent"^^xsd:string ;
  rdfs:range "xsd:decimal"^^xsd:string .

<https://edi3.org/mmt/vocab#MaterialGoodsCharacteristicDescription>
  a rdf:Property ;
  rdfs:comment "A textual description of this material goods characteristic."^^xsd:string ;
  rdfs:domain "mmt:MaterialGoodsCharacteristic"^^xsd:string ;
  rdfs:label "description"^^xsd:string ;
  rdfs:range "xsd:string"^^xsd:string .

<https://edi3.org/mmt/vocab#MaterialGoodsCharacteristicTypeCode>
  a rdf:Property ;
  rdfs:comment "The code specifying the type of material goods characteristic."^^xsd:string ;
  rdfs:domain "mmt:MaterialGoodsCharacteristic"^^xsd:string ;
  rdfs:label "typeCode"^^xsd:string ;
  rdfs:range "xsd:token"^^xsd:string .

<https://edi3.org/mmt/vocab#Measurement>
  a rdfs:Class ;
  rdfs:comment "An amount, size, or extent as established by measuring."^^xsd:string ;
  rdfs:label "Measurement"^^xsd:string .

<https://edi3.org/mmt/vocab#MeasurementActualMeasure>
  a rdf:Property ;
  rdfs:comment "An actual measure for this measurement."^^xsd:string ;
  rdfs:domain "mmt:Measurement"^^xsd:string ;
  rdfs:label "actualMeasure"^^xsd:string ;
  rdfs:range "xsd:decimal"^^xsd:string .

<https://edi3.org/mmt/vocab#MeasurementConditionMeasure>
  a rdf:Property ;
  rdfs:comment "A measure of a condition for this measurement."^^xsd:string ;
  rdfs:domain "mmt:Measurement"^^xsd:string ;
  rdfs:label "conditionMeasure"^^xsd:string ;
  rdfs:range "xsd:decimal"^^xsd:string .

<https://edi3.org/mmt/vocab#MeasurementMethodText>
  a rdf:Property ;
  rdfs:comment "A measurement method expressed as text."^^xsd:string ;
  rdfs:domain "mmt:Measurement"^^xsd:string ;
  rdfs:label "methodText"^^xsd:string ;
  rdfs:range "xsd:string"^^xsd:string .

<https://edi3.org/mmt/vocab#MeasurementTypeCode>
  a rdf:Property ;
  rdfs:comment "A code specifying a type of measurement."^^xsd:string ;
  rdfs:domain "mmt:Measurement"^^xsd:string ;
  rdfs:label "typeCode"^^xsd:string ;
  rdfs:range "xsd:token"^^xsd:string .

<https://edi3.org/mmt/vocab#Note>
  a rdfs:Class ;
  rdfs:comment "A textual or coded description, such as a remark or additional information."^^xsd:string ;
  rdfs:label "Note"^^xsd:string .

<https://edi3.org/mmt/vocab#NoteContentCode>
  a rdf:Property ;
  rdfs:comment "A code specifying the content of this note."^^xsd:string ;
  rdfs:domain "mmt:Note"^^xsd:string ;
  rdfs:label "contentCode"^^xsd:string ;
  rdfs:range "xsd:token"^^xsd:string .

<https://edi3.org/mmt/vocab#NoteContentText>
  a rdf:Property ;
  rdfs:comment "A content, expressed as text, of this note."^^xsd:string ;
  rdfs:domain "mmt:Note"^^xsd:string ;
  rdfs:label "contentText"^^xsd:string ;
  rdfs:range "xsd:string"^^xsd:string .

<https://edi3.org/mmt/vocab#NoteSubjectCode>
  a rdf:Property ;
  rdfs:comment "The code specifying the subject of this note."^^xsd:string ;
  rdfs:domain "mmt:Note"^^xsd:string ;
  rdfs:label "subjectCode"^^xsd:string ;
  rdfs:range "xsd:token"^^xsd:string .

<https://edi3.org/mmt/vocab#NoteSubjectText>
  a rdf:Property ;
  rdfs:comment "The subject, expressed as text, of this note."^^xsd:string ;
  rdfs:domain "mmt:Note"^^xsd:string ;
  rdfs:label "subjectText"^^xsd:string ;
  rdfs:range "xsd:string"^^xsd:string .

<https://edi3.org/mmt/vocab#ProductClassification>
  a rdfs:Class ;
  rdfs:comment "A systematic arrangement of products in classes or categories according to established criteria."^^xsd:string ;
  rdfs:label "ProductClassification"^^xsd:string .

<https://edi3.org/mmt/vocab#ProductClassificationClassCode>
  a rdf:Property ;
  rdfs:comment "The code specifying the class for this product classification."^^xsd:string ;
  rdfs:domain "mmt:ProductClassification"^^xsd:string ;
  rdfs:label "classCode"^^xsd:string ;
  rdfs:range "xsd:token"^^xsd:string .

<https://edi3.org/mmt/vocab#ProductClassificationClassName>
  a rdf:Property ;
  rdfs:comment "A class name, expressed as text, for this product classification."^^xsd:string ;
  rdfs:domain "mmt:ProductClassification"^^xsd:string ;
  rdfs:label "className"^^xsd:string ;
  rdfs:range "xsd:string"^^xsd:string .

<https://edi3.org/mmt/vocab#ProductClassificationSubClassCode>
  a rdf:Property ;
  rdfs:comment "The code specifying the sub class for this product classification."^^xsd:string ;
  rdfs:domain "mmt:ProductClassification"^^xsd:string ;
  rdfs:label "subClassCode"^^xsd:string ;
  rdfs:range "xsd:token"^^xsd:string .

<https://edi3.org/mmt/vocab#ProductClassificationSystemID>
  a rdf:Property ;
  rdfs:comment "The unique identifier of the classification system for this product classification."^^xsd:string ;
  rdfs:domain "mmt:ProductClassification"^^xsd:string ;
  rdfs:label "systemID"^^xsd:string ;
  rdfs:range "xsd:ID"^^xsd:string .

<https://edi3.org/mmt/vocab#ProductClassificationSystemName>
  a rdf:Property ;
  rdfs:comment "A name, expressed as text, of the classification system for this product classification."^^xsd:string ;
  rdfs:domain "mmt:ProductClassification"^^xsd:string ;
  rdfs:label "systemName"^^xsd:string ;
  rdfs:range "xsd:string"^^xsd:string .

<https://edi3.org/mmt/vocab#QuarantineInstructions>
  a rdfs:Class ;
  rdfs:comment "Instructions for a period of imposed isolation or detention."^^xsd:string ;
  rdfs:label "QuarantineInstructions"^^xsd:string .

<https://edi3.org/mmt/vocab#QuarantineInstructionsDescription>
  a rdf:Property ;
  rdfs:comment "The textual description of these quarantine instructions."^^xsd:string ;
  rdfs:domain "mmt:QuarantineInstructions"^^xsd:string ;
  rdfs:label "description"^^xsd:string ;
  rdfs:range "xsd:string"^^xsd:string .

<https://edi3.org/mmt/vocab#QuarantineInstructionsDescriptionCode>
  a rdf:Property ;
  rdfs:comment "The code specifying the description of these quarantine instructions."^^xsd:string ;
  rdfs:domain "mmt:QuarantineInstructions"^^xsd:string ;
  rdfs:label "descriptionCode"^^xsd:string ;
  rdfs:range "xsd:token"^^xsd:string .

<https://edi3.org/mmt/vocab#RadioactiveMaterial>
  a rdfs:Class ;
  rdfs:comment "Material capable of undergoing spontaneous nuclear decay involving emission of ionizing radiation in the form of particles or gamma rays."^^xsd:string ;
  rdfs:label "RadioactiveMaterial"^^xsd:string .

<https://edi3.org/mmt/vocab#RadioactiveMaterialCompositionDescription>
  a rdf:Property ;
  rdfs:comment "The textual description of the composition of this radioactive material."^^xsd:string ;
  rdfs:domain "mmt:RadioactiveMaterial"^^xsd:string ;
  rdfs:label "compositionDescription"^^xsd:string ;
  rdfs:range "xsd:string"^^xsd:string .

<https://edi3.org/mmt/vocab#RadioactiveMaterialCriticalitySafetyIndexNumber>
  a rdf:Property ;
  rdfs:comment "The criticality safety index number of this radioactive material."^^xsd:string ;
  rdfs:domain "mmt:RadioactiveMaterial"^^xsd:string ;
  rdfs:label "criticalitySafetyIndexNumber"^^xsd:string ;
  rdfs:range "xsd:decimal"^^xsd:string .

<https://edi3.org/mmt/vocab#RadioactiveMaterialFissileExceptionIndicator>
  a rdf:Property ;
  rdfs:comment "The indication of whether or not this radioactive material is a fissile exception."^^xsd:string ;
  rdfs:domain "mmt:RadioactiveMaterial"^^xsd:string ;
  rdfs:label "fissileExceptionIndicator"^^xsd:string ;
  rdfs:range "xsd:boolean"^^xsd:string .

<https://edi3.org/mmt/vocab#RadioactiveMaterialLowDispersibleInformation>
  a rdf:Property ;
  rdfs:comment "Information, expressed as text, describing the low dispersion properties of this radioactive material."^^xsd:string ;
  rdfs:domain "mmt:RadioactiveMaterial"^^xsd:string ;
  rdfs:label "lowDispersibleInformation"^^xsd:string ;
  rdfs:range "xsd:string"^^xsd:string .

<https://edi3.org/mmt/vocab#RadioactiveMaterialRadionuclideName>
  a rdf:Property ;
  rdfs:comment "The name of the radionuclide, expressed as text, of this radioactive material."^^xsd:string ;
  rdfs:domain "mmt:RadioactiveMaterial"^^xsd:string ;
  rdfs:label "radionuclideName"^^xsd:string ;
  rdfs:range "xsd:string"^^xsd:string .

<https://edi3.org/mmt/vocab#RadioactiveMaterialSpecialFormInformation>
  a rdf:Property ;
  rdfs:comment "Information, expressed as text, describing the special form for this radioactive material."^^xsd:string ;
  rdfs:domain "mmt:RadioactiveMaterial"^^xsd:string ;
  rdfs:label "specialFormInformation"^^xsd:string ;
  rdfs:range "xsd:string"^^xsd:string .

<https://edi3.org/mmt/vocab#RadioactiveMaterialTransportIndexNumber>
  a rdf:Property ;
  rdfs:comment "The transport index number of this radioactive material."^^xsd:string ;
  rdfs:domain "mmt:RadioactiveMaterial"^^xsd:string ;
  rdfs:label "transportIndexNumber"^^xsd:string ;
  rdfs:range "xsd:decimal"^^xsd:string .

<https://edi3.org/mmt/vocab#RadioactiveMaterialTypeCode>
  a rdf:Property ;
  rdfs:comment "The code specifying the type of this radioactive material."^^xsd:string ;
  rdfs:domain "mmt:RadioactiveMaterial"^^xsd:string ;
  rdfs:label "typeCode"^^xsd:string ;
  rdfs:range "xsd:token"^^xsd:string .

<https://edi3.org/mmt/vocab#ReferencedTransportService>
  a rdfs:Class ;
  rdfs:comment "A referenced service associated with a specified event during transport movement."^^xsd:string ;
  rdfs:label "ReferencedTransportService"^^xsd:string .

<https://edi3.org/mmt/vocab#ReferencedTransportServiceCategoryTypeCode>
  a rdf:Property ;
  rdfs:comment "A code specifying the category type of this referenced transport service."^^xsd:string ;
  rdfs:domain "mmt:ReferencedTransportService"^^xsd:string ;
  rdfs:label "categoryTypeCode"^^xsd:string ;
  rdfs:range "xsd:token"^^xsd:string .

<https://edi3.org/mmt/vocab#ReferencedTransportServiceContractID>
  a rdf:Property ;
  rdfs:comment "The contract identifier of this referenced transport service."^^xsd:string ;
  rdfs:domain "mmt:ReferencedTransportService"^^xsd:string ;
  rdfs:label "contractID"^^xsd:string ;
  rdfs:range "xsd:ID"^^xsd:string .

<https://edi3.org/mmt/vocab#ReferencedTransportServiceID>
  a rdf:Property ;
  rdfs:comment "An identifier of this referenced transport service."^^xsd:string ;
  rdfs:domain "mmt:ReferencedTransportService"^^xsd:string ;
  rdfs:label "iD"^^xsd:string ;
  rdfs:range "xsd:ID"^^xsd:string .

<https://edi3.org/mmt/vocab#ReferencedDocument>
  a rdfs:Class ;
  rdfs:comment "Written, printed or electronic matter that is referenced."^^xsd:string ;
  rdfs:label "ReferencedDocument"^^xsd:string .

<https://edi3.org/mmt/vocab#ReferencedDocumentAuthenticatedOriginalIndicator>
  a rdf:Property ;
  rdfs:comment "The indication of whether or not this referenced document is an authenticated original."^^xsd:string ;
  rdfs:domain "mmt:ReferencedDocument"^^xsd:string ;
  rdfs:label "authenticatedOriginalIndicator"^^xsd:string ;
  rdfs:range "xsd:boolean"^^xsd:string .

<https://edi3.org/mmt/vocab#ReferencedDocumentCategoryCode>
  a rdf:Property ;
  rdfs:comment "The code specifying the category of this referenced document."^^xsd:string ;
  rdfs:domain "mmt:ReferencedDocument"^^xsd:string ;
  rdfs:label "categoryCode"^^xsd:string ;
  rdfs:range "xsd:token"^^xsd:string .

<https://edi3.org/mmt/vocab#ReferencedDocumentElectronicPresentationIndicator>
  a rdf:Property ;
  rdfs:comment "The indication of whether or not this referenced document is presented in an electronic format."^^xsd:string ;
  rdfs:domain "mmt:ReferencedDocument"^^xsd:string ;
  rdfs:label "electronicPresentationIndicator"^^xsd:string ;
  rdfs:range "xsd:boolean"^^xsd:string .

<https://edi3.org/mmt/vocab#ReferencedDocumentFormattedIssueDateTime>
  a rdf:Property ;
  rdfs:comment "The formatted date or date time for the issuance of this referenced document."^^xsd:string ;
  rdfs:domain "mmt:ReferencedDocument"^^xsd:string ;
  rdfs:label "formattedIssueDateTime"^^xsd:string ;
  rdfs:range "xsd:datetime"^^xsd:string .

<https://edi3.org/mmt/vocab#ReferencedDocumentID>
  a rdf:Property ;
  rdfs:comment "A unique identifier for this referenced document."^^xsd:string ;
  rdfs:domain "mmt:ReferencedDocument"^^xsd:string ;
  rdfs:label "iD"^^xsd:string ;
  rdfs:range "xsd:ID"^^xsd:string .

<https://edi3.org/mmt/vocab#ReferencedDocumentLanguageCode>
  a rdf:Property ;
  rdfs:comment "An identifier for a language used in this referenced document."^^xsd:string ;
  rdfs:domain "mmt:ReferencedDocument"^^xsd:string ;
  rdfs:label "languageCode"^^xsd:string ;
  rdfs:range "ISO639_Code"^^xsd:string .

<https://edi3.org/mmt/vocab#ReferencedDocumentReferenceTypeCode>
  a rdf:Property ;
  rdfs:comment "The code specifying the reference type of this referenced document."^^xsd:string ;
  rdfs:domain "mmt:ReferencedDocument"^^xsd:string ;
  rdfs:label "referenceTypeCode"^^xsd:string ;
  rdfs:range "ReferenceType_Сode"^^xsd:string .

<https://edi3.org/mmt/vocab#ReferencedDocumentRemark>
  a rdf:Property ;
  rdfs:comment "A remark, expressed as text, regarding this referenced document."^^xsd:string ;
  rdfs:domain "mmt:ReferencedDocument"^^xsd:string ;
  rdfs:label "remark"^^xsd:string ;
  rdfs:range "xsd:string"^^xsd:string .

<https://edi3.org/mmt/vocab#ReferencedDocumentStatusCode>
  a rdf:Property ;
  rdfs:comment "The code specifying the status for this referenced document."^^xsd:string ;
  rdfs:domain "mmt:ReferencedDocument"^^xsd:string ;
  rdfs:label "statusCode"^^xsd:string ;
  rdfs:range "DocumentStatusType_Сode"^^xsd:string .

<https://edi3.org/mmt/vocab#ReferencedDocumentTypeCode>
  a rdf:Property ;
  rdfs:comment "The code specifying the type of referenced document."^^xsd:string ;
  rdfs:domain "mmt:ReferencedDocument"^^xsd:string ;
  rdfs:label "typeCode"^^xsd:string ;
  rdfs:range "DocumentNameType_Сode"^^xsd:string .

<https://edi3.org/mmt/vocab#ReferencedLogisticsTransportEquipment>
  a rdfs:Class ;
  rdfs:comment "A referenced piece of equipment used to hold, protect or secure cargo for logistics purposes."^^xsd:string ;
  rdfs:label "ReferencedLogisticsTransportEquipment"^^xsd:string .

<https://edi3.org/mmt/vocab#ReferencedLogisticsTransportEquipmentCarrierAssignedBookingID>
  a rdf:Property ;
  rdfs:comment "A carrier assigned booking identifier for this piece of referenced logistics transport equipment."^^xsd:string ;
  rdfs:domain "mmt:ReferencedLogisticsTransportEquipment"^^xsd:string ;
  rdfs:label "carrierAssignedBookingID"^^xsd:string ;
  rdfs:range "xsd:ID"^^xsd:string .

<https://edi3.org/mmt/vocab#ReferencedLogisticsTransportEquipmentCategoryCode>
  a rdf:Property ;
  rdfs:comment "The code specifying the category of this referenced piece of logistics transport equipment."^^xsd:string ;
  rdfs:domain "mmt:ReferencedLogisticsTransportEquipment"^^xsd:string ;
  rdfs:label "categoryCode"^^xsd:string ;
  rdfs:range "TransportEquipmentCategoryType_Сode"^^xsd:string .

<https://edi3.org/mmt/vocab#ReferencedLogisticsTransportEquipmentCharacteristicText>
  a rdf:Property ;
  rdfs:comment "The characteristics, expressed as text, of a referenced piece of logistics transport equipment, such as size and type."^^xsd:string ;
  rdfs:domain "mmt:ReferencedLogisticsTransportEquipment"^^xsd:string ;
  rdfs:label "characteristicText"^^xsd:string ;
  rdfs:range "xsd:string"^^xsd:string .

<https://edi3.org/mmt/vocab#ReferencedLogisticsTransportEquipmentGrossVolume>
  a rdf:Property ;
  rdfs:comment "The measure of the gross volume of this piece of referenced logistics transport equipment."^^xsd:string ;
  rdfs:domain "mmt:ReferencedLogisticsTransportEquipment"^^xsd:string ;
  rdfs:label "grossVolume"^^xsd:string ;
  rdfs:range "xsd:decimal"^^xsd:string .

<https://edi3.org/mmt/vocab#ReferencedLogisticsTransportEquipmentGrossWeight>
  a rdf:Property ;
  rdfs:comment "The measure of the gross weight (mass) of this piece of referenced logistics transport equipment which is the weight (mass) including loaded goods, packing and transport equipment."^^xsd:string ;
  rdfs:domain "mmt:ReferencedLogisticsTransportEquipment"^^xsd:string ;
  rdfs:label "grossWeight"^^xsd:string ;
  rdfs:range "xsd:decimal"^^xsd:string .

<https://edi3.org/mmt/vocab#ReferencedLogisticsTransportEquipmentID>
  a rdf:Property ;
  rdfs:comment "The unique identifier for this referenced piece of logistics transport equipment, such as a number, mark or name."^^xsd:string ;
  rdfs:domain "mmt:ReferencedLogisticsTransportEquipment"^^xsd:string ;
  rdfs:label "iD"^^xsd:string ;
  rdfs:range "xsd:ID"^^xsd:string .

<https://edi3.org/mmt/vocab#ReferencedLogisticsTransportEquipmentLoadedPackageQuantity>
  a rdf:Property ;
  rdfs:comment "The number of packages loaded into or onto this piece of referenced logistics transport equipment."^^xsd:string ;
  rdfs:domain "mmt:ReferencedLogisticsTransportEquipment"^^xsd:string ;
  rdfs:label "loadedPackageQuantity"^^xsd:string ;
  rdfs:range "xsd:decimal"^^xsd:string .

<https://edi3.org/mmt/vocab#ReferencedLogisticsTransportEquipmentNetWeight>
  a rdf:Property ;
  rdfs:comment "The measure of the net weight (mass) of this piece of referenced logistics transport equipment."^^xsd:string ;
  rdfs:domain "mmt:ReferencedLogisticsTransportEquipment"^^xsd:string ;
  rdfs:label "netWeight"^^xsd:string ;
  rdfs:range "xsd:decimal"^^xsd:string .

<https://edi3.org/mmt/vocab#ReferencedLogisticsTransportEquipmentSizeTypeCode>
  a rdf:Property ;
  rdfs:comment "The code specifying the characteristics, such as size and type, of this referenced piece of logistics transport equipment."^^xsd:string ;
  rdfs:domain "mmt:ReferencedLogisticsTransportEquipment"^^xsd:string ;
  rdfs:label "sizeTypeCode"^^xsd:string ;
  rdfs:range "EquipmentSizeTypeDescriptionType_Сode"^^xsd:string .

<https://edi3.org/mmt/vocab#ReferencedLogisticsTransportEquipmentUnitQuantity>
  a rdf:Property ;
  rdfs:comment "The number of units of this type of referenced logistics transport equipment."^^xsd:string ;
  rdfs:domain "mmt:ReferencedLogisticsTransportEquipment"^^xsd:string ;
  rdfs:label "unitQuantity"^^xsd:string ;
  rdfs:range "xsd:decimal"^^xsd:string .

<https://edi3.org/mmt/vocab#ReferencedSupplyChainConsignment>
  a rdfs:Class ;
  rdfs:comment "A referenced, separately identifiable collection of goods items to be transported or available to be transported from one consignor to one consignee via one or more modes of transport where each consignment is the subject of one single transport contract."^^xsd:string ;
  rdfs:label "ReferencedSupplyChainConsignment"^^xsd:string .

<https://edi3.org/mmt/vocab#ReferencedSupplyChainConsignmentCarrierAcceptanceDateTime>
  a rdf:Property ;
  rdfs:comment "The date, time, date time or other date time value when this referenced supply chain consignment will be, or has been, accepted by the carrier."^^xsd:string ;
  rdfs:domain "mmt:ReferencedSupplyChainConsignment"^^xsd:string ;
  rdfs:label "carrierAcceptanceDateTime"^^xsd:string ;
  rdfs:range "xsd:datetime"^^xsd:string .

<https://edi3.org/mmt/vocab#ReferencedSupplyChainConsignmentCarrierAssignedID>
  a rdf:Property ;
  rdfs:comment "The unique identifier assigned by the carrier to this referenced supply chain consignment, such as a booking reference number when cargo space is reserved prior to loading."^^xsd:string ;
  rdfs:domain "mmt:ReferencedSupplyChainConsignment"^^xsd:string ;
  rdfs:label "carrierAssignedID"^^xsd:string ;
  rdfs:range "xsd:ID"^^xsd:string .

<https://edi3.org/mmt/vocab#ReferencedSupplyChainConsignmentConsigneeAssignedID>
  a rdf:Property ;
  rdfs:comment "The unique identifier assigned by the consignee to this referenced supply chain consignment."^^xsd:string ;
  rdfs:domain "mmt:ReferencedSupplyChainConsignment"^^xsd:string ;
  rdfs:label "consigneeAssignedID"^^xsd:string ;
  rdfs:range "xsd:ID"^^xsd:string .

<https://edi3.org/mmt/vocab#ReferencedSupplyChainConsignmentConsignmentItemQuantity>
  a rdf:Property ;
  rdfs:comment "The number of consignment items separately defined for transport or customs purposes within this referenced supply chain consignment."^^xsd:string ;
  rdfs:domain "mmt:ReferencedSupplyChainConsignment"^^xsd:string ;
  rdfs:label "consignmentItemQuantity"^^xsd:string ;
  rdfs:range "xsd:decimal"^^xsd:string .

<https://edi3.org/mmt/vocab#ReferencedSupplyChainConsignmentConsignorAssignedID>
  a rdf:Property ;
  rdfs:comment "The unique identifier assigned by the consignor to this referenced supply chain consignment."^^xsd:string ;
  rdfs:domain "mmt:ReferencedSupplyChainConsignment"^^xsd:string ;
  rdfs:label "consignorAssignedID"^^xsd:string ;
  rdfs:range "xsd:ID"^^xsd:string .

<https://edi3.org/mmt/vocab#ReferencedSupplyChainConsignmentCustomsID>
  a rdf:Property ;
  rdfs:comment "The identifier, for customs purposes, for this referenced supply chain consignment."^^xsd:string ;
  rdfs:domain "mmt:ReferencedSupplyChainConsignment"^^xsd:string ;
  rdfs:label "customsID"^^xsd:string ;
  rdfs:range "xsd:ID"^^xsd:string .

<https://edi3.org/mmt/vocab#ReferencedSupplyChainConsignmentFreightForwarderAssignedID>
  a rdf:Property ;
  rdfs:comment "The unique identifier assigned by the freight forwarder to this referenced supply chain consignment."^^xsd:string ;
  rdfs:domain "mmt:ReferencedSupplyChainConsignment"^^xsd:string ;
  rdfs:label "freightForwarderAssignedID"^^xsd:string ;
  rdfs:range "xsd:ID"^^xsd:string .

<https://edi3.org/mmt/vocab#ReferencedSupplyChainConsignmentGrossVolume>
  a rdf:Property ;
  rdfs:comment "A measure of the gross volume, normally calculated by multiplying the maximum length, width and height, of this referenced supply chain consignment."^^xsd:string ;
  rdfs:domain "mmt:ReferencedSupplyChainConsignment"^^xsd:string ;
  rdfs:label "grossVolume"^^xsd:string ;
  rdfs:range "xsd:decimal"^^xsd:string .

<https://edi3.org/mmt/vocab#ReferencedSupplyChainConsignmentGrossWeight>
  a rdf:Property ;
  rdfs:comment "A measure of the gross weight (mass) of this referenced supply chain consignment which includes the weight of packaging but which excludes the weight of any transport equipment."^^xsd:string ;
  rdfs:domain "mmt:ReferencedSupplyChainConsignment"^^xsd:string ;
  rdfs:label "grossWeight"^^xsd:string ;
  rdfs:range "xsd:decimal"^^xsd:string .

<https://edi3.org/mmt/vocab#ReferencedSupplyChainConsignmentID>
  a rdf:Property ;
  rdfs:comment "A unique identifier for this referenced supply chain consignment."^^xsd:string ;
  rdfs:domain "mmt:ReferencedSupplyChainConsignment"^^xsd:string ;
  rdfs:label "iD"^^xsd:string ;
  rdfs:range "xsd:ID"^^xsd:string .

<https://edi3.org/mmt/vocab#ReferencedSupplyChainConsignmentNetWeight>
  a rdf:Property ;
  rdfs:comment "A measure of the net weight (mass) of this referenced consignment which excludes the weight of packaging and the weight of any transport equipment."^^xsd:string ;
  rdfs:domain "mmt:ReferencedSupplyChainConsignment"^^xsd:string ;
  rdfs:label "netWeight"^^xsd:string ;
  rdfs:range "xsd:decimal"^^xsd:string .

<https://edi3.org/mmt/vocab#ReferencedSupplyChainConsignmentSequenceNumber>
  a rdf:Property ;
  rdfs:comment "The sequence number for this referenced supply chain consignment."^^xsd:string ;
  rdfs:domain "mmt:ReferencedSupplyChainConsignment"^^xsd:string ;
  rdfs:label "sequenceNumber"^^xsd:string ;
  rdfs:range "xsd:decimal"^^xsd:string .

<https://edi3.org/mmt/vocab#ReferencedSupplyChainConsignmentTransportSplitDescription>
  a rdf:Property ;
  rdfs:comment "The textual description of the transport split of this referenced supply chain consignment across different transport means or transport equipment."^^xsd:string ;
  rdfs:domain "mmt:ReferencedSupplyChainConsignment"^^xsd:string ;
  rdfs:label "transportSplitDescription"^^xsd:string ;
  rdfs:range "xsd:string"^^xsd:string .

<https://edi3.org/mmt/vocab#ReferencedSupplyChainConsignmentItem>
  a rdfs:Class ;
  rdfs:comment "A reference to an item within a supply chain consignment of goods separately identified for transport and customs purposes."^^xsd:string ;
  rdfs:label "ReferencedSupplyChainConsignmentItem"^^xsd:string .

<https://edi3.org/mmt/vocab#ReferencedSupplyChainConsignmentItemGoodsTypeCode>
  a rdf:Property ;
  rdfs:comment "The code specifying the type of referenced supply chain consignment item."^^xsd:string ;
  rdfs:domain "mmt:ReferencedSupplyChainConsignmentItem"^^xsd:string ;
  rdfs:label "goodsTypeCode"^^xsd:string ;
  rdfs:range "GoodsType_Сode"^^xsd:string .

<https://edi3.org/mmt/vocab#ReferencedSupplyChainConsignmentItemGoodsTypeExtensionCode>
  a rdf:Property ;
  rdfs:comment "The code used as an extension to the type code for further specifying the type of referenced supply chain consignment item."^^xsd:string ;
  rdfs:domain "mmt:ReferencedSupplyChainConsignmentItem"^^xsd:string ;
  rdfs:label "goodsTypeExtensionCode"^^xsd:string ;
  rdfs:range "GoodsTypeExtensionType_Сode"^^xsd:string .

<https://edi3.org/mmt/vocab#ReferencedSupplyChainConsignmentItemSequenceNumber>
  a rdf:Property ;
  rdfs:comment "The sequence number for this referenced supply chain consignment item."^^xsd:string ;
  rdfs:domain "mmt:ReferencedSupplyChainConsignmentItem"^^xsd:string ;
  rdfs:label "sequenceNumber"^^xsd:string ;
  rdfs:range "xsd:decimal"^^xsd:string .

<https://edi3.org/mmt/vocab#ReferencedSupplyChainConsignmentItemTradeLineItemQuantity>
  a rdf:Property ;
  rdfs:comment "The number of trade line items in this referenced supply chain consignment item."^^xsd:string ;
  rdfs:domain "mmt:ReferencedSupplyChainConsignmentItem"^^xsd:string ;
  rdfs:label "tradeLineItemQuantity"^^xsd:string ;
  rdfs:range "xsd:decimal"^^xsd:string .

<https://edi3.org/mmt/vocab#ReferencedTransportMeans>
  a rdfs:Class ;
  rdfs:comment "Reference to a device or method used to convey people, goods, or other objects from place to place."^^xsd:string ;
  rdfs:label "ReferencedTransportMeans"^^xsd:string .

<https://edi3.org/mmt/vocab#ReferencedTransportMeansDriverAccompaniedIndicator>
  a rdf:Property ;
  rdfs:comment "The indication of whether or not this referenced means of transport is accompanied by a driver."^^xsd:string ;
  rdfs:domain "mmt:ReferencedTransportMeans"^^xsd:string ;
  rdfs:label "driverAccompaniedIndicator"^^xsd:string ;
  rdfs:range "xsd:boolean"^^xsd:string .

<https://edi3.org/mmt/vocab#ReferencedTransportMeansID>
  a rdf:Property ;
  rdfs:comment "An identifier of this referenced transport means, such as the International Maritime Organization number for a vessel."^^xsd:string ;
  rdfs:domain "mmt:ReferencedTransportMeans"^^xsd:string ;
  rdfs:label "iD"^^xsd:string ;
  rdfs:range "xsd:ID"^^xsd:string .

<https://edi3.org/mmt/vocab#ReferencedTransportMeansName>
  a rdf:Property ;
  rdfs:comment "The name, expressed as text, of this referenced transport means, such as the vessel name."^^xsd:string ;
  rdfs:domain "mmt:ReferencedTransportMeans"^^xsd:string ;
  rdfs:label "name"^^xsd:string ;
  rdfs:range "xsd:string"^^xsd:string .

<https://edi3.org/mmt/vocab#ReferencedTransportMeansTypeCode>
  a rdf:Property ;
  rdfs:comment "The code specifying the type of referenced transport means [Reference UNECE Recommendation 28]."^^xsd:string ;
  rdfs:domain "mmt:ReferencedTransportMeans"^^xsd:string ;
  rdfs:label "typeCode"^^xsd:string ;
  rdfs:range "TransportMeansType_Сode"^^xsd:string .

<https://edi3.org/mmt/vocab#ReferencedTransportMeansTypeText>
  a rdf:Property ;
  rdfs:comment "The type, expressed as text, of this referenced transport means."^^xsd:string ;
  rdfs:domain "mmt:ReferencedTransportMeans"^^xsd:string ;
  rdfs:label "typeText"^^xsd:string ;
  rdfs:range "xsd:string"^^xsd:string .

<https://edi3.org/mmt/vocab#ReferencedTransportEvent>
  a rdfs:Class ;
  rdfs:comment "A referenced significant occurrence or happening during transport."^^xsd:string ;
  rdfs:label "ReferencedTransportEvent"^^xsd:string .

<https://edi3.org/mmt/vocab#ReferencedTransportEventReasonTypeCode>
  a rdf:Property ;
  rdfs:comment "The code specifying the reason type for this referenced transport event."^^xsd:string ;
  rdfs:domain "mmt:ReferencedTransportEvent"^^xsd:string ;
  rdfs:label "reasonTypeCode"^^xsd:string ;
  rdfs:range "xsd:token"^^xsd:string .

<https://edi3.org/mmt/vocab#ReferencedTransportEventScheduledArrivalDateTime>
  a rdf:Property ;
  rdfs:comment "The date, time, date time or other date time value of the scheduled arrival related to this referenced transport event."^^xsd:string ;
  rdfs:domain "mmt:ReferencedTransportEvent"^^xsd:string ;
  rdfs:label "scheduledArrivalDateTime"^^xsd:string ;
  rdfs:range "xsd:datetime"^^xsd:string .

<https://edi3.org/mmt/vocab#ReferencedTransportEventScheduledDepartureDateTime>
  a rdf:Property ;
  rdfs:comment "The date, time, date time or other date time value of the scheduled departure related to this referenced transport event."^^xsd:string ;
  rdfs:domain "mmt:ReferencedTransportEvent"^^xsd:string ;
  rdfs:label "scheduledDepartureDateTime"^^xsd:string ;
  rdfs:range "xsd:datetime"^^xsd:string .

<https://edi3.org/mmt/vocab#RegisteredTax>
  a rdfs:Class ;
  rdfs:comment "A registered tax or duty system pertaining to an authority."^^xsd:string ;
  rdfs:label "RegisteredTax"^^xsd:string .

<https://edi3.org/mmt/vocab#RegisteredTaxCurrencyCode>
  a rdf:Property ;
  rdfs:comment "The code specifying the currency for this registered tax."^^xsd:string ;
  rdfs:domain "mmt:RegisteredTax"^^xsd:string ;
  rdfs:label "currencyCode"^^xsd:string ;
  rdfs:range "xsd:token"^^xsd:string .

<https://edi3.org/mmt/vocab#RegisteredTaxCustomsDutyIndicator>
  a rdf:Property ;
  rdfs:comment "The indication of whether or not this registered tax is a customs duty."^^xsd:string ;
  rdfs:domain "mmt:RegisteredTax"^^xsd:string ;
  rdfs:label "customsDutyIndicator"^^xsd:string ;
  rdfs:range "xsd:boolean"^^xsd:string .

<https://edi3.org/mmt/vocab#RegisteredTaxDescription>
  a rdf:Property ;
  rdfs:comment "A textual description of this registered tax."^^xsd:string ;
  rdfs:domain "mmt:RegisteredTax"^^xsd:string ;
  rdfs:label "description"^^xsd:string ;
  rdfs:range "xsd:string"^^xsd:string .

<https://edi3.org/mmt/vocab#RegisteredTaxExemptionReasonCode>
  a rdf:Property ;
  rdfs:comment "The code specifying the exemption reason for this registered tax."^^xsd:string ;
  rdfs:domain "mmt:RegisteredTax"^^xsd:string ;
  rdfs:label "exemptionReasonCode"^^xsd:string ;
  rdfs:range "xsd:token"^^xsd:string .

<https://edi3.org/mmt/vocab#RegisteredTaxExemptionReasonText>
  a rdf:Property ;
  rdfs:comment "A reason, expressed as text, for exemption from this registered tax."^^xsd:string ;
  rdfs:domain "mmt:RegisteredTax"^^xsd:string ;
  rdfs:label "exemptionReasonText"^^xsd:string ;
  rdfs:range "xsd:string"^^xsd:string .

<https://edi3.org/mmt/vocab#RegisteredTaxJurisdictionText>
  a rdf:Property ;
  rdfs:comment "A jurisdiction, expressed as text, for this registered tax."^^xsd:string ;
  rdfs:domain "mmt:RegisteredTax"^^xsd:string ;
  rdfs:label "jurisdictionText"^^xsd:string ;
  rdfs:range "xsd:string"^^xsd:string .

<https://edi3.org/mmt/vocab#RegisteredTaxTypeCode>
  a rdf:Property ;
  rdfs:comment "The code specifying the type of registered tax."^^xsd:string ;
  rdfs:domain "mmt:RegisteredTax"^^xsd:string ;
  rdfs:label "typeCode"^^xsd:string ;
  rdfs:range "xsd:token"^^xsd:string .

<https://edi3.org/mmt/vocab#SpatialDimension>
  a rdfs:Class ;
  rdfs:comment "A measure of spatial extent of an object, such as the length, breadth or height of a shipping container."^^xsd:string ;
  rdfs:label "SpatialDimension"^^xsd:string .

<https://edi3.org/mmt/vocab#SpatialDimensionDiameter>
  a rdf:Property ;
  rdfs:comment "The measure of the diameter component for this spatial dimension."^^xsd:string ;
  rdfs:domain "mmt:SpatialDimension"^^xsd:string ;
  rdfs:label "diameter"^^xsd:string ;
  rdfs:range "xsd:decimal"^^xsd:string .

<https://edi3.org/mmt/vocab#SpatialDimensionHeight>
  a rdf:Property ;
  rdfs:comment "The measure of the height component of this spatial dimension."^^xsd:string ;
  rdfs:domain "mmt:SpatialDimension"^^xsd:string ;
  rdfs:label "height"^^xsd:string ;
  rdfs:range "xsd:decimal"^^xsd:string .

<https://edi3.org/mmt/vocab#SpatialDimensionLength>
  a rdf:Property ;
  rdfs:comment "The measure of the length component of this spatial dimension."^^xsd:string ;
  rdfs:domain "mmt:SpatialDimension"^^xsd:string ;
  rdfs:label "length"^^xsd:string ;
  rdfs:range "xsd:decimal"^^xsd:string .

<https://edi3.org/mmt/vocab#SpatialDimensionTypeCode>
  a rdf:Property ;
  rdfs:comment "The code specifying the type of spatial dimension, such as thickness, area, or volume."^^xsd:string ;
  rdfs:domain "mmt:SpatialDimension"^^xsd:string ;
  rdfs:label "typeCode"^^xsd:string ;
  rdfs:range "DimensionType_Сode"^^xsd:string .

<https://edi3.org/mmt/vocab#SpatialDimensionWidth>
  a rdf:Property ;
  rdfs:comment "The measure of the width component of this spatial dimension."^^xsd:string ;
  rdfs:domain "mmt:SpatialDimension"^^xsd:string ;
  rdfs:label "width"^^xsd:string ;
  rdfs:range "xsd:decimal"^^xsd:string .

<https://edi3.org/mmt/vocab#SpecifiedBinaryFile>
  a rdfs:Class ;
  rdfs:comment "A specified computer file or program stored in a binary format."^^xsd:string ;
  rdfs:label "SpecifiedBinaryFile"^^xsd:string .

<https://edi3.org/mmt/vocab#SpecifiedBinaryFileCharacterSetCode>
  a rdf:Property ;
  rdfs:comment "The code specifying the character set for this specified binary file."^^xsd:string ;
  rdfs:domain "mmt:SpecifiedBinaryFile"^^xsd:string ;
  rdfs:label "characterSetCode"^^xsd:string ;
  rdfs:range "xsd:token"^^xsd:string .

<https://edi3.org/mmt/vocab#SpecifiedBinaryFileEncodingCode>
  a rdf:Property ;
  rdfs:comment "The code specifying the encoding of this specified binary file."^^xsd:string ;
  rdfs:domain "mmt:SpecifiedBinaryFile"^^xsd:string ;
  rdfs:label "encodingCode"^^xsd:string ;
  rdfs:range "xsd:token"^^xsd:string .

<https://edi3.org/mmt/vocab#SpecifiedBinaryFileID>
  a rdf:Property ;
  rdfs:comment "A unique identifier for this specified binary file."^^xsd:string ;
  rdfs:domain "mmt:SpecifiedBinaryFile"^^xsd:string ;
  rdfs:label "iD"^^xsd:string ;
  rdfs:range "xsd:ID"^^xsd:string .

<https://edi3.org/mmt/vocab#SpecifiedBinaryFileMIMECode>
  a rdf:Property ;
  rdfs:comment "The code specifying the Multipurpose Internet Mail Extensions (MIME) type for this specified binary file."^^xsd:string ;
  rdfs:domain "mmt:SpecifiedBinaryFile"^^xsd:string ;
  rdfs:label "mIMECode"^^xsd:string ;
  rdfs:range "xsd:token"^^xsd:string .

<https://edi3.org/mmt/vocab#SpecifiedBinaryFileSize>
  a rdf:Property ;
  rdfs:comment "The measure of the size of this specified binary file."^^xsd:string ;
  rdfs:domain "mmt:SpecifiedBinaryFile"^^xsd:string ;
  rdfs:label "size"^^xsd:string ;
  rdfs:range "xsd:decimal"^^xsd:string .

<https://edi3.org/mmt/vocab#SpecifiedBinaryFileURI>
  a rdf:Property ;
  rdfs:comment "The unique Uniform Resource Identifier (URI) for this specified binary file."^^xsd:string ;
  rdfs:domain "mmt:SpecifiedBinaryFile"^^xsd:string ;
  rdfs:label "uRI"^^xsd:string ;
  rdfs:range "xsd:ID"^^xsd:string .

<https://edi3.org/mmt/vocab#SpecifiedObservation>
  a rdfs:Class ;
  rdfs:comment "A specified act or instance of viewing or noting a fact or occurrence for some scientific or other special purpose."^^xsd:string ;
  rdfs:label "SpecifiedObservation"^^xsd:string .

<https://edi3.org/mmt/vocab#SpecifiedObservationDescription>
  a rdf:Property ;
  rdfs:comment "The textual description for this specified observation."^^xsd:string ;
  rdfs:domain "mmt:SpecifiedObservation"^^xsd:string ;
  rdfs:label "description"^^xsd:string ;
  rdfs:range "xsd:string"^^xsd:string .

<https://edi3.org/mmt/vocab#SpecifiedObservationID>
  a rdf:Property ;
  rdfs:comment "The identifier for this specified observation."^^xsd:string ;
  rdfs:domain "mmt:SpecifiedObservation"^^xsd:string ;
  rdfs:label "iD"^^xsd:string ;
  rdfs:range "xsd:ID"^^xsd:string .

<https://edi3.org/mmt/vocab#SpecifiedPeriod>
  a rdfs:Class ;
  rdfs:comment "A specified period of time."^^xsd:string ;
  rdfs:label "SpecifiedPeriod"^^xsd:string .

<https://edi3.org/mmt/vocab#SpecifiedPeriodDurationMeasure>
  a rdf:Property ;
  rdfs:comment "A measure of the length of time for this specified time period such as hours, days, weeks, months, years."^^xsd:string ;
  rdfs:domain "mmt:SpecifiedPeriod"^^xsd:string ;
  rdfs:label "durationMeasure"^^xsd:string ;
  rdfs:range "xsd:decimal"^^xsd:string .

<https://edi3.org/mmt/vocab#SpecifiedPeriodEndDateTime>
  a rdf:Property ;
  rdfs:comment "The date, time, date time or other date time value for the end of this specified period of time."^^xsd:string ;
  rdfs:domain "mmt:SpecifiedPeriod"^^xsd:string ;
  rdfs:label "endDateTime"^^xsd:string ;
  rdfs:range "xsd:datetime"^^xsd:string .

<https://edi3.org/mmt/vocab#SpecifiedPeriodStartDateTime>
  a rdf:Property ;
  rdfs:comment "The date, time, date time or other date time value for the start of this specified period of time."^^xsd:string ;
  rdfs:domain "mmt:SpecifiedPeriod"^^xsd:string ;
  rdfs:label "startDateTime"^^xsd:string ;
  rdfs:range "xsd:datetime"^^xsd:string .

<https://edi3.org/mmt/vocab#SpecifiedTemperature>
  a rdfs:Class ;
  rdfs:comment "A specified temperature value or range of values."^^xsd:string ;
  rdfs:label "SpecifiedTemperature"^^xsd:string .

<https://edi3.org/mmt/vocab#SpecifiedTemperatureMaximumValue>
  a rdf:Property ;
  rdfs:comment "The measure of the highest value of a range for this specified temperature, such as a maximum temperature value of fourteen degrees Celsius."^^xsd:string ;
  rdfs:domain "mmt:SpecifiedTemperature"^^xsd:string ;
  rdfs:label "maximumValue"^^xsd:string ;
  rdfs:range "xsd:decimal"^^xsd:string .

<https://edi3.org/mmt/vocab#SpecifiedTemperatureMinimumValue>
  a rdf:Property ;
  rdfs:comment "The measure of the lowest value of a range for this specified temperature, such as a minimum temperature value of four degrees Celsius."^^xsd:string ;
  rdfs:domain "mmt:SpecifiedTemperature"^^xsd:string ;
  rdfs:label "minimumValue"^^xsd:string ;
  rdfs:range "xsd:decimal"^^xsd:string .

<https://edi3.org/mmt/vocab#SpecifiedTemperatureValue>
  a rdf:Property ;
  rdfs:comment "The measure of the value of this specified temperature, such as a temperature value of ten degrees Celsius."^^xsd:string ;
  rdfs:domain "mmt:SpecifiedTemperature"^^xsd:string ;
  rdfs:label "value"^^xsd:string ;
  rdfs:range "xsd:decimal"^^xsd:string .

<https://edi3.org/mmt/vocab#SubordinateSubordinateLocation>
  a rdfs:Class ;
  rdfs:comment "A physical location or place which is a subordinate location of a subordinate location."^^xsd:string ;
  rdfs:label "SubordinateSubordinateLocation"^^xsd:string .

<https://edi3.org/mmt/vocab#SubordinateSubordinateLocationID>
  a rdf:Property ;
  rdfs:comment "The unique identifier for this subordinate of a subordinate location, such as a United Nations Location Code (UNLOCODE) or GS1 Global Location Number (GLN)."^^xsd:string ;
  rdfs:domain "mmt:SubordinateSubordinateLocation"^^xsd:string ;
  rdfs:label "iD"^^xsd:string ;
  rdfs:range "xsd:ID"^^xsd:string .

<https://edi3.org/mmt/vocab#SubordinateSubordinateLocationName>
  a rdf:Property ;
  rdfs:comment "The name, expressed as text, of this subordinate of a subordinate location."^^xsd:string ;
  rdfs:domain "mmt:SubordinateSubordinateLocation"^^xsd:string ;
  rdfs:label "name"^^xsd:string ;
  rdfs:range "xsd:string"^^xsd:string .

<https://edi3.org/mmt/vocab#SubordinateSubordinateLocationTypeCode>
  a rdf:Property ;
  rdfs:comment "The code specifying the type of subordinate of a subordinate location."^^xsd:string ;
  rdfs:domain "mmt:SubordinateSubordinateLocation"^^xsd:string ;
  rdfs:label "typeCode"^^xsd:string ;
  rdfs:range "LocationFunctionType_Сode"^^xsd:string .

<https://edi3.org/mmt/vocab#SubordinateLocation>
  a rdfs:Class ;
  rdfs:comment "A physical location or place which is a subordinate location of a location."^^xsd:string ;
  rdfs:label "SubordinateLocation"^^xsd:string .

<https://edi3.org/mmt/vocab#SubordinateLocationID>
  a rdf:Property ;
  rdfs:comment "The unique identifier for this subordinate location, such as a United Nations Location Code (UNLOCODE) or GS1 Global Location Number (GLN)."^^xsd:string ;
  rdfs:domain "mmt:SubordinateLocation"^^xsd:string ;
  rdfs:label "iD"^^xsd:string ;
  rdfs:range "xsd:ID"^^xsd:string .

<https://edi3.org/mmt/vocab#SubordinateLocationName>
  a rdf:Property ;
  rdfs:comment "The name, expressed as text, of this subordinate location."^^xsd:string ;
  rdfs:domain "mmt:SubordinateLocation"^^xsd:string ;
  rdfs:label "name"^^xsd:string ;
  rdfs:range "xsd:string"^^xsd:string .

<https://edi3.org/mmt/vocab#SubordinateLocationTypeCode>
  a rdf:Property ;
  rdfs:comment "The code specifying the type of subordinate location."^^xsd:string ;
  rdfs:domain "mmt:SubordinateLocation"^^xsd:string ;
  rdfs:label "typeCode"^^xsd:string ;
  rdfs:range "LocationFunctionType_Сode"^^xsd:string .

<https://edi3.org/mmt/vocab#SupplyChainConsignment>
  a rdfs:Class ;
  rdfs:comment "A separately identifiable collection of goods items to be transported or available to be transported from one consignor to one consignee in a supply chain via one or more modes of transport where each consignment is the subject of one single transport contract."^^xsd:string ;
  rdfs:label "SupplyChainConsignment"^^xsd:string .

<https://edi3.org/mmt/vocab#SupplyChainConsignmentAssociatedInvoiceAmount>
  a rdf:Property ;
  rdfs:comment "A monetary value of an invoice associated with this supply chain consignment."^^xsd:string ;
  rdfs:domain "mmt:SupplyChainConsignment"^^xsd:string ;
  rdfs:label "associatedInvoiceAmount"^^xsd:string ;
  rdfs:range "http://schema.org/amount"^^xsd:string .

<https://edi3.org/mmt/vocab#SupplyChainConsignmentAssociatedInvoiceDiscountAmount>
  a rdf:Property ;
  rdfs:comment "A monetary value of the discount on an invoice associated with this supply chain consignment."^^xsd:string ;
  rdfs:domain "mmt:SupplyChainConsignment"^^xsd:string ;
  rdfs:label "associatedInvoiceDiscountAmount"^^xsd:string ;
  rdfs:range "http://schema.org/amount"^^xsd:string .

<https://edi3.org/mmt/vocab#SupplyChainConsignmentAssociatedInvoiceDiscountPercent>
  a rdf:Property ;
  rdfs:comment "A percent that is a discount on an invoice amount associated with this supply chain consignment."^^xsd:string ;
  rdfs:domain "mmt:SupplyChainConsignment"^^xsd:string ;
  rdfs:label "associatedInvoiceDiscountPercent"^^xsd:string ;
  rdfs:range "xsd:decimal"^^xsd:string .

<https://edi3.org/mmt/vocab#SupplyChainConsignmentAvailabilityDueDateTime>
  a rdf:Property ;
  rdfs:comment "The date, time, date time or other date time value when this supply chain consignment is due to be available."^^xsd:string ;
  rdfs:domain "mmt:SupplyChainConsignment"^^xsd:string ;
  rdfs:label "availabilityDueDateTime"^^xsd:string ;
  rdfs:range "xsd:datetime"^^xsd:string .

<https://edi3.org/mmt/vocab#SupplyChainConsignmentCODAmount>
  a rdf:Property ;
  rdfs:comment "The monetary value of the COD (Cash On Delivery) amount to be collected by the carrier upon delivery of this supply chain consignment."^^xsd:string ;
  rdfs:domain "mmt:SupplyChainConsignment"^^xsd:string ;
  rdfs:label "cODAmount"^^xsd:string ;
  rdfs:range "http://schema.org/amount"^^xsd:string .

<https://edi3.org/mmt/vocab#SupplyChainConsignmentCargoInsuranceInstructions>
  a rdf:Property ;
  rdfs:comment "Cargo insurance instructions, expressed as text, for this supply chain consignment."^^xsd:string ;
  rdfs:domain "mmt:SupplyChainConsignment"^^xsd:string ;
  rdfs:label "cargoInsuranceInstructions"^^xsd:string ;
  rdfs:range "xsd:string"^^xsd:string .

<https://edi3.org/mmt/vocab#SupplyChainConsignmentCargoToleranceInformation>
  a rdf:Property ;
  rdfs:comment "Cargo tolerance information, expressed as text, for this supply chain consignment."^^xsd:string ;
  rdfs:domain "mmt:SupplyChainConsignment"^^xsd:string ;
  rdfs:label "cargoToleranceInformation"^^xsd:string ;
  rdfs:range "xsd:string"^^xsd:string .

<https://edi3.org/mmt/vocab#SupplyChainConsignmentCarrierAcceptanceDateTime>
  a rdf:Property ;
  rdfs:comment "The date, time, date time or other date time value when this supply chain consignment will be, or has been, accepted by the carrier."^^xsd:string ;
  rdfs:domain "mmt:SupplyChainConsignment"^^xsd:string ;
  rdfs:label "carrierAcceptanceDateTime"^^xsd:string ;
  rdfs:range "xsd:datetime"^^xsd:string .

<https://edi3.org/mmt/vocab#SupplyChainConsignmentCarrierAssignedID>
  a rdf:Property ;
  rdfs:comment "The unique identifier assigned by the carrier to this supply chain consignment, such as a booking reference number when cargo space is reserved prior to loading."^^xsd:string ;
  rdfs:domain "mmt:SupplyChainConsignment"^^xsd:string ;
  rdfs:label "carrierAssignedID"^^xsd:string ;
  rdfs:range "xsd:ID"^^xsd:string .

<https://edi3.org/mmt/vocab#SupplyChainConsignmentCarrierProvidedInformation>
  a rdf:Property ;
  rdfs:comment "Information, expressed as text, provided by the carrier for this supply chain consignment."^^xsd:string ;
  rdfs:domain "mmt:SupplyChainConsignment"^^xsd:string ;
  rdfs:label "carrierProvidedInformation"^^xsd:string ;
  rdfs:range "xsd:string"^^xsd:string .

<https://edi3.org/mmt/vocab#SupplyChainConsignmentChargeableTransportationStageQuantity>
  a rdf:Property ;
  rdfs:comment "The number of separately chargeable transportation stages to be covered by this supply chain consignment."^^xsd:string ;
  rdfs:domain "mmt:SupplyChainConsignment"^^xsd:string ;
  rdfs:label "chargeableTransportationStageQuantity"^^xsd:string ;
  rdfs:range "xsd:decimal"^^xsd:string .

<https://edi3.org/mmt/vocab#SupplyChainConsignmentChargeableWeight>
  a rdf:Property ;
  rdfs:comment "A measure of a chargeable weight of this supply chain consignment."^^xsd:string ;
  rdfs:domain "mmt:SupplyChainConsignment"^^xsd:string ;
  rdfs:label "chargeableWeight"^^xsd:string ;
  rdfs:range "xsd:decimal"^^xsd:string .

<https://edi3.org/mmt/vocab#SupplyChainConsignmentConsigneeAssignedID>
  a rdf:Property ;
  rdfs:comment "The unique identifier assigned by the consignee to this supply chain consignment."^^xsd:string ;
  rdfs:domain "mmt:SupplyChainConsignment"^^xsd:string ;
  rdfs:label "consigneeAssignedID"^^xsd:string ;
  rdfs:range "xsd:ID"^^xsd:string .

<https://edi3.org/mmt/vocab#SupplyChainConsignmentConsignmentItemQuantity>
  a rdf:Property ;
  rdfs:comment "The number of consignment items separately defined for transport or customs purposes within this supply chain consignment."^^xsd:string ;
  rdfs:domain "mmt:SupplyChainConsignment"^^xsd:string ;
  rdfs:label "consignmentItemQuantity"^^xsd:string ;
  rdfs:range "xsd:decimal"^^xsd:string .

<https://edi3.org/mmt/vocab#SupplyChainConsignmentConsignorAssignedID>
  a rdf:Property ;
  rdfs:comment "The unique identifier assigned by the consignor to this supply chain consignment."^^xsd:string ;
  rdfs:domain "mmt:SupplyChainConsignment"^^xsd:string ;
  rdfs:label "consignorAssignedID"^^xsd:string ;
  rdfs:range "xsd:ID"^^xsd:string .

<https://edi3.org/mmt/vocab#SupplyChainConsignmentContainerizationIndicator>
  a rdf:Property ;
  rdfs:comment "The indication of whether or not this supply chain consignment is to be transported in a container or containers."^^xsd:string ;
  rdfs:domain "mmt:SupplyChainConsignment"^^xsd:string ;
  rdfs:label "containerizationIndicator"^^xsd:string ;
  rdfs:range "xsd:boolean"^^xsd:string .

<https://edi3.org/mmt/vocab#SupplyChainConsignmentCustomsID>
  a rdf:Property ;
  rdfs:comment "A unique identifier, for customs purposes, for this consignment."^^xsd:string ;
  rdfs:domain "mmt:SupplyChainConsignment"^^xsd:string ;
  rdfs:label "customsID"^^xsd:string ;
  rdfs:range "xsd:ID"^^xsd:string .

<https://edi3.org/mmt/vocab#SupplyChainConsignmentDeclaredValueForCarriageAmount>
  a rdf:Property ;
  rdfs:comment "The monetary value of this supply chain consignment as declared by the shipper or his agent for the purpose of varying the carrier's level of liability from that provided in the contract of carriage, in case of loss or damage to goods or delayed delivery."^^xsd:string ;
  rdfs:domain "mmt:SupplyChainConsignment"^^xsd:string ;
  rdfs:label "declaredValueForCarriageAmount"^^xsd:string ;
  rdfs:range "http://schema.org/amount"^^xsd:string .

<https://edi3.org/mmt/vocab#SupplyChainConsignmentDeclaredValueForCustomsAmount>
  a rdf:Property ;
  rdfs:comment "The monetary value declared for customs purposes for this supply chain consignment."^^xsd:string ;
  rdfs:domain "mmt:SupplyChainConsignment"^^xsd:string ;
  rdfs:label "declaredValueForCustomsAmount"^^xsd:string ;
  rdfs:range "http://schema.org/amount"^^xsd:string .

<https://edi3.org/mmt/vocab#SupplyChainConsignmentDeliveryInformation>
  a rdf:Property ;
  rdfs:comment "The delivery information, expressed as text, for this supply chain consignment."^^xsd:string ;
  rdfs:domain "mmt:SupplyChainConsignment"^^xsd:string ;
  rdfs:label "deliveryInformation"^^xsd:string ;
  rdfs:range "xsd:string"^^xsd:string .

<https://edi3.org/mmt/vocab#SupplyChainConsignmentDemurrageInformation>
  a rdf:Property ;
  rdfs:comment "Demurrage information, expressed as text, for this supply chain consignment."^^xsd:string ;
  rdfs:domain "mmt:SupplyChainConsignment"^^xsd:string ;
  rdfs:label "demurrageInformation"^^xsd:string ;
  rdfs:range "xsd:string"^^xsd:string .

<https://edi3.org/mmt/vocab#SupplyChainConsignmentExportExitDateTime>
  a rdf:Property ;
  rdfs:comment "The date, time, date time or other date time value when this supply chain consignment will exit, or has exited from the last port, airport, or border post of the country of export."^^xsd:string ;
  rdfs:domain "mmt:SupplyChainConsignment"^^xsd:string ;
  rdfs:label "exportExitDateTime"^^xsd:string ;
  rdfs:range "xsd:datetime"^^xsd:string .

<https://edi3.org/mmt/vocab#SupplyChainConsignmentFOBAmount>
  a rdf:Property ;
  rdfs:comment "The monetary value that has to be, or has been, paid for this supply chain consignment as calculated under FOB (Free on Board) delivery terms."^^xsd:string ;
  rdfs:domain "mmt:SupplyChainConsignment"^^xsd:string ;
  rdfs:label "fOBAmount"^^xsd:string ;
  rdfs:range "http://schema.org/amount"^^xsd:string .

<https://edi3.org/mmt/vocab#SupplyChainConsignmentFreightForwarderAssignedID>
  a rdf:Property ;
  rdfs:comment "The unique identifier assigned by the freight forwarder to this supply chain consignment."^^xsd:string ;
  rdfs:domain "mmt:SupplyChainConsignment"^^xsd:string ;
  rdfs:label "freightForwarderAssignedID"^^xsd:string ;
  rdfs:range "xsd:ID"^^xsd:string .

<https://edi3.org/mmt/vocab#SupplyChainConsignmentGoodsReleaseRestrictionText>
  a rdf:Property ;
  rdfs:comment "A goods release restriction, expressed as text, for this supply chain consignment."^^xsd:string ;
  rdfs:domain "mmt:SupplyChainConsignment"^^xsd:string ;
  rdfs:label "goodsReleaseRestrictionText"^^xsd:string ;
  rdfs:range "xsd:string"^^xsd:string .

<https://edi3.org/mmt/vocab#SupplyChainConsignmentGrossVolume>
  a rdf:Property ;
  rdfs:comment "A measure of the gross volume, normally calculated by multiplying the maximum length, width and height of this supply chain consignment."^^xsd:string ;
  rdfs:domain "mmt:SupplyChainConsignment"^^xsd:string ;
  rdfs:label "grossVolume"^^xsd:string ;
  rdfs:range "xsd:decimal"^^xsd:string .

<https://edi3.org/mmt/vocab#SupplyChainConsignmentGrossWeight>
  a rdf:Property ;
  rdfs:comment "A measure of the gross weight (mass) of this supply chain consignment which includes the weight of packaging but which excludes the weight of any transport equipment."^^xsd:string ;
  rdfs:domain "mmt:SupplyChainConsignment"^^xsd:string ;
  rdfs:label "grossWeight"^^xsd:string ;
  rdfs:range "xsd:decimal"^^xsd:string .

<https://edi3.org/mmt/vocab#SupplyChainConsignmentID>
  a rdf:Property ;
  rdfs:comment "A unique identifier for this supply chain consignment."^^xsd:string ;
  rdfs:domain "mmt:SupplyChainConsignment"^^xsd:string ;
  rdfs:label "iD"^^xsd:string ;
  rdfs:range "xsd:ID"^^xsd:string .

<https://edi3.org/mmt/vocab#SupplyChainConsignmentInformation>
  a rdf:Property ;
  rdfs:comment "Information, expressed as text, for this supply chain consignment."^^xsd:string ;
  rdfs:domain "mmt:SupplyChainConsignment"^^xsd:string ;
  rdfs:label "information"^^xsd:string ;
  rdfs:range "xsd:string"^^xsd:string .

<https://edi3.org/mmt/vocab#SupplyChainConsignmentInsurancePremiumAmount>
  a rdf:Property ;
  rdfs:comment "The monetary value of the insurance premium for this supply chain consignment."^^xsd:string ;
  rdfs:domain "mmt:SupplyChainConsignment"^^xsd:string ;
  rdfs:label "insurancePremiumAmount"^^xsd:string ;
  rdfs:range "http://schema.org/amount"^^xsd:string .

<https://edi3.org/mmt/vocab#SupplyChainConsignmentInsuranceValueAmount>
  a rdf:Property ;
  rdfs:comment "The monetary value of this supply chain consignment as covered by an insurance policy."^^xsd:string ;
  rdfs:domain "mmt:SupplyChainConsignment"^^xsd:string ;
  rdfs:label "insuranceValueAmount"^^xsd:string ;
  rdfs:range "http://schema.org/amount"^^xsd:string .

<https://edi3.org/mmt/vocab#SupplyChainConsignmentLoadingInformation>
  a rdf:Property ;
  rdfs:comment "Loading information, expressed as text, for this supply chain consignment, such as advice and instructions."^^xsd:string ;
  rdfs:domain "mmt:SupplyChainConsignment"^^xsd:string ;
  rdfs:label "loadingInformation"^^xsd:string ;
  rdfs:range "xsd:string"^^xsd:string .

<https://edi3.org/mmt/vocab#SupplyChainConsignmentLoadingLength>
  a rdf:Property ;
  rdfs:comment "A measure of the loading length which is the length along a means of transport over which the complete width and height is needed for loading all the goods items in this supply chain consignment."^^xsd:string ;
  rdfs:domain "mmt:SupplyChainConsignment"^^xsd:string ;
  rdfs:label "loadingLength"^^xsd:string ;
  rdfs:range "xsd:decimal"^^xsd:string .

<https://edi3.org/mmt/vocab#SupplyChainConsignmentLoadingListQuantity>
  a rdf:Property ;
  rdfs:comment "The number of loading lists, manifests or similar documents for this supply chain consignment."^^xsd:string ;
  rdfs:domain "mmt:SupplyChainConsignment"^^xsd:string ;
  rdfs:label "loadingListQuantity"^^xsd:string ;
  rdfs:range "xsd:decimal"^^xsd:string .

<https://edi3.org/mmt/vocab#SupplyChainConsignmentLoadingSequenceNumber>
  a rdf:Property ;
  rdfs:comment "The loading sequence number for this supply chain consignment."^^xsd:string ;
  rdfs:domain "mmt:SupplyChainConsignment"^^xsd:string ;
  rdfs:label "loadingSequenceNumber"^^xsd:string ;
  rdfs:range "xsd:decimal"^^xsd:string .

<https://edi3.org/mmt/vocab#SupplyChainConsignmentNetWeight>
  a rdf:Property ;
  rdfs:comment "A measure of the net weight (mass) of this consignment which excludes the weight of packaging of this supply chain consignment and that of any transport equipment."^^xsd:string ;
  rdfs:domain "mmt:SupplyChainConsignment"^^xsd:string ;
  rdfs:label "netWeight"^^xsd:string ;
  rdfs:range "xsd:decimal"^^xsd:string .

<https://edi3.org/mmt/vocab#SupplyChainConsignmentNilCarriageValueIndicator>
  a rdf:Property ;
  rdfs:comment "The indication of whether or not this supply chain consignment has a nil value for carriage."^^xsd:string ;
  rdfs:domain "mmt:SupplyChainConsignment"^^xsd:string ;
  rdfs:label "nilCarriageValueIndicator"^^xsd:string ;
  rdfs:range "xsd:boolean"^^xsd:string .

<https://edi3.org/mmt/vocab#SupplyChainConsignmentNilCustomsValueIndicator>
  a rdf:Property ;
  rdfs:comment "The indication of whether or not this supply chain consignment has a nil value for customs."^^xsd:string ;
  rdfs:domain "mmt:SupplyChainConsignment"^^xsd:string ;
  rdfs:label "nilCustomsValueIndicator"^^xsd:string ;
  rdfs:range "xsd:boolean"^^xsd:string .

<https://edi3.org/mmt/vocab#SupplyChainConsignmentNilInsuranceValueIndicator>
  a rdf:Property ;
  rdfs:comment "The indication of whether or not this supply chain consignment has a nil value for insurance."^^xsd:string ;
  rdfs:domain "mmt:SupplyChainConsignment"^^xsd:string ;
  rdfs:label "nilInsuranceValueIndicator"^^xsd:string ;
  rdfs:range "xsd:boolean"^^xsd:string .

<https://edi3.org/mmt/vocab#SupplyChainConsignmentNumberOfPackages>
  a rdf:Property ;
  rdfs:comment "The number of packages within this supply chain consignment."^^xsd:string ;
  rdfs:domain "mmt:SupplyChainConsignment"^^xsd:string ;
  rdfs:label "numberOfPackages"^^xsd:string ;
  rdfs:range "xsd:decimal"^^xsd:string .

<https://edi3.org/mmt/vocab#SupplyChainConsignmentPackageTypeText>
  a rdf:Property ;
  rdfs:comment "A type of package, expressed as text, for this supply chain consignment."^^xsd:string ;
  rdfs:domain "mmt:SupplyChainConsignment"^^xsd:string ;
  rdfs:label "packageTypeText"^^xsd:string ;
  rdfs:range "xsd:string"^^xsd:string .

<https://edi3.org/mmt/vocab#SupplyChainConsignmentPaymentArrangementCode>
  a rdf:Property ;
  rdfs:comment "The code specifying the payment arrangements for this supply chain consignment."^^xsd:string ;
  rdfs:domain "mmt:SupplyChainConsignment"^^xsd:string ;
  rdfs:label "paymentArrangementCode"^^xsd:string ;
  rdfs:range "TransportPaymentArrangementType_Сode"^^xsd:string .

<https://edi3.org/mmt/vocab#SupplyChainConsignmentRiskFactorCode>
  a rdf:Property ;
  rdfs:comment "The code specifying a risk factor for this supply chain consignment."^^xsd:string ;
  rdfs:domain "mmt:SupplyChainConsignment"^^xsd:string ;
  rdfs:label "riskFactorCode"^^xsd:string ;
  rdfs:range "xsd:token"^^xsd:string .

<https://edi3.org/mmt/vocab#SupplyChainConsignmentSequenceNumber>
  a rdf:Property ;
  rdfs:comment "A sequence number for this supply chain consignment."^^xsd:string ;
  rdfs:domain "mmt:SupplyChainConsignment"^^xsd:string ;
  rdfs:label "sequenceNumber"^^xsd:string ;
  rdfs:range "xsd:decimal"^^xsd:string .

<https://edi3.org/mmt/vocab#SupplyChainConsignmentShipStoresIndicator>
  a rdf:Property ;
  rdfs:comment "The indication of whether or not this supply chain consignment is for ship stores, such as for consumption on the means of transport."^^xsd:string ;
  rdfs:domain "mmt:SupplyChainConsignment"^^xsd:string ;
  rdfs:label "shipStoresIndicator"^^xsd:string ;
  rdfs:range "xsd:boolean"^^xsd:string .

<https://edi3.org/mmt/vocab#SupplyChainConsignmentSummaryDescription>
  a rdf:Property ;
  rdfs:comment "A textual summary description of this supply chain consignment."^^xsd:string ;
  rdfs:domain "mmt:SupplyChainConsignment"^^xsd:string ;
  rdfs:label "summaryDescription"^^xsd:string ;
  rdfs:range "xsd:string"^^xsd:string .

<https://edi3.org/mmt/vocab#SupplyChainConsignmentTareGrossWeight>
  a rdf:Property ;
  rdfs:comment "The measure of the gross weight (mass) including the tare weight of this supply chain consignment."^^xsd:string ;
  rdfs:domain "mmt:SupplyChainConsignment"^^xsd:string ;
  rdfs:label "tareGrossWeight"^^xsd:string ;
  rdfs:range "xsd:decimal"^^xsd:string .

<https://edi3.org/mmt/vocab#SupplyChainConsignmentTotalAllowanceChargeAmount>
  a rdf:Property ;
  rdfs:comment "The total monetary value of all allowances and charges for this supply chain consignment."^^xsd:string ;
  rdfs:domain "mmt:SupplyChainConsignment"^^xsd:string ;
  rdfs:label "totalAllowanceChargeAmount"^^xsd:string ;
  rdfs:range "http://schema.org/amount"^^xsd:string .

<https://edi3.org/mmt/vocab#SupplyChainConsignmentTotalChargeAmount>
  a rdf:Property ;
  rdfs:comment "The total monetary value of all freight and other service charges for this supply chain consignment."^^xsd:string ;
  rdfs:domain "mmt:SupplyChainConsignment"^^xsd:string ;
  rdfs:label "totalChargeAmount"^^xsd:string ;
  rdfs:range "http://schema.org/amount"^^xsd:string .

<https://edi3.org/mmt/vocab#SupplyChainConsignmentTotalCollectChargeAmount>
  a rdf:Property ;
  rdfs:comment "The total monetary value of all freight and other service charges which are to be collected from the consignee at or after delivery for this supply chain consignment."^^xsd:string ;
  rdfs:domain "mmt:SupplyChainConsignment"^^xsd:string ;
  rdfs:label "totalCollectChargeAmount"^^xsd:string ;
  rdfs:range "http://schema.org/amount"^^xsd:string .

<https://edi3.org/mmt/vocab#SupplyChainConsignmentTotalDisbursementAmount>
  a rdf:Property ;
  rdfs:comment "The monetary value of total disbursement for this supply chain consignment, such as the amount to be collected by the carrier according to the order given by the consignor."^^xsd:string ;
  rdfs:domain "mmt:SupplyChainConsignment"^^xsd:string ;
  rdfs:label "totalDisbursementAmount"^^xsd:string ;
  rdfs:range "http://schema.org/amount"^^xsd:string .

<https://edi3.org/mmt/vocab#SupplyChainConsignmentTotalExportExitToImportEntryChargeAmount>
  a rdf:Property ;
  rdfs:comment "The monetary value of the total charge or charges of freight, insurance and other services for this supply chain consignment calculated from the export exit location to the import entry location."^^xsd:string ;
  rdfs:domain "mmt:SupplyChainConsignment"^^xsd:string ;
  rdfs:label "totalExportExitToImportEntryChargeAmount"^^xsd:string ;
  rdfs:range "http://schema.org/amount"^^xsd:string .

<https://edi3.org/mmt/vocab#SupplyChainConsignmentTotalPrepaidChargeAmount>
  a rdf:Property ;
  rdfs:comment "The total monetary value of all freight and other service charges which have been paid in advance for this supply chain consignment."^^xsd:string ;
  rdfs:domain "mmt:SupplyChainConsignment"^^xsd:string ;
  rdfs:label "totalPrepaidChargeAmount"^^xsd:string ;
  rdfs:range "http://schema.org/amount"^^xsd:string .

<https://edi3.org/mmt/vocab#SupplyChainConsignmentTotalTareWeight>
  a rdf:Property ;
  rdfs:comment "The measure of the total tare weight (mass) of this supply chain consignment."^^xsd:string ;
  rdfs:domain "mmt:SupplyChainConsignment"^^xsd:string ;
  rdfs:label "totalTareWeight"^^xsd:string ;
  rdfs:range "xsd:decimal"^^xsd:string .

<https://edi3.org/mmt/vocab#SupplyChainConsignmentTradedParcelID>
  a rdf:Property ;
  rdfs:comment "A traded parcel identifier for this supply chain consignment."^^xsd:string ;
  rdfs:domain "mmt:SupplyChainConsignment"^^xsd:string ;
  rdfs:label "tradedParcelID"^^xsd:string ;
  rdfs:range "xsd:ID"^^xsd:string .

<https://edi3.org/mmt/vocab#SupplyChainConsignmentTransportEquipmentQuantity>
  a rdf:Property ;
  rdfs:comment "A number of pieces of transport equipment, such as containers or similar unit load devices, in this supply chain consignment."^^xsd:string ;
  rdfs:domain "mmt:SupplyChainConsignment"^^xsd:string ;
  rdfs:label "transportEquipmentQuantity"^^xsd:string ;
  rdfs:range "xsd:decimal"^^xsd:string .

<https://edi3.org/mmt/vocab#SupplyChainConsignmentTransportEquipmentSplitGoodsIndicator>
  a rdf:Property ;
  rdfs:comment "The indication of whether or not the goods in this supply chain consignment are split across more than one piece of transport equipment."^^xsd:string ;
  rdfs:domain "mmt:SupplyChainConsignment"^^xsd:string ;
  rdfs:label "transportEquipmentSplitGoodsIndicator"^^xsd:string ;
  rdfs:range "xsd:boolean"^^xsd:string .

<https://edi3.org/mmt/vocab#SupplyChainConsignmentTransportSplitDescription>
  a rdf:Property ;
  rdfs:comment "The textual description of the transport split of this supply chain consignment across different transport means or transport equipment."^^xsd:string ;
  rdfs:domain "mmt:SupplyChainConsignment"^^xsd:string ;
  rdfs:label "transportSplitDescription"^^xsd:string ;
  rdfs:range "xsd:string"^^xsd:string .

<https://edi3.org/mmt/vocab#SupplyChainConsignmentTransshipmentPermittedIndicator>
  a rdf:Property ;
  rdfs:comment "The indication of whether or not transshipment is permitted for this supply chain consignment."^^xsd:string ;
  rdfs:domain "mmt:SupplyChainConsignment"^^xsd:string ;
  rdfs:label "transshipmentPermittedIndicator"^^xsd:string ;
  rdfs:range "xsd:boolean"^^xsd:string .

<https://edi3.org/mmt/vocab#SupplyChainConsignmentUnloadingSequenceNumber>
  a rdf:Property ;
  rdfs:comment "The unloading sequence number for this supply chain consignment."^^xsd:string ;
  rdfs:domain "mmt:SupplyChainConsignment"^^xsd:string ;
  rdfs:label "unloadingSequenceNumber"^^xsd:string ;
  rdfs:range "xsd:decimal"^^xsd:string .

<https://edi3.org/mmt/vocab#SupplyChainConsignmentWarehouseArrivalDateTime>
  a rdf:Property ;
  rdfs:comment "The date, time, date time or other date time value of the arrival of this supply chain consignment at a warehouse."^^xsd:string ;
  rdfs:domain "mmt:SupplyChainConsignment"^^xsd:string ;
  rdfs:label "warehouseArrivalDateTime"^^xsd:string ;
  rdfs:range "xsd:datetime"^^xsd:string .

<https://edi3.org/mmt/vocab#SupplyChainConsignmentItem>
  a rdfs:Class ;
  rdfs:comment "An item within a supply chain consignment of goods separately identified for transport and customs purposes."^^xsd:string ;
  rdfs:label "SupplyChainConsignmentItem"^^xsd:string .

<https://edi3.org/mmt/vocab#SupplyChainConsignmentItemCargoToleranceInformation>
  a rdf:Property ;
  rdfs:comment "Cargo tolerance information, expressed as text, for this supply chain consignment item."^^xsd:string ;
  rdfs:domain "mmt:SupplyChainConsignmentItem"^^xsd:string ;
  rdfs:label "cargoToleranceInformation"^^xsd:string ;
  rdfs:range "xsd:string"^^xsd:string .

<https://edi3.org/mmt/vocab#SupplyChainConsignmentItemChargeableWeight>
  a rdf:Property ;
  rdfs:comment "A measure of the supply chain consignment item weight on which charges are to be based."^^xsd:string ;
  rdfs:domain "mmt:SupplyChainConsignmentItem"^^xsd:string ;
  rdfs:label "chargeableWeight"^^xsd:string ;
  rdfs:range "xsd:decimal"^^xsd:string .

<https://edi3.org/mmt/vocab#SupplyChainConsignmentItemDamageRemark>
  a rdf:Property ;
  rdfs:comment "Damage remarks, expressed as text, for this supply chain consignment item."^^xsd:string ;
  rdfs:domain "mmt:SupplyChainConsignmentItem"^^xsd:string ;
  rdfs:label "damageRemark"^^xsd:string ;
  rdfs:range "xsd:string"^^xsd:string .

<https://edi3.org/mmt/vocab#SupplyChainConsignmentItemDeclaredValueForCarriageAmount>
  a rdf:Property ;
  rdfs:comment "The monetary value of this supply chain consignment item as declared by the shipper or his agent for the purpose of varying the carrier's level of liability from that provided in the contract of carriage, in case of loss or damage to goods or delayed delivery."^^xsd:string ;
  rdfs:domain "mmt:SupplyChainConsignmentItem"^^xsd:string ;
  rdfs:label "declaredValueForCarriageAmount"^^xsd:string ;
  rdfs:range "http://schema.org/amount"^^xsd:string .

<https://edi3.org/mmt/vocab#SupplyChainConsignmentItemDeclaredValueForCustomsAmount>
  a rdf:Property ;
  rdfs:comment "The monetary value of this supply chain consignment item as declared for customs purposes."^^xsd:string ;
  rdfs:domain "mmt:SupplyChainConsignmentItem"^^xsd:string ;
  rdfs:label "declaredValueForCustomsAmount"^^xsd:string ;
  rdfs:range "http://schema.org/amount"^^xsd:string .

<https://edi3.org/mmt/vocab#SupplyChainConsignmentItemDeclaredValueForStatisticsAmount>
  a rdf:Property ;
  rdfs:comment "The monetary value of this supply chain consignment item as declared for statistical purposes."^^xsd:string ;
  rdfs:domain "mmt:SupplyChainConsignmentItem"^^xsd:string ;
  rdfs:label "declaredValueForStatisticsAmount"^^xsd:string ;
  rdfs:range "http://schema.org/amount"^^xsd:string .

<https://edi3.org/mmt/vocab#SupplyChainConsignmentItemDeliveryInstructions>
  a rdf:Property ;
  rdfs:comment "Delivery instructions, expressed as text, for this supply chain consignment item."^^xsd:string ;
  rdfs:domain "mmt:SupplyChainConsignmentItem"^^xsd:string ;
  rdfs:label "deliveryInstructions"^^xsd:string ;
  rdfs:range "xsd:string"^^xsd:string .

<https://edi3.org/mmt/vocab#SupplyChainConsignmentItemExportTypeCode>
  a rdf:Property ;
  rdfs:comment "The code specifying the export type of supply chain consignment item."^^xsd:string ;
  rdfs:domain "mmt:SupplyChainConsignmentItem"^^xsd:string ;
  rdfs:label "exportTypeCode"^^xsd:string ;
  rdfs:range "xsd:token"^^xsd:string .

<https://edi3.org/mmt/vocab#SupplyChainConsignmentItemFOBAmount>
  a rdf:Property ;
  rdfs:comment "The monetary value for this supply chain consignment item as calculated under FOB (Free On Board) delivery terms."^^xsd:string ;
  rdfs:domain "mmt:SupplyChainConsignmentItem"^^xsd:string ;
  rdfs:label "fOBAmount"^^xsd:string ;
  rdfs:range "http://schema.org/amount"^^xsd:string .

<https://edi3.org/mmt/vocab#SupplyChainConsignmentItemFirstTypeExtensionCode>
  a rdf:Property ;
  rdfs:comment "The code used as a first extension to the type code for further specifying the type of supply chain consignment item."^^xsd:string ;
  rdfs:domain "mmt:SupplyChainConsignmentItem"^^xsd:string ;
  rdfs:label "firstTypeExtensionCode"^^xsd:string ;
  rdfs:range "xsd:token"^^xsd:string .

<https://edi3.org/mmt/vocab#SupplyChainConsignmentItemGlobalID>
  a rdf:Property ;
  rdfs:comment "A global identifier for this supply chain consignment item."^^xsd:string ;
  rdfs:domain "mmt:SupplyChainConsignmentItem"^^xsd:string ;
  rdfs:label "globalID"^^xsd:string ;
  rdfs:range "xsd:ID"^^xsd:string .

<https://edi3.org/mmt/vocab#SupplyChainConsignmentItemGoodsTypeCode>
  a rdf:Property ;
  rdfs:comment "The code specifying the type of supply chain consignment item."^^xsd:string ;
  rdfs:domain "mmt:SupplyChainConsignmentItem"^^xsd:string ;
  rdfs:label "goodsTypeCode"^^xsd:string ;
  rdfs:range "GoodsType_Сode"^^xsd:string .

<https://edi3.org/mmt/vocab#SupplyChainConsignmentItemGoodsTypeExtensionCode>
  a rdf:Property ;
  rdfs:comment "The code used as an extension to the type code for further specifying the type of supply chain consignment item."^^xsd:string ;
  rdfs:domain "mmt:SupplyChainConsignmentItem"^^xsd:string ;
  rdfs:label "goodsTypeExtensionCode"^^xsd:string ;
  rdfs:range "GoodsTypeExtensionType_Сode"^^xsd:string .

<https://edi3.org/mmt/vocab#SupplyChainConsignmentItemGrossVolume>
  a rdf:Property ;
  rdfs:comment "A measure of the gross volume, normally calculated by multiplying the maximum length, width and height of this supply chain consignment item."^^xsd:string ;
  rdfs:domain "mmt:SupplyChainConsignmentItem"^^xsd:string ;
  rdfs:label "grossVolume"^^xsd:string ;
  rdfs:range "xsd:decimal"^^xsd:string .

<https://edi3.org/mmt/vocab#SupplyChainConsignmentItemGrossWeight>
  a rdf:Property ;
  rdfs:comment "A measure of the gross weight (mass) of this supply chain consignment item which includes packaging but excludes any transport equipment."^^xsd:string ;
  rdfs:domain "mmt:SupplyChainConsignmentItem"^^xsd:string ;
  rdfs:label "grossWeight"^^xsd:string ;
  rdfs:range "xsd:decimal"^^xsd:string .

<https://edi3.org/mmt/vocab#SupplyChainConsignmentItemID>
  a rdf:Property ;
  rdfs:comment "A unique identifier for this supply chain consignment item."^^xsd:string ;
  rdfs:domain "mmt:SupplyChainConsignmentItem"^^xsd:string ;
  rdfs:label "iD"^^xsd:string ;
  rdfs:range "xsd:ID"^^xsd:string .

<https://edi3.org/mmt/vocab#SupplyChainConsignmentItemImportTypeCode>
  a rdf:Property ;
  rdfs:comment "The code specifying the import type of supply chain consignment item."^^xsd:string ;
  rdfs:domain "mmt:SupplyChainConsignmentItem"^^xsd:string ;
  rdfs:label "importTypeCode"^^xsd:string ;
  rdfs:range "xsd:token"^^xsd:string .

<https://edi3.org/mmt/vocab#SupplyChainConsignmentItemInformation>
  a rdf:Property ;
  rdfs:comment "Information, expressed as text, for this supply chain consignment item."^^xsd:string ;
  rdfs:domain "mmt:SupplyChainConsignmentItem"^^xsd:string ;
  rdfs:label "information"^^xsd:string ;
  rdfs:range "xsd:string"^^xsd:string .

<https://edi3.org/mmt/vocab#SupplyChainConsignmentItemInsuranceValueAmount>
  a rdf:Property ;
  rdfs:comment "The monetary value of this supply chain consignment item as covered by an insurance policy."^^xsd:string ;
  rdfs:domain "mmt:SupplyChainConsignmentItem"^^xsd:string ;
  rdfs:label "insuranceValueAmount"^^xsd:string ;
  rdfs:range "http://schema.org/amount"^^xsd:string .

<https://edi3.org/mmt/vocab#SupplyChainConsignmentItemInvoiceAmount>
  a rdf:Property ;
  rdfs:comment "A monetary value for an invoice for this supply chain consignment item."^^xsd:string ;
  rdfs:domain "mmt:SupplyChainConsignmentItem"^^xsd:string ;
  rdfs:label "invoiceAmount"^^xsd:string ;
  rdfs:range "http://schema.org/amount"^^xsd:string .

<https://edi3.org/mmt/vocab#SupplyChainConsignmentItemLoadingLength>
  a rdf:Property ;
  rdfs:comment "The measure of the loading length of this supply chain consignment item."^^xsd:string ;
  rdfs:domain "mmt:SupplyChainConsignmentItem"^^xsd:string ;
  rdfs:label "loadingLength"^^xsd:string ;
  rdfs:range "xsd:decimal"^^xsd:string .

<https://edi3.org/mmt/vocab#SupplyChainConsignmentItemNationalTypeExtensionCode>
  a rdf:Property ;
  rdfs:comment "The code used as a national extension to the type code for further specifying the type of supply chain consignment item."^^xsd:string ;
  rdfs:domain "mmt:SupplyChainConsignmentItem"^^xsd:string ;
  rdfs:label "nationalTypeExtensionCode"^^xsd:string ;
  rdfs:range "xsd:token"^^xsd:string .

<https://edi3.org/mmt/vocab#SupplyChainConsignmentItemNetWeight>
  a rdf:Property ;
  rdfs:comment "A measure of the net weight (mass) of this supply chain consignment item which excludes all packaging."^^xsd:string ;
  rdfs:domain "mmt:SupplyChainConsignmentItem"^^xsd:string ;
  rdfs:label "netWeight"^^xsd:string ;
  rdfs:range "xsd:decimal"^^xsd:string .

<https://edi3.org/mmt/vocab#SupplyChainConsignmentItemPackageQuantity>
  a rdf:Property ;
  rdfs:comment "The package quantity for this supply chain consignment item."^^xsd:string ;
  rdfs:domain "mmt:SupplyChainConsignmentItem"^^xsd:string ;
  rdfs:label "packageQuantity"^^xsd:string ;
  rdfs:range "xsd:decimal"^^xsd:string .

<https://edi3.org/mmt/vocab#SupplyChainConsignmentItemPackageTypeText>
  a rdf:Property ;
  rdfs:comment "A package type, expressed as text, for this supply chain consignment item."^^xsd:string ;
  rdfs:domain "mmt:SupplyChainConsignmentItem"^^xsd:string ;
  rdfs:label "packageTypeText"^^xsd:string ;
  rdfs:range "xsd:string"^^xsd:string .

<https://edi3.org/mmt/vocab#SupplyChainConsignmentItemSecondTypeExtensionCode>
  a rdf:Property ;
  rdfs:comment "The code used as a second extension to the type code for further specifying the type of supply chain consignment item."^^xsd:string ;
  rdfs:domain "mmt:SupplyChainConsignmentItem"^^xsd:string ;
  rdfs:label "secondTypeExtensionCode"^^xsd:string ;
  rdfs:range "xsd:token"^^xsd:string .

<https://edi3.org/mmt/vocab#SupplyChainConsignmentItemSequenceNumber>
  a rdf:Property ;
  rdfs:comment "The sequence number for this supply chain consignment item."^^xsd:string ;
  rdfs:domain "mmt:SupplyChainConsignmentItem"^^xsd:string ;
  rdfs:label "sequenceNumber"^^xsd:string ;
  rdfs:range "xsd:decimal"^^xsd:string .

<https://edi3.org/mmt/vocab#SupplyChainConsignmentItemSpecialInstructions>
  a rdf:Property ;
  rdfs:comment "Special instructions, expressed as text, for this supply chain consignment item."^^xsd:string ;
  rdfs:domain "mmt:SupplyChainConsignmentItem"^^xsd:string ;
  rdfs:label "specialInstructions"^^xsd:string ;
  rdfs:range "xsd:string"^^xsd:string .

<https://edi3.org/mmt/vocab#SupplyChainConsignmentItemTariffQuantity>
  a rdf:Property ;
  rdfs:comment "The tariff quantity in this supply chain consignment item."^^xsd:string ;
  rdfs:domain "mmt:SupplyChainConsignmentItem"^^xsd:string ;
  rdfs:label "tariffQuantity"^^xsd:string ;
  rdfs:range "xsd:decimal"^^xsd:string .

<https://edi3.org/mmt/vocab#SupplyChainConsignmentItemTotalChargeAmount>
  a rdf:Property ;
  rdfs:comment "The monetary value of all freight and other service charges for this supply chain consignment item."^^xsd:string ;
  rdfs:domain "mmt:SupplyChainConsignmentItem"^^xsd:string ;
  rdfs:label "totalChargeAmount"^^xsd:string ;
  rdfs:range "http://schema.org/amount"^^xsd:string .

<https://edi3.org/mmt/vocab#SupplyChainConsignmentItemTotalExportExitToImportEntryChargeAmount>
  a rdf:Property ;
  rdfs:comment "The monetary value of the total charge or charges of freight, insurance and other services for this supply chain consignment item calculated from the export exit location to the import entry location."^^xsd:string ;
  rdfs:domain "mmt:SupplyChainConsignmentItem"^^xsd:string ;
  rdfs:label "totalExportExitToImportEntryChargeAmount"^^xsd:string ;
  rdfs:range "http://schema.org/amount"^^xsd:string .

<https://edi3.org/mmt/vocab#SupplyChainConsignmentItemTradeLineItemQuantity>
  a rdf:Property ;
  rdfs:comment "The number of trade line items in this supply chain consignment item."^^xsd:string ;
  rdfs:domain "mmt:SupplyChainConsignmentItem"^^xsd:string ;
  rdfs:label "tradeLineItemQuantity"^^xsd:string ;
  rdfs:range "xsd:decimal"^^xsd:string .

<https://edi3.org/mmt/vocab#SupplyChainEvent>
  a rdfs:Class ;
  rdfs:comment "A significant occurrence or happening in a supply chain."^^xsd:string ;
  rdfs:label "SupplyChainEvent"^^xsd:string .

<https://edi3.org/mmt/vocab#SupplyChainEventDescription>
  a rdf:Property ;
  rdfs:comment "A textual description of this supply chain event."^^xsd:string ;
  rdfs:domain "mmt:SupplyChainEvent"^^xsd:string ;
  rdfs:label "description"^^xsd:string ;
  rdfs:range "xsd:string"^^xsd:string .

<https://edi3.org/mmt/vocab#SupplyChainEventDescriptionBinaryObject>
  a rdf:Property ;
  rdfs:comment "Binary object data, such as a photograph, describing this supply chain event."^^xsd:string ;
  rdfs:domain "mmt:SupplyChainEvent"^^xsd:string ;
  rdfs:label "descriptionBinaryObject"^^xsd:string ;
  rdfs:range "xsd:base64Binary"^^xsd:string .

<https://edi3.org/mmt/vocab#SupplyChainEventEarliestOccurrenceDateTime>
  a rdf:Property ;
  rdfs:comment "The date, time, date time, or other date time value of the earliest occurrence of this supply chain event."^^xsd:string ;
  rdfs:domain "mmt:SupplyChainEvent"^^xsd:string ;
  rdfs:label "earliestOccurrenceDateTime"^^xsd:string ;
  rdfs:range "xsd:datetime"^^xsd:string .

<https://edi3.org/mmt/vocab#SupplyChainEventFrequencyCode>
  a rdf:Property ;
  rdfs:comment "The code specifying a frequency for this supply chain event."^^xsd:string ;
  rdfs:domain "mmt:SupplyChainEvent"^^xsd:string ;
  rdfs:label "frequencyCode"^^xsd:string ;
  rdfs:range "xsd:token"^^xsd:string .

<https://edi3.org/mmt/vocab#SupplyChainEventID>
  a rdf:Property ;
  rdfs:comment "The unique identifier for this supply chain event."^^xsd:string ;
  rdfs:domain "mmt:SupplyChainEvent"^^xsd:string ;
  rdfs:label "iD"^^xsd:string ;
  rdfs:range "xsd:ID"^^xsd:string .

<https://edi3.org/mmt/vocab#SupplyChainEventLatestOccurrenceDateTime>
  a rdf:Property ;
  rdfs:comment "The date, time, date time, or other date time value of the latest occurrence of this supply chain event."^^xsd:string ;
  rdfs:domain "mmt:SupplyChainEvent"^^xsd:string ;
  rdfs:label "latestOccurrenceDateTime"^^xsd:string ;
  rdfs:range "xsd:datetime"^^xsd:string .

<https://edi3.org/mmt/vocab#SupplyChainEventOccurrenceDateTime>
  a rdf:Property ;
  rdfs:comment "A date, time, date time, or other date time value of an occurrence of this supply chain event."^^xsd:string ;
  rdfs:domain "mmt:SupplyChainEvent"^^xsd:string ;
  rdfs:label "occurrenceDateTime"^^xsd:string ;
  rdfs:range "xsd:datetime"^^xsd:string .

<https://edi3.org/mmt/vocab#SupplyChainEventOccurrenceTime>
  a rdf:Property ;
  rdfs:comment "A time value of an occurrence of this supply chain event."^^xsd:string ;
  rdfs:domain "mmt:SupplyChainEvent"^^xsd:string ;
  rdfs:label "occurrenceTime"^^xsd:string ;
  rdfs:range "xsd:datetime"^^xsd:string .

<https://edi3.org/mmt/vocab#SupplyChainEventTypeCode>
  a rdf:Property ;
  rdfs:comment "A code specifying the type of supply chain event."^^xsd:string ;
  rdfs:domain "mmt:SupplyChainEvent"^^xsd:string ;
  rdfs:label "typeCode"^^xsd:string ;
  rdfs:range "xsd:token"^^xsd:string .

<https://edi3.org/mmt/vocab#SupplyChainEventUnitQuantity>
  a rdf:Property ;
  rdfs:comment "A number of units for this supply chain event."^^xsd:string ;
  rdfs:domain "mmt:SupplyChainEvent"^^xsd:string ;
  rdfs:label "unitQuantity"^^xsd:string ;
  rdfs:range "xsd:decimal"^^xsd:string .

<https://edi3.org/mmt/vocab#SupplyChainPackaging>
  a rdfs:Class ;
  rdfs:comment "Any material with which supply chain goods are packaged, such as a box or bubble wrap."^^xsd:string ;
  rdfs:label "SupplyChainPackaging"^^xsd:string .

<https://edi3.org/mmt/vocab#SupplyChainPackagingConditionCode>
  a rdf:Property ;
  rdfs:comment "A code specifying the condition of this supply chain packaging."^^xsd:string ;
  rdfs:domain "mmt:SupplyChainPackaging"^^xsd:string ;
  rdfs:label "conditionCode"^^xsd:string ;
  rdfs:range "xsd:token"^^xsd:string .

<https://edi3.org/mmt/vocab#SupplyChainPackagingDescription>
  a rdf:Property ;
  rdfs:comment "A textual description of this supply chain packaging."^^xsd:string ;
  rdfs:domain "mmt:SupplyChainPackaging"^^xsd:string ;
  rdfs:label "description"^^xsd:string ;
  rdfs:range "xsd:string"^^xsd:string .

<https://edi3.org/mmt/vocab#SupplyChainPackagingDisposalMethodCode>
  a rdf:Property ;
  rdfs:comment "A code specifying the disposal method of this supply chain packaging."^^xsd:string ;
  rdfs:domain "mmt:SupplyChainPackaging"^^xsd:string ;
  rdfs:label "disposalMethodCode"^^xsd:string ;
  rdfs:range "xsd:token"^^xsd:string .

<https://edi3.org/mmt/vocab#SupplyChainPackagingMaximumStackabilityQuantity>
  a rdf:Property ;
  rdfs:comment "The number of units of this type of supply chain packaging which can be stacked on top of each other."^^xsd:string ;
  rdfs:domain "mmt:SupplyChainPackaging"^^xsd:string ;
  rdfs:label "maximumStackabilityQuantity"^^xsd:string ;
  rdfs:range "xsd:decimal"^^xsd:string .

<https://edi3.org/mmt/vocab#SupplyChainPackagingMaximumStackabilityWeight>
  a rdf:Property ;
  rdfs:comment "The measure of the maximum stackability weight of this supply chain packaging."^^xsd:string ;
  rdfs:domain "mmt:SupplyChainPackaging"^^xsd:string ;
  rdfs:label "maximumStackabilityWeight"^^xsd:string ;
  rdfs:range "xsd:decimal"^^xsd:string .

<https://edi3.org/mmt/vocab#SupplyChainPackagingReturnableIndicator>
  a rdf:Property ;
  rdfs:comment "The indication of whether or not this supply chain packaging is returnable."^^xsd:string ;
  rdfs:domain "mmt:SupplyChainPackaging"^^xsd:string ;
  rdfs:label "returnableIndicator"^^xsd:string ;
  rdfs:range "xsd:boolean"^^xsd:string .

<https://edi3.org/mmt/vocab#SupplyChainPackagingTypeCode>
  a rdf:Property ;
  rdfs:comment "The code specifying the type of supply chain packaging."^^xsd:string ;
  rdfs:domain "mmt:SupplyChainPackaging"^^xsd:string ;
  rdfs:label "typeCode"^^xsd:string ;
  rdfs:range "PackageType_Сode"^^xsd:string .

<https://edi3.org/mmt/vocab#SupplyChainPackagingTypeText>
  a rdf:Property ;
  rdfs:comment "The type, expressed as text, of supply chain packaging."^^xsd:string ;
  rdfs:domain "mmt:SupplyChainPackaging"^^xsd:string ;
  rdfs:label "typeText"^^xsd:string ;
  rdfs:range "xsd:string"^^xsd:string .

<https://edi3.org/mmt/vocab#SupplyChainPackagingWeight>
  a rdf:Property ;
  rdfs:comment "A measure of the weight of this supply chain packaging."^^xsd:string ;
  rdfs:domain "mmt:SupplyChainPackaging"^^xsd:string ;
  rdfs:label "weight"^^xsd:string ;
  rdfs:range "xsd:decimal"^^xsd:string .

<https://edi3.org/mmt/vocab#SupplyChainTradeLineItem>
  a rdfs:Class ;
  rdfs:comment "A collection of information specific to an item being used or reported on for supply chain trade purposes."^^xsd:string ;
  rdfs:label "SupplyChainTradeLineItem"^^xsd:string .

<https://edi3.org/mmt/vocab#SupplyChainTradeLineItemBarcodeID>
  a rdf:Property ;
  rdfs:comment "A unique barcode identifier for this supply chain trade line item."^^xsd:string ;
  rdfs:domain "mmt:SupplyChainTradeLineItem"^^xsd:string ;
  rdfs:label "barcodeID"^^xsd:string ;
  rdfs:range "xsd:ID"^^xsd:string .

<https://edi3.org/mmt/vocab#SupplyChainTradeLineItemDescriptionCode>
  a rdf:Property ;
  rdfs:comment "The code specifying a description of this supply chain trade line item."^^xsd:string ;
  rdfs:domain "mmt:SupplyChainTradeLineItem"^^xsd:string ;
  rdfs:label "descriptionCode"^^xsd:string ;
  rdfs:range "xsd:token"^^xsd:string .

<https://edi3.org/mmt/vocab#SupplyChainTradeLineItemID>
  a rdf:Property ;
  rdfs:comment "The unique identifier for this supply chain trade line item."^^xsd:string ;
  rdfs:domain "mmt:SupplyChainTradeLineItem"^^xsd:string ;
  rdfs:label "iD"^^xsd:string ;
  rdfs:range "xsd:ID"^^xsd:string .

<https://edi3.org/mmt/vocab#SupplyChainTradeLineItemSequenceNumber>
  a rdf:Property ;
  rdfs:comment "A sequence number for this supply chain trade line item."^^xsd:string ;
  rdfs:domain "mmt:SupplyChainTradeLineItem"^^xsd:string ;
  rdfs:label "sequenceNumber"^^xsd:string ;
  rdfs:range "xsd:decimal"^^xsd:string .

<https://edi3.org/mmt/vocab#SupplyChainTradeLineItemTypeCode>
  a rdf:Property ;
  rdfs:comment "The code specifying the type of supply chain trade line item."^^xsd:string ;
  rdfs:domain "mmt:SupplyChainTradeLineItem"^^xsd:string ;
  rdfs:label "typeCode"^^xsd:string ;
  rdfs:range "xsd:token"^^xsd:string .

<https://edi3.org/mmt/vocab#SupplyChainTradeLineItemTypeExtensionCode>
  a rdf:Property ;
  rdfs:comment "The code used as an extension to the type code for further specifying a type of supply chain trade line item."^^xsd:string ;
  rdfs:domain "mmt:SupplyChainTradeLineItem"^^xsd:string ;
  rdfs:label "typeExtensionCode"^^xsd:string ;
  rdfs:range "xsd:token"^^xsd:string .

<https://edi3.org/mmt/vocab#SupplyChainTradeTransaction>
  a rdfs:Class ;
  rdfs:comment "A group of supply chain trade line items, trade agreement, trade delivery and trade settlement details."^^xsd:string ;
  rdfs:label "SupplyChainTradeTransaction"^^xsd:string .

<https://edi3.org/mmt/vocab#SupplyChainTradeTransactionID>
  a rdf:Property ;
  rdfs:comment "A unique identifier for this supply chain trade transaction."^^xsd:string ;
  rdfs:domain "mmt:SupplyChainTradeTransaction"^^xsd:string ;
  rdfs:label "iD"^^xsd:string ;
  rdfs:range "xsd:ID"^^xsd:string .

<https://edi3.org/mmt/vocab#SupplyChainTradeTransactionInformation>
  a rdf:Property ;
  rdfs:comment "Information, expressed as text, for this supply chain trade transaction."^^xsd:string ;
  rdfs:domain "mmt:SupplyChainTradeTransaction"^^xsd:string ;
  rdfs:label "information"^^xsd:string ;
  rdfs:range "xsd:string"^^xsd:string .

<https://edi3.org/mmt/vocab#SupplyChainTradeTransactionLineItemQuantity>
  a rdf:Property ;
  rdfs:comment "The number of line items for this supply chain trade transaction."^^xsd:string ;
  rdfs:domain "mmt:SupplyChainTradeTransaction"^^xsd:string ;
  rdfs:label "lineItemQuantity"^^xsd:string ;
  rdfs:range "xsd:decimal"^^xsd:string .

<https://edi3.org/mmt/vocab#SupplyChainTradeTransactionSalesAgentAssignedID>
  a rdf:Property ;
  rdfs:comment "The unique identifier assigned by the sales agent to identify this supply chain trade transaction."^^xsd:string ;
  rdfs:domain "mmt:SupplyChainTradeTransaction"^^xsd:string ;
  rdfs:label "salesAgentAssignedID"^^xsd:string ;
  rdfs:range "xsd:ID"^^xsd:string .

<https://edi3.org/mmt/vocab#SupplyChainTradeTransactionTypeCode>
  a rdf:Property ;
  rdfs:comment "The code specifying the type of supply chain trade transaction."^^xsd:string ;
  rdfs:domain "mmt:SupplyChainTradeTransaction"^^xsd:string ;
  rdfs:label "typeCode"^^xsd:string ;
  rdfs:range "xsd:token"^^xsd:string .

<https://edi3.org/mmt/vocab#TaxRegistration>
  a rdfs:Class ;
  rdfs:comment "Registration with a specific tax authority."^^xsd:string ;
  rdfs:label "TaxRegistration"^^xsd:string .

<https://edi3.org/mmt/vocab#TaxRegistrationID>
  a rdf:Property ;
  rdfs:comment "The unique identifier for this tax registration."^^xsd:string ;
  rdfs:domain "mmt:TaxRegistration"^^xsd:string ;
  rdfs:label "iD"^^xsd:string ;
  rdfs:range "xsd:ID"^^xsd:string .

<https://edi3.org/mmt/vocab#TemperatureSettingInstructions>
  a rdfs:Class ;
  rdfs:comment "Temperature setting related information of an instructive nature."^^xsd:string ;
  rdfs:label "TemperatureSettingInstructions"^^xsd:string .

<https://edi3.org/mmt/vocab#TemperatureSettingInstructionsDescription>
  a rdf:Property ;
  rdfs:comment "A textual description of these temperature setting instructions."^^xsd:string ;
  rdfs:domain "mmt:TemperatureSettingInstructions"^^xsd:string ;
  rdfs:label "description"^^xsd:string ;
  rdfs:range "xsd:string"^^xsd:string .

<https://edi3.org/mmt/vocab#TemperatureSettingInstructionsDescriptionCode>
  a rdf:Property ;
  rdfs:comment "The code specifying a description of these temperature setting instructions."^^xsd:string ;
  rdfs:domain "mmt:TemperatureSettingInstructions"^^xsd:string ;
  rdfs:label "descriptionCode"^^xsd:string ;
  rdfs:range "xsd:token"^^xsd:string .

<https://edi3.org/mmt/vocab#TemperatureSettingInstructionsProcedureText>
  a rdf:Property ;
  rdfs:comment "A procedure, expressed as text, for these temperature setting instructions."^^xsd:string ;
  rdfs:domain "mmt:TemperatureSettingInstructions"^^xsd:string ;
  rdfs:label "procedureText"^^xsd:string ;
  rdfs:range "xsd:string"^^xsd:string .

<https://edi3.org/mmt/vocab#TradeProductCertification>
  a rdfs:Class ;
  rdfs:comment "The process of certifying that a certain product has passed performance and quality assurance tests, or qualification requirements stipulated in regulations."^^xsd:string ;
  rdfs:label "TradeProductCertification"^^xsd:string .

<https://edi3.org/mmt/vocab#TradeProductCertificationAssertionCode>
  a rdf:Property ;
  rdfs:comment "A code specifying an assertion for this trade product certification, such as claims that a product is free from peanuts."^^xsd:string ;
  rdfs:domain "mmt:TradeProductCertification"^^xsd:string ;
  rdfs:label "assertionCode"^^xsd:string ;
  rdfs:range "xsd:token"^^xsd:string .

<https://edi3.org/mmt/vocab#TradeProductCertificationAssertionText>
  a rdf:Property ;
  rdfs:comment "An assertion, expressed as text, for this trade product certification, such as that this product is free from peanuts."^^xsd:string ;
  rdfs:domain "mmt:TradeProductCertification"^^xsd:string ;
  rdfs:label "assertionText"^^xsd:string ;
  rdfs:range "xsd:string"^^xsd:string .

<https://edi3.org/mmt/vocab#TradeProductCertificationResponsibleAgencyText>
  a rdf:Property ;
  rdfs:comment "The agency, expressed as text, responsible for this trade product certification."^^xsd:string ;
  rdfs:domain "mmt:TradeProductCertification"^^xsd:string ;
  rdfs:label "responsibleAgencyText"^^xsd:string ;
  rdfs:range "xsd:string"^^xsd:string .

<https://edi3.org/mmt/vocab#TradeProductCertificationStandardText>
  a rdf:Property ;
  rdfs:comment "The standard, expressed as text, for this trade product certification."^^xsd:string ;
  rdfs:domain "mmt:TradeProductCertification"^^xsd:string ;
  rdfs:label "standardText"^^xsd:string ;
  rdfs:range "xsd:string"^^xsd:string .

<https://edi3.org/mmt/vocab#TradeSettlementHeaderMonetarySummation>
  a rdfs:Class ;
  rdfs:comment "A collection of monetary amount totals, specified at header level, for a trade settlement."^^xsd:string ;
  rdfs:label "TradeSettlementHeaderMonetarySummation"^^xsd:string .

<https://edi3.org/mmt/vocab#TradeSettlementHeaderMonetarySummationAllowanceTotalAmount>
  a rdf:Property ;
  rdfs:comment "A monetary value of the total of all allowance amounts being reported in this trade settlement header monetary summation."^^xsd:string ;
  rdfs:domain "mmt:TradeSettlementHeaderMonetarySummation"^^xsd:string ;
  rdfs:label "allowanceTotalAmount"^^xsd:string ;
  rdfs:range "http://schema.org/amount"^^xsd:string .

<https://edi3.org/mmt/vocab#TradeSettlementHeaderMonetarySummationChargeTotalAmount>
  a rdf:Property ;
  rdfs:comment "A monetary value of the total of all charge amounts being reported in this trade settlement header monetary summation."^^xsd:string ;
  rdfs:domain "mmt:TradeSettlementHeaderMonetarySummation"^^xsd:string ;
  rdfs:label "chargeTotalAmount"^^xsd:string ;
  rdfs:range "http://schema.org/amount"^^xsd:string .

<https://edi3.org/mmt/vocab#TradeSettlementHeaderMonetarySummationDuePayableAmount>
  a rdf:Property ;
  rdfs:comment "A monetary value that is an amount due and payable for this trade settlement header monetary summation, such as the amount due to the creditor."^^xsd:string ;
  rdfs:domain "mmt:TradeSettlementHeaderMonetarySummation"^^xsd:string ;
  rdfs:label "duePayableAmount"^^xsd:string ;
  rdfs:range "http://schema.org/amount"^^xsd:string .

<https://edi3.org/mmt/vocab#TradeSettlementHeaderMonetarySummationGrandTotalAmount>
  a rdf:Property ;
  rdfs:comment "A monetary value of the grand total of this trade settlement header monetary summation, to include addition and subtraction of individual summation amounts."^^xsd:string ;
  rdfs:domain "mmt:TradeSettlementHeaderMonetarySummation"^^xsd:string ;
  rdfs:label "grandTotalAmount"^^xsd:string ;
  rdfs:range "http://schema.org/amount"^^xsd:string .

<https://edi3.org/mmt/vocab#TradeSettlementHeaderMonetarySummationGrossLineTotalAmount>
  a rdf:Property ;
  rdfs:comment "A monetary value of the total of all line amounts, excluding line level allowances and charges and taxes, being reported in this trade settlement header monetary summation."^^xsd:string ;
  rdfs:domain "mmt:TradeSettlementHeaderMonetarySummation"^^xsd:string ;
  rdfs:label "grossLineTotalAmount"^^xsd:string ;
  rdfs:range "http://schema.org/amount"^^xsd:string .

<https://edi3.org/mmt/vocab#TradeSettlementHeaderMonetarySummationLineTotalAmount>
  a rdf:Property ;
  rdfs:comment "A monetary value of the line amount total being reported in this trade settlement header monetary summation."^^xsd:string ;
  rdfs:domain "mmt:TradeSettlementHeaderMonetarySummation"^^xsd:string ;
  rdfs:label "lineTotalAmount"^^xsd:string ;
  rdfs:range "http://schema.org/amount"^^xsd:string .

<https://edi3.org/mmt/vocab#TradeSettlementHeaderMonetarySummationNetIncludingTaxesLineTotalAmount>
  a rdf:Property ;
  rdfs:comment "A monetary value of the total of all line amounts, including line level allowances and charges and including line level taxes, being reported in this trade settlement header monetary summation."^^xsd:string ;
  rdfs:domain "mmt:TradeSettlementHeaderMonetarySummation"^^xsd:string ;
  rdfs:label "netIncludingTaxesLineTotalAmount"^^xsd:string ;
  rdfs:range "http://schema.org/amount"^^xsd:string .

<https://edi3.org/mmt/vocab#TradeSettlementHeaderMonetarySummationNetLineTotalAmount>
  a rdf:Property ;
  rdfs:comment "A monetary value of the total of all line amounts, including line level allowances and charges and excluding line level taxes, being reported in this trade settlement header monetary summation."^^xsd:string ;
  rdfs:domain "mmt:TradeSettlementHeaderMonetarySummation"^^xsd:string ;
  rdfs:label "netLineTotalAmount"^^xsd:string ;
  rdfs:range "http://schema.org/amount"^^xsd:string .

<https://edi3.org/mmt/vocab#TradeSettlementHeaderMonetarySummationPaymentTotalAmount>
  a rdf:Property ;
  rdfs:comment "A monetary value of a payment total reported in this header trade settlement payment monetary summation."^^xsd:string ;
  rdfs:domain "mmt:TradeSettlementHeaderMonetarySummation"^^xsd:string ;
  rdfs:label "paymentTotalAmount"^^xsd:string ;
  rdfs:range "http://schema.org/amount"^^xsd:string .

<https://edi3.org/mmt/vocab#TradeSettlementHeaderMonetarySummationProductValueExcludingTobaccoTaxInformationAmount>
  a rdf:Property ;
  rdfs:comment "A monetary value which constitutes the total product value, excluding tobacco tax, stated for information purposes in this trade settlement header monetary summation."^^xsd:string ;
  rdfs:domain "mmt:TradeSettlementHeaderMonetarySummation"^^xsd:string ;
  rdfs:label "productValueExcludingTobaccoTaxInformationAmount"^^xsd:string ;
  rdfs:range "http://schema.org/amount"^^xsd:string .

<https://edi3.org/mmt/vocab#TradeSettlementHeaderMonetarySummationTaxBasisTotalAmount>
  a rdf:Property ;
  rdfs:comment "A monetary value of the total of all tax basis amounts being reported in this trade settlement monetary summation."^^xsd:string ;
  rdfs:domain "mmt:TradeSettlementHeaderMonetarySummation"^^xsd:string ;
  rdfs:label "taxBasisTotalAmount"^^xsd:string ;
  rdfs:range "http://schema.org/amount"^^xsd:string .

<https://edi3.org/mmt/vocab#TradeSettlementHeaderMonetarySummationTaxTotalAmount>
  a rdf:Property ;
  rdfs:comment "A monetary value of the total of all tax amounts being reported in this trade settlement header monetary summation."^^xsd:string ;
  rdfs:domain "mmt:TradeSettlementHeaderMonetarySummation"^^xsd:string ;
  rdfs:label "taxTotalAmount"^^xsd:string ;
  rdfs:range "http://schema.org/amount"^^xsd:string .

<https://edi3.org/mmt/vocab#TradeSettlementHeaderMonetarySummationTotalAllowanceChargeAmount>
  a rdf:Property ;
  rdfs:comment "A monetary value of a total allowance and charge reported in this trade settlement header monetary summation."^^xsd:string ;
  rdfs:domain "mmt:TradeSettlementHeaderMonetarySummation"^^xsd:string ;
  rdfs:label "totalAllowanceChargeAmount"^^xsd:string ;
  rdfs:range "http://schema.org/amount"^^xsd:string .

<https://edi3.org/mmt/vocab#TradeSettlementHeaderMonetarySummationTotalDiscountAmount>
  a rdf:Property ;
  rdfs:comment "A monetary value of a total discount reported in this trade settlement header monetary summation."^^xsd:string ;
  rdfs:domain "mmt:TradeSettlementHeaderMonetarySummation"^^xsd:string ;
  rdfs:label "totalDiscountAmount"^^xsd:string ;
  rdfs:range "http://schema.org/amount"^^xsd:string .

<https://edi3.org/mmt/vocab#TradeSettlementHeaderMonetarySummationTotalDiscountBasisAmount>
  a rdf:Property ;
  rdfs:comment "A monetary value of a total discount basis reported in this trade settlement header monetary summation."^^xsd:string ;
  rdfs:domain "mmt:TradeSettlementHeaderMonetarySummation"^^xsd:string ;
  rdfs:label "totalDiscountBasisAmount"^^xsd:string ;
  rdfs:range "http://schema.org/amount"^^xsd:string .

<https://edi3.org/mmt/vocab#TradeSettlementHeaderMonetarySummationTotalPrepaidAmount>
  a rdf:Property ;
  rdfs:comment "A monetary value of a prepaid total reported in this trade settlement header monetary summation."^^xsd:string ;
  rdfs:domain "mmt:TradeSettlementHeaderMonetarySummation"^^xsd:string ;
  rdfs:label "totalPrepaidAmount"^^xsd:string ;
  rdfs:range "http://schema.org/amount"^^xsd:string .

<https://edi3.org/mmt/vocab#TradeSettlementLineMonetarySummation>
  a rdfs:Class ;
  rdfs:comment "A collection of monetary amount totals, specified at line level, for a trade settlement."^^xsd:string ;
  rdfs:label "TradeSettlementLineMonetarySummation"^^xsd:string .

<https://edi3.org/mmt/vocab#TradeSettlementLineMonetarySummationAllowanceTotalAmount>
  a rdf:Property ;
  rdfs:comment "A monetary value of the total of all allowance amounts being reported in this trade settlement line monetary summation."^^xsd:string ;
  rdfs:domain "mmt:TradeSettlementLineMonetarySummation"^^xsd:string ;
  rdfs:label "allowanceTotalAmount"^^xsd:string ;
  rdfs:range "http://schema.org/amount"^^xsd:string .

<https://edi3.org/mmt/vocab#TradeSettlementLineMonetarySummationChargeTotalAmount>
  a rdf:Property ;
  rdfs:comment "A monetary value of the total of all charge amounts being reported in this trade settlement line monetary summation."^^xsd:string ;
  rdfs:domain "mmt:TradeSettlementLineMonetarySummation"^^xsd:string ;
  rdfs:label "chargeTotalAmount"^^xsd:string ;
  rdfs:range "http://schema.org/amount"^^xsd:string .

<https://edi3.org/mmt/vocab#TradeSettlementLineMonetarySummationDuePayableAmount>
  a rdf:Property ;
  rdfs:comment "A monetary value that is an amount due and payable for this trade settlement line monetary summation, such as the amount due to the creditor."^^xsd:string ;
  rdfs:domain "mmt:TradeSettlementLineMonetarySummation"^^xsd:string ;
  rdfs:label "duePayableAmount"^^xsd:string ;
  rdfs:range "http://schema.org/amount"^^xsd:string .

<https://edi3.org/mmt/vocab#TradeSettlementLineMonetarySummationGrandTotalAmount>
  a rdf:Property ;
  rdfs:comment "A monetary value of the grand total of this trade settlement line monetary summation, to include addition and subtraction of individual summation amounts."^^xsd:string ;
  rdfs:domain "mmt:TradeSettlementLineMonetarySummation"^^xsd:string ;
  rdfs:label "grandTotalAmount"^^xsd:string ;
  rdfs:range "http://schema.org/amount"^^xsd:string .

<https://edi3.org/mmt/vocab#TradeSettlementLineMonetarySummationGrossLineTotalAmount>
  a rdf:Property ;
  rdfs:comment "A monetary value of the total of all line amounts, excluding line level allowances and charges and taxes, being reported in this trade settlement line monetary summation."^^xsd:string ;
  rdfs:domain "mmt:TradeSettlementLineMonetarySummation"^^xsd:string ;
  rdfs:label "grossLineTotalAmount"^^xsd:string ;
  rdfs:range "http://schema.org/amount"^^xsd:string .

<https://edi3.org/mmt/vocab#TradeSettlementLineMonetarySummationLineTotalAmount>
  a rdf:Property ;
  rdfs:comment "A monetary value of the line amount total being reported in this trade settlement line monetary summation."^^xsd:string ;
  rdfs:domain "mmt:TradeSettlementLineMonetarySummation"^^xsd:string ;
  rdfs:label "lineTotalAmount"^^xsd:string ;
  rdfs:range "http://schema.org/amount"^^xsd:string .

<https://edi3.org/mmt/vocab#TradeSettlementLineMonetarySummationNetIncludingTaxesLineTotalAmount>
  a rdf:Property ;
  rdfs:comment "A monetary value of the total of all line amounts, including line level allowances and charges and including line level taxes, being reported in this trade settlement line monetary summation."^^xsd:string ;
  rdfs:domain "mmt:TradeSettlementLineMonetarySummation"^^xsd:string ;
  rdfs:label "netIncludingTaxesLineTotalAmount"^^xsd:string ;
  rdfs:range "http://schema.org/amount"^^xsd:string .

<https://edi3.org/mmt/vocab#TradeSettlementLineMonetarySummationNetLineTotalAmount>
  a rdf:Property ;
  rdfs:comment "A monetary value of the total of all line amounts, including line level allowances and charges and excluding line level taxes, being reported in this trade settlement line monetary summation."^^xsd:string ;
  rdfs:domain "mmt:TradeSettlementLineMonetarySummation"^^xsd:string ;
  rdfs:label "netLineTotalAmount"^^xsd:string ;
  rdfs:range "http://schema.org/amount"^^xsd:string .

<https://edi3.org/mmt/vocab#TradeSettlementLineMonetarySummationPaymentTotalAmount>
  a rdf:Property ;
  rdfs:comment "A monetary value of a payment total reported in this trade settlement line monetary summation."^^xsd:string ;
  rdfs:domain "mmt:TradeSettlementLineMonetarySummation"^^xsd:string ;
  rdfs:label "paymentTotalAmount"^^xsd:string ;
  rdfs:range "http://schema.org/amount"^^xsd:string .

<https://edi3.org/mmt/vocab#TradeSettlementLineMonetarySummationTaxBasisTotalAmount>
  a rdf:Property ;
  rdfs:comment "A monetary value of the total of all tax basis amounts being reported in this trade settlement line monetary summation."^^xsd:string ;
  rdfs:domain "mmt:TradeSettlementLineMonetarySummation"^^xsd:string ;
  rdfs:label "taxBasisTotalAmount"^^xsd:string ;
  rdfs:range "http://schema.org/amount"^^xsd:string .

<https://edi3.org/mmt/vocab#TradeSettlementLineMonetarySummationTaxTotalAmount>
  a rdf:Property ;
  rdfs:comment "A monetary value of the total of all tax amounts being reported in this trade settlement line monetary summation."^^xsd:string ;
  rdfs:domain "mmt:TradeSettlementLineMonetarySummation"^^xsd:string ;
  rdfs:label "taxTotalAmount"^^xsd:string ;
  rdfs:range "http://schema.org/amount"^^xsd:string .

<https://edi3.org/mmt/vocab#TradeSettlementLineMonetarySummationTotalAllowanceChargeAmount>
  a rdf:Property ;
  rdfs:comment "A monetary value of a total allowance and charge reported in this trade settlement line monetary summation."^^xsd:string ;
  rdfs:domain "mmt:TradeSettlementLineMonetarySummation"^^xsd:string ;
  rdfs:label "totalAllowanceChargeAmount"^^xsd:string ;
  rdfs:range "http://schema.org/amount"^^xsd:string .

<https://edi3.org/mmt/vocab#TradeSettlementPaymentMeans>
  a rdfs:Class ;
  rdfs:comment "The means by which a payment will be or has been made for trade settlement purposes."^^xsd:string ;
  rdfs:label "TradeSettlementPaymentMeans"^^xsd:string .

<https://edi3.org/mmt/vocab#TradeSettlementPaymentMeansGuaranteeMethodCode>
  a rdf:Property ;
  rdfs:comment "The code specifying the method of guarantee for this trade settlement payment means."^^xsd:string ;
  rdfs:domain "mmt:TradeSettlementPaymentMeans"^^xsd:string ;
  rdfs:label "guaranteeMethodCode"^^xsd:string ;
  rdfs:range "PaymentGuaranteeMeansType_Сode"^^xsd:string .

<https://edi3.org/mmt/vocab#TradeSettlementPaymentMeansPaymentChannelCode>
  a rdf:Property ;
  rdfs:comment "The code specifying the payment channel through which this trade settlement payment is to be processed (Reference United Nations Code List (UNCL) 4435)."^^xsd:string ;
  rdfs:domain "mmt:TradeSettlementPaymentMeans"^^xsd:string ;
  rdfs:label "paymentChannelCode"^^xsd:string ;
  rdfs:range "PaymentMeansChannelType_Сode"^^xsd:string .

<https://edi3.org/mmt/vocab#TradeSettlementPaymentMeansPaymentMethodCode>
  a rdf:Property ;
  rdfs:comment "The code specifying the method by which a payment may be made for this trade settlement payment means."^^xsd:string ;
  rdfs:domain "mmt:TradeSettlementPaymentMeans"^^xsd:string ;
  rdfs:label "paymentMethodCode"^^xsd:string ;
  rdfs:range "xsd:token"^^xsd:string .

<https://edi3.org/mmt/vocab#TradeSettlementPaymentMeansTypeCode>
  a rdf:Property ;
  rdfs:comment "The code specifying the type of trade settlement payment means, such as cash or check."^^xsd:string ;
  rdfs:domain "mmt:TradeSettlementPaymentMeans"^^xsd:string ;
  rdfs:label "typeCode"^^xsd:string ;
  rdfs:range "PaymentMeansType_Сode"^^xsd:string .

<https://edi3.org/mmt/vocab#TradeAddress>
  a rdfs:Class ;
  rdfs:comment "The location at which a particular trade related organization or person may be found or reached."^^xsd:string ;
  rdfs:label "TradeAddress"^^xsd:string .

<https://edi3.org/mmt/vocab#TradeAddressCityName>
  a rdf:Property ;
  rdfs:comment "The name, expressed as text, of the city, town or village of this trade address."^^xsd:string ;
  rdfs:domain "mmt:TradeAddress"^^xsd:string ;
  rdfs:label "cityName"^^xsd:string ;
  rdfs:range "xsd:string"^^xsd:string .

<https://edi3.org/mmt/vocab#TradeAddressCountryCode>
  a rdf:Property ;
  rdfs:comment "The unique identifier of a country for this trade address."^^xsd:string ;
  rdfs:domain "mmt:TradeAddress"^^xsd:string ;
  rdfs:label "countryCode"^^xsd:string ;
  rdfs:range "ISO3166_Code"^^xsd:string .

<https://edi3.org/mmt/vocab#TradeAddressCountryName>
  a rdf:Property ;
  rdfs:comment "A name, expressed as text, of the country for this trade address."^^xsd:string ;
  rdfs:domain "mmt:TradeAddress"^^xsd:string ;
  rdfs:label "countryName"^^xsd:string ;
  rdfs:range "xsd:string"^^xsd:string .

<https://edi3.org/mmt/vocab#TradeAddressCountrySubDivisionName>
  a rdf:Property ;
  rdfs:comment "A name, expressed as text, of the sub-division of a country for this trade address."^^xsd:string ;
  rdfs:domain "mmt:TradeAddress"^^xsd:string ;
  rdfs:label "countrySubDivisionName"^^xsd:string ;
  rdfs:range "xsd:string"^^xsd:string .

<https://edi3.org/mmt/vocab#TradeAddressID>
  a rdf:Property ;
  rdfs:comment "A unique identifier for this trade address."^^xsd:string ;
  rdfs:domain "mmt:TradeAddress"^^xsd:string ;
  rdfs:label "iD"^^xsd:string ;
  rdfs:range "xsd:ID"^^xsd:string .

<https://edi3.org/mmt/vocab#TradeAddressPostcode>
  a rdf:Property ;
  rdfs:comment "A code specifying the postcode of this trade address."^^xsd:string ;
  rdfs:domain "mmt:TradeAddress"^^xsd:string ;
  rdfs:label "postcode"^^xsd:string ;
  rdfs:range "xsd:token"^^xsd:string .

<https://edi3.org/mmt/vocab#TradeAddressStreetName>
  a rdf:Property ;
  rdfs:comment "A name, expressed as text, of a street or thoroughfare for this trade address."^^xsd:string ;
  rdfs:domain "mmt:TradeAddress"^^xsd:string ;
  rdfs:label "streetName"^^xsd:string ;
  rdfs:range "xsd:string"^^xsd:string .

<https://edi3.org/mmt/vocab#TradeAllowanceCharge>
  a rdfs:Class ;
  rdfs:comment "A component of pricing, such as an allowance or charge for trade purposes."^^xsd:string ;
  rdfs:label "TradeAllowanceCharge"^^xsd:string .

<https://edi3.org/mmt/vocab#TradeAllowanceChargeActualAmount>
  a rdf:Property ;
  rdfs:comment "An actual monetary value of the trade allowance charge."^^xsd:string ;
  rdfs:domain "mmt:TradeAllowanceCharge"^^xsd:string ;
  rdfs:label "actualAmount"^^xsd:string ;
  rdfs:range "http://schema.org/amount"^^xsd:string .

<https://edi3.org/mmt/vocab#TradeAllowanceChargeBasisAmount>
  a rdf:Property ;
  rdfs:comment "The monetary value that is the basis on which this trade allowance charge is calculated."^^xsd:string ;
  rdfs:domain "mmt:TradeAllowanceCharge"^^xsd:string ;
  rdfs:label "basisAmount"^^xsd:string ;
  rdfs:range "http://schema.org/amount"^^xsd:string .

<https://edi3.org/mmt/vocab#TradeAllowanceChargeBasisQuantity>
  a rdf:Property ;
  rdfs:comment "The quantity on which this trade allowance charge is based."^^xsd:string ;
  rdfs:domain "mmt:TradeAllowanceCharge"^^xsd:string ;
  rdfs:label "basisQuantity"^^xsd:string ;
  rdfs:range "xsd:decimal"^^xsd:string .

<https://edi3.org/mmt/vocab#TradeAllowanceChargeCalculationPercent>
  a rdf:Property ;
  rdfs:comment "The percentage applied to calculate this trade allowance charge."^^xsd:string ;
  rdfs:domain "mmt:TradeAllowanceCharge"^^xsd:string ;
  rdfs:label "calculationPercent"^^xsd:string ;
  rdfs:range "xsd:decimal"^^xsd:string .

<https://edi3.org/mmt/vocab#TradeAllowanceChargeChargeIndicator>
  a rdf:Property ;
  rdfs:comment "The indication of whether or not the trade allowance charge is a charge."^^xsd:string ;
  rdfs:domain "mmt:TradeAllowanceCharge"^^xsd:string ;
  rdfs:label "chargeIndicator"^^xsd:string ;
  rdfs:range "xsd:boolean"^^xsd:string .

<https://edi3.org/mmt/vocab#TradeAllowanceChargePrepaidIndicator>
  a rdf:Property ;
  rdfs:comment "The indication of whether or not this trade allowance charge is prepaid."^^xsd:string ;
  rdfs:domain "mmt:TradeAllowanceCharge"^^xsd:string ;
  rdfs:label "prepaidIndicator"^^xsd:string ;
  rdfs:range "xsd:boolean"^^xsd:string .

<https://edi3.org/mmt/vocab#TradeAllowanceChargeReasonCode>
  a rdf:Property ;
  rdfs:comment "The code specifying the reason for this trade allowance charge."^^xsd:string ;
  rdfs:domain "mmt:TradeAllowanceCharge"^^xsd:string ;
  rdfs:label "reasonCode"^^xsd:string ;
  rdfs:range "AllowanceChargeReasonType_Сode"^^xsd:string .

<https://edi3.org/mmt/vocab#TradeAllowanceChargeTypeCode>
  a rdf:Property ;
  rdfs:comment "The code specifying the type of this trade allowance charge."^^xsd:string ;
  rdfs:domain "mmt:TradeAllowanceCharge"^^xsd:string ;
  rdfs:label "typeCode"^^xsd:string ;
  rdfs:range "AllowanceChargeIdentificationType_Сode"^^xsd:string .

<https://edi3.org/mmt/vocab#TradeAllowanceChargeUnitBasisAmount>
  a rdf:Property ;
  rdfs:comment "The monetary value of the unit basis on which the allowance or charge is calculated."^^xsd:string ;
  rdfs:domain "mmt:TradeAllowanceCharge"^^xsd:string ;
  rdfs:label "unitBasisAmount"^^xsd:string ;
  rdfs:range "http://schema.org/amount"^^xsd:string .

<https://edi3.org/mmt/vocab#TradeContact>
  a rdfs:Class ;
  rdfs:comment "A person or a department that acts as a point of contact with another person or department in a trading relationship."^^xsd:string ;
  rdfs:label "TradeContact"^^xsd:string .

<https://edi3.org/mmt/vocab#TradeContactDepartmentName>
  a rdf:Property ;
  rdfs:comment "The name, expressed as text, of the department to which this trade contact belongs within an organization."^^xsd:string ;
  rdfs:domain "mmt:TradeContact"^^xsd:string ;
  rdfs:label "departmentName"^^xsd:string ;
  rdfs:range "xsd:string"^^xsd:string .

<https://edi3.org/mmt/vocab#TradeContactID>
  a rdf:Property ;
  rdfs:comment "The unique identifier for this trade contact."^^xsd:string ;
  rdfs:domain "mmt:TradeContact"^^xsd:string ;
  rdfs:label "iD"^^xsd:string ;
  rdfs:range "xsd:ID"^^xsd:string .

<https://edi3.org/mmt/vocab#TradeContactPersonName>
  a rdf:Property ;
  rdfs:comment "The name, expressed as text, of this trade contact person."^^xsd:string ;
  rdfs:domain "mmt:TradeContact"^^xsd:string ;
  rdfs:label "personName"^^xsd:string ;
  rdfs:range "xsd:string"^^xsd:string .

<https://edi3.org/mmt/vocab#TradeContactTypeCode>
  a rdf:Property ;
  rdfs:comment "The code specifying the type of trade contact."^^xsd:string ;
  rdfs:domain "mmt:TradeContact"^^xsd:string ;
  rdfs:label "typeCode"^^xsd:string ;
  rdfs:range "ContactFunctionType_Сode"^^xsd:string .

<https://edi3.org/mmt/vocab#TradeCountry>
  a rdfs:Class ;
  rdfs:comment "The area of land that belongs to a nation together with its properties, such as population, political organization, etc., used or referenced for trade purposes."^^xsd:string ;
  rdfs:label "TradeCountry"^^xsd:string .

<https://edi3.org/mmt/vocab#TradeCountryCode>
  a rdf:Property ;
  rdfs:comment "A unique identifier for this trade country."^^xsd:string ;
  rdfs:domain "mmt:TradeCountry"^^xsd:string ;
  rdfs:label "code"^^xsd:string ;
  rdfs:range "ISO3166_Code"^^xsd:string .

<https://edi3.org/mmt/vocab#TradeCountryName>
  a rdf:Property ;
  rdfs:comment "A name, expressed as text, of this trade country."^^xsd:string ;
  rdfs:domain "mmt:TradeCountry"^^xsd:string ;
  rdfs:label "name"^^xsd:string ;
  rdfs:range "xsd:string"^^xsd:string .

<https://edi3.org/mmt/vocab#TradeCountrySubDivision>
  a rdfs:Class ;
  rdfs:comment "A political or physical area or region within the political boundaries of a country used or referenced for trade purposes."^^xsd:string ;
  rdfs:label "TradeCountrySubDivision"^^xsd:string .

<https://edi3.org/mmt/vocab#TradeCountrySubDivisionID>
  a rdf:Property ;
  rdfs:comment "The unique identifier for this trade country sub-division."^^xsd:string ;
  rdfs:domain "mmt:TradeCountrySubDivision"^^xsd:string ;
  rdfs:label "iD"^^xsd:string ;
  rdfs:range "xsd:ID"^^xsd:string .

<https://edi3.org/mmt/vocab#TradeCountrySubDivisionName>
  a rdf:Property ;
  rdfs:comment "A name, expressed as text, of this trade country sub-division."^^xsd:string ;
  rdfs:domain "mmt:TradeCountrySubDivision"^^xsd:string ;
  rdfs:label "name"^^xsd:string ;
  rdfs:range "xsd:string"^^xsd:string .

<https://edi3.org/mmt/vocab#TradeCurrencyExchange>
  a rdfs:Class ;
  rdfs:comment "The conversion of one currency to another for trade purposes."^^xsd:string ;
  rdfs:label "TradeCurrencyExchange"^^xsd:string .

<https://edi3.org/mmt/vocab#TradeCurrencyExchangeConversionRate>
  a rdf:Property ;
  rdfs:comment "The rate factor used for conversion from the source currency to the target currency for trade purposes."^^xsd:string ;
  rdfs:domain "mmt:TradeCurrencyExchange"^^xsd:string ;
  rdfs:label "conversionRate"^^xsd:string ;
  rdfs:range "xsd:decimal"^^xsd:string .

<https://edi3.org/mmt/vocab#TradeCurrencyExchangeSourceCurrencyCode>
  a rdf:Property ;
  rdfs:comment "The code specifying the source currency of a trade related currency conversion."^^xsd:string ;
  rdfs:domain "mmt:TradeCurrencyExchange"^^xsd:string ;
  rdfs:label "sourceCurrencyCode"^^xsd:string ;
  rdfs:range "ISO4217_Code"^^xsd:string .

<https://edi3.org/mmt/vocab#TradeCurrencyExchangeTargetCurrencyCode>
  a rdf:Property ;
  rdfs:comment "The code specifying the target currency of a trade related currency conversion."^^xsd:string ;
  rdfs:domain "mmt:TradeCurrencyExchange"^^xsd:string ;
  rdfs:label "targetCurrencyCode"^^xsd:string ;
  rdfs:range "ISO4217_Code"^^xsd:string .

<https://edi3.org/mmt/vocab#TradeDeliveryTerms>
  a rdfs:Class ;
  rdfs:comment "Conditions agreed upon between the parties with regard to the delivery of goods and or services for trade purposes."^^xsd:string ;
  rdfs:label "TradeDeliveryTerms"^^xsd:string .

<https://edi3.org/mmt/vocab#TradeDeliveryTermsCode>
  a rdf:Property ;
  rdfs:comment "The code specifying the type of delivery for these trade delivery terms."^^xsd:string ;
  rdfs:domain "mmt:TradeDeliveryTerms"^^xsd:string ;
  rdfs:label "code"^^xsd:string ;
  rdfs:range "DeliveryTermsType_Сode"^^xsd:string .

<https://edi3.org/mmt/vocab#TradeDeliveryTermsDescription>
  a rdf:Property ;
  rdfs:comment "A textual description of these trade delivery terms."^^xsd:string ;
  rdfs:domain "mmt:TradeDeliveryTerms"^^xsd:string ;
  rdfs:label "description"^^xsd:string ;
  rdfs:range "xsd:string"^^xsd:string .

<https://edi3.org/mmt/vocab#TradeDeliveryTermsFunctionCode>
  a rdf:Property ;
  rdfs:comment "A code specifying a function of these trade delivery terms."^^xsd:string ;
  rdfs:domain "mmt:TradeDeliveryTerms"^^xsd:string ;
  rdfs:label "functionCode"^^xsd:string ;
  rdfs:range "DeliveryTermsFunctionType_Сode"^^xsd:string .

<https://edi3.org/mmt/vocab#TradeGeopoliticalRegion>
  a rdfs:Class ;
  rdfs:comment "A collection of countries and/or economies united for trade purposes."^^xsd:string ;
  rdfs:label "TradeGeopoliticalRegion"^^xsd:string .

<https://edi3.org/mmt/vocab#TradeGeopoliticalRegionID>
  a rdf:Property ;
  rdfs:comment "The unique identifier for this trade geopolitical region."^^xsd:string ;
  rdfs:domain "mmt:TradeGeopoliticalRegion"^^xsd:string ;
  rdfs:label "iD"^^xsd:string ;
  rdfs:range "xsd:ID"^^xsd:string .

<https://edi3.org/mmt/vocab#TradeGeopoliticalRegionName>
  a rdf:Property ;
  rdfs:comment "The name, expressed as text, of this trade geopolitical region."^^xsd:string ;
  rdfs:domain "mmt:TradeGeopoliticalRegion"^^xsd:string ;
  rdfs:label "name"^^xsd:string ;
  rdfs:range "xsd:string"^^xsd:string .

<https://edi3.org/mmt/vocab#TradeGeopoliticalRegionTypeCode>
  a rdf:Property ;
  rdfs:comment "The code specifying the type of trade geopolitical region."^^xsd:string ;
  rdfs:domain "mmt:TradeGeopoliticalRegion"^^xsd:string ;
  rdfs:label "typeCode"^^xsd:string ;
  rdfs:range "xsd:token"^^xsd:string .

<https://edi3.org/mmt/vocab#TradeLocation>
  a rdfs:Class ;
  rdfs:comment "A physical location or place used or referenced for trade purposes."^^xsd:string ;
  rdfs:label "TradeLocation"^^xsd:string .

<https://edi3.org/mmt/vocab#TradeLocationID>
  a rdf:Property ;
  rdfs:comment "The unique identifier for this location used or referenced in trade."^^xsd:string ;
  rdfs:domain "mmt:TradeLocation"^^xsd:string ;
  rdfs:label "iD"^^xsd:string ;
  rdfs:range "xsd:ID"^^xsd:string .

<https://edi3.org/mmt/vocab#TradeLocationName>
  a rdf:Property ;
  rdfs:comment "The name, expressed as text, of this location used or referenced in trade."^^xsd:string ;
  rdfs:domain "mmt:TradeLocation"^^xsd:string ;
  rdfs:label "name"^^xsd:string ;
  rdfs:range "xsd:string"^^xsd:string .

<https://edi3.org/mmt/vocab#TradeParty>
  a rdfs:Class ;
  rdfs:comment "An individual, a group, or a body having a role in a trade business function."^^xsd:string ;
  rdfs:label "TradeParty"^^xsd:string .

<https://edi3.org/mmt/vocab#TradePartyID>
  a rdf:Property ;
  rdfs:comment "A unique identifier of this trade party."^^xsd:string ;
  rdfs:domain "mmt:TradeParty"^^xsd:string ;
  rdfs:label "iD"^^xsd:string ;
  rdfs:range "xsd:ID"^^xsd:string .

<https://edi3.org/mmt/vocab#TradePartyLanguageCode>
  a rdf:Property ;
  rdfs:comment "A code specifying a language for this trade party."^^xsd:string ;
  rdfs:domain "mmt:TradeParty"^^xsd:string ;
  rdfs:label "languageCode"^^xsd:string ;
  rdfs:range "ISO639_Code"^^xsd:string .

<https://edi3.org/mmt/vocab#TradePartyName>
  a rdf:Property ;
  rdfs:comment "The name, expressed as text, for this trade party."^^xsd:string ;
  rdfs:domain "mmt:TradeParty"^^xsd:string ;
  rdfs:label "name"^^xsd:string ;
  rdfs:range "xsd:string"^^xsd:string .

<https://edi3.org/mmt/vocab#TradePartyQualityAssuranceIndicator>
  a rdf:Property ;
  rdfs:comment "The indication of whether or not this trade party is quality assured."^^xsd:string ;
  rdfs:domain "mmt:TradeParty"^^xsd:string ;
  rdfs:label "qualityAssuranceIndicator"^^xsd:string ;
  rdfs:range "xsd:boolean"^^xsd:string .

<https://edi3.org/mmt/vocab#TradePartyRoleCode>
  a rdf:Property ;
  rdfs:comment "A code specifying the role of this trade party."^^xsd:string ;
  rdfs:domain "mmt:TradeParty"^^xsd:string ;
  rdfs:label "roleCode"^^xsd:string ;
  rdfs:range "PartyRoleType_Сode"^^xsd:string .

<https://edi3.org/mmt/vocab#TradePaymentDiscountTerms>
  a rdfs:Class ;
  rdfs:comment "Trade terms and conditions by which a discount is or can be applied to a payable amount."^^xsd:string ;
  rdfs:label "TradePaymentDiscountTerms"^^xsd:string .

<https://edi3.org/mmt/vocab#TradePaymentDiscountTermsActualDiscountAmount>
  a rdf:Property ;
  rdfs:comment "A monetary value of the actual discount in these trade payment discount terms."^^xsd:string ;
  rdfs:domain "mmt:TradePaymentDiscountTerms"^^xsd:string ;
  rdfs:label "actualDiscountAmount"^^xsd:string ;
  rdfs:range "http://schema.org/amount"^^xsd:string .

<https://edi3.org/mmt/vocab#TradePaymentDiscountTermsBasisAmount>
  a rdf:Property ;
  rdfs:comment "A monetary value used as a basis to calculate the discount in these trade payment discount terms."^^xsd:string ;
  rdfs:domain "mmt:TradePaymentDiscountTerms"^^xsd:string ;
  rdfs:label "basisAmount"^^xsd:string ;
  rdfs:range "http://schema.org/amount"^^xsd:string .

<https://edi3.org/mmt/vocab#TradePaymentDiscountTermsBasisDateTime>
  a rdf:Property ;
  rdfs:comment "The date, time, date time, or other date time value used as the basis to calculate the discount in the trade payment discount terms."^^xsd:string ;
  rdfs:domain "mmt:TradePaymentDiscountTerms"^^xsd:string ;
  rdfs:label "basisDateTime"^^xsd:string ;
  rdfs:range "xsd:datetime"^^xsd:string .

<https://edi3.org/mmt/vocab#TradePaymentDiscountTermsBasisPeriodMeasure>
  a rdf:Property ;
  rdfs:comment "The measure of the basis period for these trade payment discount terms."^^xsd:string ;
  rdfs:domain "mmt:TradePaymentDiscountTerms"^^xsd:string ;
  rdfs:label "basisPeriodMeasure"^^xsd:string ;
  rdfs:range "xsd:decimal"^^xsd:string .

<https://edi3.org/mmt/vocab#TradePaymentDiscountTermsCalculationPercent>
  a rdf:Property ;
  rdfs:comment "The percent used to calculate the discount in these trade payment discount terms."^^xsd:string ;
  rdfs:domain "mmt:TradePaymentDiscountTerms"^^xsd:string ;
  rdfs:label "calculationPercent"^^xsd:string ;
  rdfs:range "xsd:decimal"^^xsd:string .

<https://edi3.org/mmt/vocab#TradePaymentPenaltyTerms>
  a rdfs:Class ;
  rdfs:comment "Trade terms and conditions by which a penalty is or can be applied to a payable amount."^^xsd:string ;
  rdfs:label "TradePaymentPenaltyTerms"^^xsd:string .

<https://edi3.org/mmt/vocab#TradePaymentPenaltyTermsActualPenaltyAmount>
  a rdf:Property ;
  rdfs:comment "A monetary value of the actual penalty in these trade payment penalty terms."^^xsd:string ;
  rdfs:domain "mmt:TradePaymentPenaltyTerms"^^xsd:string ;
  rdfs:label "actualPenaltyAmount"^^xsd:string ;
  rdfs:range "http://schema.org/amount"^^xsd:string .

<https://edi3.org/mmt/vocab#TradePaymentPenaltyTermsBasisAmount>
  a rdf:Property ;
  rdfs:comment "A monetary value used as a basis to calculate these trade payment penalty terms."^^xsd:string ;
  rdfs:domain "mmt:TradePaymentPenaltyTerms"^^xsd:string ;
  rdfs:label "basisAmount"^^xsd:string ;
  rdfs:range "http://schema.org/amount"^^xsd:string .

<https://edi3.org/mmt/vocab#TradePaymentPenaltyTermsBasisDateTime>
  a rdf:Property ;
  rdfs:comment "The date, time, date time, or other date time value used as the basis to calculate these trade payment penalty terms."^^xsd:string ;
  rdfs:domain "mmt:TradePaymentPenaltyTerms"^^xsd:string ;
  rdfs:label "basisDateTime"^^xsd:string ;
  rdfs:range "xsd:datetime"^^xsd:string .

<https://edi3.org/mmt/vocab#TradePaymentPenaltyTermsBasisPeriodMeasure>
  a rdf:Property ;
  rdfs:comment "The measure of the period used as a basis to calculate these trade payment penalty terms."^^xsd:string ;
  rdfs:domain "mmt:TradePaymentPenaltyTerms"^^xsd:string ;
  rdfs:label "basisPeriodMeasure"^^xsd:string ;
  rdfs:range "xsd:decimal"^^xsd:string .

<https://edi3.org/mmt/vocab#TradePaymentPenaltyTermsCalculationPercent>
  a rdf:Property ;
  rdfs:comment "The percent applied to calculate these trade payment penalty terms."^^xsd:string ;
  rdfs:domain "mmt:TradePaymentPenaltyTerms"^^xsd:string ;
  rdfs:label "calculationPercent"^^xsd:string ;
  rdfs:range "xsd:decimal"^^xsd:string .

<https://edi3.org/mmt/vocab#TradePaymentTerms>
  a rdfs:Class ;
  rdfs:comment "Terms and conditions by which payment has been or will be made for trade purposes."^^xsd:string ;
  rdfs:label "TradePaymentTerms"^^xsd:string .

<https://edi3.org/mmt/vocab#TradePaymentTermsDeprecatedDueDateDateTime>
  a rdf:Property ;
  rdfs:comment "The date, time, date time, or other date time value for a due date specified by these trade payment terms."^^xsd:string ;
  rdfs:domain "mmt:TradePaymentTerms"^^xsd:string ;
  rdfs:label "deprecatedDueDateDateTime"^^xsd:string ;
  rdfs:range "xsd:datetime"^^xsd:string .

<https://edi3.org/mmt/vocab#TradePaymentTermsDescription>
  a rdf:Property ;
  rdfs:comment "A textual description of these trade payment terms."^^xsd:string ;
  rdfs:domain "mmt:TradePaymentTerms"^^xsd:string ;
  rdfs:label "description"^^xsd:string ;
  rdfs:range "xsd:string"^^xsd:string .

<https://edi3.org/mmt/vocab#TradePaymentTermsDueDateTime>
  a rdf:Property ;
  rdfs:comment "The date, time, date time, or other date time value of the due date specified by these trade payment terms."^^xsd:string ;
  rdfs:domain "mmt:TradePaymentTerms"^^xsd:string ;
  rdfs:label "dueDateTime"^^xsd:string ;
  rdfs:range "xsd:datetime"^^xsd:string .

<https://edi3.org/mmt/vocab#TradePaymentTermsInstructionCode>
  a rdf:Property ;
  rdfs:comment "A code specifying an instruction for these trade payment terms."^^xsd:string ;
  rdfs:domain "mmt:TradePaymentTerms"^^xsd:string ;
  rdfs:label "instructionCode"^^xsd:string ;
  rdfs:range "xsd:token"^^xsd:string .

<https://edi3.org/mmt/vocab#TradePaymentTermsSettlementPeriodMeasure>
  a rdf:Property ;
  rdfs:comment "The measure of the number of settlement periods from this trade payment term time reference to the latest payment date, such as 30 days, 3 months."^^xsd:string ;
  rdfs:domain "mmt:TradePaymentTerms"^^xsd:string ;
  rdfs:label "settlementPeriodMeasure"^^xsd:string ;
  rdfs:range "xsd:decimal"^^xsd:string .

<https://edi3.org/mmt/vocab#TradePaymentTermsTypeCode>
  a rdf:Property ;
  rdfs:comment "A code specifying the type of trade payment terms."^^xsd:string ;
  rdfs:domain "mmt:TradePaymentTerms"^^xsd:string ;
  rdfs:label "typeCode"^^xsd:string ;
  rdfs:range "PaymentTermsType_Сode"^^xsd:string .

<https://edi3.org/mmt/vocab#TradePrice>
  a rdfs:Class ;
  rdfs:comment "A sum of money for which something is or may be bought or sold for trade purposes."^^xsd:string ;
  rdfs:label "TradePrice"^^xsd:string .

<https://edi3.org/mmt/vocab#TradePriceBasisQuantity>
  a rdf:Property ;
  rdfs:comment "The quantity on which the trade price is based."^^xsd:string ;
  rdfs:domain "mmt:TradePrice"^^xsd:string ;
  rdfs:label "basisQuantity"^^xsd:string ;
  rdfs:range "xsd:decimal"^^xsd:string .

<https://edi3.org/mmt/vocab#TradePriceChargeAmount>
  a rdf:Property ;
  rdfs:comment "A monetary value of the trade price charge."^^xsd:string ;
  rdfs:domain "mmt:TradePrice"^^xsd:string ;
  rdfs:label "chargeAmount"^^xsd:string ;
  rdfs:range "http://schema.org/amount"^^xsd:string .

<https://edi3.org/mmt/vocab#TradePriceTypeCode>
  a rdf:Property ;
  rdfs:comment "The code specifying the type of trade price."^^xsd:string ;
  rdfs:domain "mmt:TradePrice"^^xsd:string ;
  rdfs:label "typeCode"^^xsd:string ;
  rdfs:range "PriceType_Сode"^^xsd:string .

<https://edi3.org/mmt/vocab#TradePriceUnitAmount>
  a rdf:Property ;
  rdfs:comment "A monetary value of the unit of this trade price."^^xsd:string ;
  rdfs:domain "mmt:TradePrice"^^xsd:string ;
  rdfs:label "unitAmount"^^xsd:string ;
  rdfs:range "http://schema.org/amount"^^xsd:string .

<https://edi3.org/mmt/vocab#TradeProduct>
  a rdfs:Class ;
  rdfs:comment "Any tangible output or service produced by human or mechanical effort or by a natural process for trade purposes."^^xsd:string ;
  rdfs:label "TradeProduct"^^xsd:string .

<https://edi3.org/mmt/vocab#TradeProductBatchID>
  a rdf:Property ;
  rdfs:comment "A batch identifier for this trade product."^^xsd:string ;
  rdfs:domain "mmt:TradeProduct"^^xsd:string ;
  rdfs:label "batchID"^^xsd:string ;
  rdfs:range "xsd:ID"^^xsd:string .

<https://edi3.org/mmt/vocab#TradeProductBrandName>
  a rdf:Property ;
  rdfs:comment "The brand name, expressed as text, for this trade product."^^xsd:string ;
  rdfs:domain "mmt:TradeProduct"^^xsd:string ;
  rdfs:label "brandName"^^xsd:string ;
  rdfs:range "xsd:string"^^xsd:string .

<https://edi3.org/mmt/vocab#TradeProductBrandRangeName>
  a rdf:Property ;
  rdfs:comment "The brand range name, expressed as text, for this trade product."^^xsd:string ;
  rdfs:domain "mmt:TradeProduct"^^xsd:string ;
  rdfs:label "brandRangeName"^^xsd:string ;
  rdfs:range "xsd:string"^^xsd:string .

<https://edi3.org/mmt/vocab#TradeProductColourCode>
  a rdf:Property ;
  rdfs:comment "The code specifying the colour for this trade product."^^xsd:string ;
  rdfs:domain "mmt:TradeProduct"^^xsd:string ;
  rdfs:label "colourCode"^^xsd:string ;
  rdfs:range "xsd:token"^^xsd:string .

<https://edi3.org/mmt/vocab#TradeProductColourDescription>
  a rdf:Property ;
  rdfs:comment "A textual description of the colour of this trade product."^^xsd:string ;
  rdfs:domain "mmt:TradeProduct"^^xsd:string ;
  rdfs:label "colourDescription"^^xsd:string ;
  rdfs:range "xsd:string"^^xsd:string .

<https://edi3.org/mmt/vocab#TradeProductCommonName>
  a rdf:Property ;
  rdfs:comment "A common name, expressed as text, for this trade product."^^xsd:string ;
  rdfs:domain "mmt:TradeProduct"^^xsd:string ;
  rdfs:label "commonName"^^xsd:string ;
  rdfs:range "xsd:string"^^xsd:string .

<https://edi3.org/mmt/vocab#TradeProductConciseDescription>
  a rdf:Property ;
  rdfs:comment "A concise textual description for this trade product, such as the description used on a shelf or printed on a receipt."^^xsd:string ;
  rdfs:domain "mmt:TradeProduct"^^xsd:string ;
  rdfs:label "conciseDescription"^^xsd:string ;
  rdfs:range "xsd:string"^^xsd:string .

<https://edi3.org/mmt/vocab#TradeProductContentUnitQuantity>
  a rdf:Property ;
  rdfs:comment "The number of content units of this trade product."^^xsd:string ;
  rdfs:domain "mmt:TradeProduct"^^xsd:string ;
  rdfs:label "contentUnitQuantity"^^xsd:string ;
  rdfs:range "xsd:decimal"^^xsd:string .

<https://edi3.org/mmt/vocab#TradeProductDescription>
  a rdf:Property ;
  rdfs:comment "A textual description for this trade product."^^xsd:string ;
  rdfs:domain "mmt:TradeProduct"^^xsd:string ;
  rdfs:label "description"^^xsd:string ;
  rdfs:range "xsd:string"^^xsd:string .

<https://edi3.org/mmt/vocab#TradeProductGlobalID>
  a rdf:Property ;
  rdfs:comment "A unique global identifier for this trade product."^^xsd:string ;
  rdfs:domain "mmt:TradeProduct"^^xsd:string ;
  rdfs:label "globalID"^^xsd:string ;
  rdfs:range "xsd:ID"^^xsd:string .

<https://edi3.org/mmt/vocab#TradeProductGrossVolume>
  a rdf:Property ;
  rdfs:comment "A measure of the gross volume for this trade product."^^xsd:string ;
  rdfs:domain "mmt:TradeProduct"^^xsd:string ;
  rdfs:label "grossVolume"^^xsd:string ;
  rdfs:range "xsd:decimal"^^xsd:string .

<https://edi3.org/mmt/vocab#TradeProductGrossWeight>
  a rdf:Property ;
  rdfs:comment "A measure of the gross weight (mass) of this trade product."^^xsd:string ;
  rdfs:domain "mmt:TradeProduct"^^xsd:string ;
  rdfs:label "grossWeight"^^xsd:string ;
  rdfs:range "xsd:decimal"^^xsd:string .

<https://edi3.org/mmt/vocab#TradeProductID>
  a rdf:Property ;
  rdfs:comment "A unique identifier for this trade product."^^xsd:string ;
  rdfs:domain "mmt:TradeProduct"^^xsd:string ;
  rdfs:label "iD"^^xsd:string ;
  rdfs:range "xsd:ID"^^xsd:string .

<https://edi3.org/mmt/vocab#TradeProductIntendedUseText>
  a rdf:Property ;
  rdfs:comment "An intended use, expressed as text, for this trade product."^^xsd:string ;
  rdfs:domain "mmt:TradeProduct"^^xsd:string ;
  rdfs:label "intendedUseText"^^xsd:string ;
  rdfs:range "xsd:string"^^xsd:string .

<https://edi3.org/mmt/vocab#TradeProductModelID>
  a rdf:Property ;
  rdfs:comment "A unique model identifier for this trade product."^^xsd:string ;
  rdfs:domain "mmt:TradeProduct"^^xsd:string ;
  rdfs:label "modelID"^^xsd:string ;
  rdfs:range "xsd:ID"^^xsd:string .

<https://edi3.org/mmt/vocab#TradeProductNetVolume>
  a rdf:Property ;
  rdfs:comment "A measure of a net volume for this trade product."^^xsd:string ;
  rdfs:domain "mmt:TradeProduct"^^xsd:string ;
  rdfs:label "netVolume"^^xsd:string ;
  rdfs:range "xsd:decimal"^^xsd:string .

<https://edi3.org/mmt/vocab#TradeProductNetWeight>
  a rdf:Property ;
  rdfs:comment "A measure of the net weight (mass) of this trade product."^^xsd:string ;
  rdfs:domain "mmt:TradeProduct"^^xsd:string ;
  rdfs:label "netWeight"^^xsd:string ;
  rdfs:range "xsd:decimal"^^xsd:string .

<https://edi3.org/mmt/vocab#TradeProductRecyclingTypeCode>
  a rdf:Property ;
  rdfs:comment "The code specifying the type of recycling for this trade product."^^xsd:string ;
  rdfs:domain "mmt:TradeProduct"^^xsd:string ;
  rdfs:label "recyclingTypeCode"^^xsd:string ;
  rdfs:range "xsd:token"^^xsd:string .

<https://edi3.org/mmt/vocab#TradeProductRegulationConformityID>
  a rdf:Property ;
  rdfs:comment "An identifier assigned to indicate conformity with a regulation or standard for this trade product, such as \"CE\" which declares that the product conforms with the essential requirements of the applicable EC directives."^^xsd:string ;
  rdfs:domain "mmt:TradeProduct"^^xsd:string ;
  rdfs:label "regulationConformityID"^^xsd:string ;
  rdfs:range "xsd:ID"^^xsd:string .

<https://edi3.org/mmt/vocab#TradeProductScientificName>
  a rdf:Property ;
  rdfs:comment "A scientific name, expressed as text, for this trade product."^^xsd:string ;
  rdfs:domain "mmt:TradeProduct"^^xsd:string ;
  rdfs:label "scientificName"^^xsd:string ;
  rdfs:range "xsd:string"^^xsd:string .

<https://edi3.org/mmt/vocab#TradeProductSubBrandName>
  a rdf:Property ;
  rdfs:comment "The sub-brand name, expressed as text, for this trade product."^^xsd:string ;
  rdfs:domain "mmt:TradeProduct"^^xsd:string ;
  rdfs:label "subBrandName"^^xsd:string ;
  rdfs:range "xsd:string"^^xsd:string .

<https://edi3.org/mmt/vocab#TradeProductTradeName>
  a rdf:Property ;
  rdfs:comment "A trade name, expressed as text, for this trade product."^^xsd:string ;
  rdfs:domain "mmt:TradeProduct"^^xsd:string ;
  rdfs:label "tradeName"^^xsd:string ;
  rdfs:range "xsd:string"^^xsd:string .

<https://edi3.org/mmt/vocab#TradeProductUseDescription>
  a rdf:Property ;
  rdfs:comment "A textual description of a use of this trade product."^^xsd:string ;
  rdfs:domain "mmt:TradeProduct"^^xsd:string ;
  rdfs:label "useDescription"^^xsd:string ;
  rdfs:range "xsd:string"^^xsd:string .

<https://edi3.org/mmt/vocab#TradeProductInstance>
  a rdfs:Class ;
  rdfs:comment "An individual trade product or batch of similar trade products produced by human or mechanical effort or by a natural process."^^xsd:string ;
  rdfs:label "TradeProductInstance"^^xsd:string .

<https://edi3.org/mmt/vocab#TradeProductInstanceActualQuantity>
  a rdf:Property ;
  rdfs:comment "The actual quantity of items in this trade product instance."^^xsd:string ;
  rdfs:domain "mmt:TradeProductInstance"^^xsd:string ;
  rdfs:label "actualQuantity"^^xsd:string ;
  rdfs:range "xsd:decimal"^^xsd:string .

<https://edi3.org/mmt/vocab#TradeProductInstanceBatchID>
  a rdf:Property ;
  rdfs:comment "The unique batch identifier for this trade product instance."^^xsd:string ;
  rdfs:domain "mmt:TradeProductInstance"^^xsd:string ;
  rdfs:label "batchID"^^xsd:string ;
  rdfs:range "xsd:ID"^^xsd:string .

<https://edi3.org/mmt/vocab#TradeProductInstanceBestBeforeDateTime>
  a rdf:Property ;
  rdfs:comment "The date, time, date time, or other date time value before which it is best to consume the items contained in this trade product instance."^^xsd:string ;
  rdfs:domain "mmt:TradeProductInstance"^^xsd:string ;
  rdfs:label "bestBeforeDateTime"^^xsd:string ;
  rdfs:range "xsd:datetime"^^xsd:string .

<https://edi3.org/mmt/vocab#TradeProductInstanceExpiryDateTime>
  a rdf:Property ;
  rdfs:comment "The date, time, date time, or other date time value of expiry of the items contained in the trade product instance."^^xsd:string ;
  rdfs:domain "mmt:TradeProductInstance"^^xsd:string ;
  rdfs:label "expiryDateTime"^^xsd:string ;
  rdfs:range "xsd:datetime"^^xsd:string .

<https://edi3.org/mmt/vocab#TradeProductInstanceLotID>
  a rdf:Property ;
  rdfs:comment "The unique lot identifier for this trade product instance."^^xsd:string ;
  rdfs:domain "mmt:TradeProductInstance"^^xsd:string ;
  rdfs:label "lotID"^^xsd:string ;
  rdfs:range "xsd:ID"^^xsd:string .

<https://edi3.org/mmt/vocab#TradeProductInstanceSellByDateTime>
  a rdf:Property ;
  rdfs:comment "The date, time, date time, or other date time value by after which the items contained in the trade product instance should not be sold."^^xsd:string ;
  rdfs:domain "mmt:TradeProductInstance"^^xsd:string ;
  rdfs:label "sellByDateTime"^^xsd:string ;
  rdfs:range "xsd:datetime"^^xsd:string .

<https://edi3.org/mmt/vocab#TradeProductInstanceSerialID>
  a rdf:Property ;
  rdfs:comment "A unique serial identifier for this trade product instance."^^xsd:string ;
  rdfs:domain "mmt:TradeProductInstance"^^xsd:string ;
  rdfs:label "serialID"^^xsd:string ;
  rdfs:range "xsd:ID"^^xsd:string .

<https://edi3.org/mmt/vocab#TradeTax>
  a rdfs:Class ;
  rdfs:comment "A trade related fiscal levy or duty."^^xsd:string ;
  rdfs:label "TradeTax"^^xsd:string .

<https://edi3.org/mmt/vocab#TradeTaxAllowanceChargeBasisAmount>
  a rdf:Property ;
  rdfs:comment "A monetary value used as the allowance and charge basis on which this trade related tax, levy or duty is calculated."^^xsd:string ;
  rdfs:domain "mmt:TradeTax"^^xsd:string ;
  rdfs:label "allowanceChargeBasisAmount"^^xsd:string ;
  rdfs:range "http://schema.org/amount"^^xsd:string .

<https://edi3.org/mmt/vocab#TradeTaxApplicableRatePercent>
  a rdf:Property ;
  rdfs:comment "The applicable rate, expressed as a percentage, for this trade tax, levy or duty."^^xsd:string ;
  rdfs:domain "mmt:TradeTax"^^xsd:string ;
  rdfs:label "applicableRatePercent"^^xsd:string ;
  rdfs:range "xsd:decimal"^^xsd:string .

<https://edi3.org/mmt/vocab#TradeTaxBasisAllowanceRate>
  a rdf:Property ;
  rdfs:comment "The rate of the tax basis allowance (deduction or discount) used to calculate the trade related tax, levy or duty."^^xsd:string ;
  rdfs:domain "mmt:TradeTax"^^xsd:string ;
  rdfs:label "basisAllowanceRate"^^xsd:string ;
  rdfs:range "xsd:decimal"^^xsd:string .

<https://edi3.org/mmt/vocab#TradeTaxBasisAmount>
  a rdf:Property ;
  rdfs:comment "A monetary value used as the basis on which this trade related tax, levy or duty is calculated."^^xsd:string ;
  rdfs:domain "mmt:TradeTax"^^xsd:string ;
  rdfs:label "basisAmount"^^xsd:string ;
  rdfs:range "http://schema.org/amount"^^xsd:string .

<https://edi3.org/mmt/vocab#TradeTaxBasisQuantity>
  a rdf:Property ;
  rdfs:comment "The quantity used as the basis for calculating the amount of this trade related tax, levy or duty."^^xsd:string ;
  rdfs:domain "mmt:TradeTax"^^xsd:string ;
  rdfs:label "basisQuantity"^^xsd:string ;
  rdfs:range "xsd:decimal"^^xsd:string .

<https://edi3.org/mmt/vocab#TradeTaxCalculatedAmount>
  a rdf:Property ;
  rdfs:comment "A monetary value resulting from the calculation of this trade related tax, levy or duty."^^xsd:string ;
  rdfs:domain "mmt:TradeTax"^^xsd:string ;
  rdfs:label "calculatedAmount"^^xsd:string ;
  rdfs:range "http://schema.org/amount"^^xsd:string .

<https://edi3.org/mmt/vocab#TradeTaxCalculatedRate>
  a rdf:Property ;
  rdfs:comment "The rate used to calculate the amount of this trade related tax, levy or duty."^^xsd:string ;
  rdfs:domain "mmt:TradeTax"^^xsd:string ;
  rdfs:label "calculatedRate"^^xsd:string ;
  rdfs:range "xsd:decimal"^^xsd:string .

<https://edi3.org/mmt/vocab#TradeTaxCalculationSequenceNumber>
  a rdf:Property ;
  rdfs:comment "A numeric expression of the sequence in which this trade related tax is to be or has been applied when multiple taxes are applicable per calculation, such as first \"Value Added Tax (VAT)\", second \"Transfer\"."^^xsd:string ;
  rdfs:domain "mmt:TradeTax"^^xsd:string ;
  rdfs:label "calculationSequenceNumber"^^xsd:string ;
  rdfs:range "xsd:decimal"^^xsd:string .

<https://edi3.org/mmt/vocab#TradeTaxCategoryCode>
  a rdf:Property ;
  rdfs:comment "The code specifying the category to which this trade related tax, levy or duty applies, such as codes for \"Exempt from Tax\", \"Standard Rate\", \"Free Export Item - Tax Not Charged\" [Reference United Nations Code List (UNCL) 5305]."^^xsd:string ;
  rdfs:domain "mmt:TradeTax"^^xsd:string ;
  rdfs:label "categoryCode"^^xsd:string ;
  rdfs:range "DutyorTaxorFeeCategoryType_Сode"^^xsd:string .

<https://edi3.org/mmt/vocab#TradeTaxCurrencyCode>
  a rdf:Property ;
  rdfs:comment "The code specifying the currency for this trade related tax, levy or duty [UNCL 6345]."^^xsd:string ;
  rdfs:domain "mmt:TradeTax"^^xsd:string ;
  rdfs:label "currencyCode"^^xsd:string ;
  rdfs:range "ISO4217_Code"^^xsd:string .

<https://edi3.org/mmt/vocab#TradeTaxCustomsDutyIndicator>
  a rdf:Property ;
  rdfs:comment "The indication of whether or not this trade related tax, levy or duty is a customs duty."^^xsd:string ;
  rdfs:domain "mmt:TradeTax"^^xsd:string ;
  rdfs:label "customsDutyIndicator"^^xsd:string ;
  rdfs:range "xsd:boolean"^^xsd:string .

<https://edi3.org/mmt/vocab#TradeTaxDeductionAmount>
  a rdf:Property ;
  rdfs:comment "A monetary value of the deduction from this trade related tax, levy or duty."^^xsd:string ;
  rdfs:domain "mmt:TradeTax"^^xsd:string ;
  rdfs:label "deductionAmount"^^xsd:string ;
  rdfs:range "http://schema.org/amount"^^xsd:string .

<https://edi3.org/mmt/vocab#TradeTaxDueDateTypeCode>
  a rdf:Property ;
  rdfs:comment "The code specifying a type of due date for this trade tax."^^xsd:string ;
  rdfs:domain "mmt:TradeTax"^^xsd:string ;
  rdfs:label "dueDateTypeCode"^^xsd:string ;
  rdfs:range "EventTimeReferenceType_Сode"^^xsd:string .

<https://edi3.org/mmt/vocab#TradeTaxExemptionAuthorizationID>
  a rdf:Property ;
  rdfs:comment "The unique identifier of the exemption authorization for this trade tax."^^xsd:string ;
  rdfs:domain "mmt:TradeTax"^^xsd:string ;
  rdfs:label "exemptionAuthorizationID"^^xsd:string ;
  rdfs:range "xsd:ID"^^xsd:string .

<https://edi3.org/mmt/vocab#TradeTaxExemptionIndicator>
  a rdf:Property ;
  rdfs:comment "The indication of whether or not there is an exemption from this trade tax."^^xsd:string ;
  rdfs:domain "mmt:TradeTax"^^xsd:string ;
  rdfs:label "exemptionIndicator"^^xsd:string ;
  rdfs:range "xsd:boolean"^^xsd:string .

<https://edi3.org/mmt/vocab#TradeTaxExemptionReasonCode>
  a rdf:Property ;
  rdfs:comment "A code specifying a reason for exemption from this trade related tax, levy or duty."^^xsd:string ;
  rdfs:domain "mmt:TradeTax"^^xsd:string ;
  rdfs:label "exemptionReasonCode"^^xsd:string ;
  rdfs:range "xsd:token"^^xsd:string .

<https://edi3.org/mmt/vocab#TradeTaxExemptionReasonText>
  a rdf:Property ;
  rdfs:comment "The reason, expressed as text, for exemption from this trade related tax, levy or duty."^^xsd:string ;
  rdfs:domain "mmt:TradeTax"^^xsd:string ;
  rdfs:label "exemptionReasonText"^^xsd:string ;
  rdfs:range "xsd:string"^^xsd:string .

<https://edi3.org/mmt/vocab#TradeTaxGuaranteeCode>
  a rdf:Property ;
  rdfs:comment "The code specifying an undertaking given in cash, bond or as a written guarantee to ensure that an obligation will be fulfilled for this trade related tax, levy or duty."^^xsd:string ;
  rdfs:domain "mmt:TradeTax"^^xsd:string ;
  rdfs:label "guaranteeCode"^^xsd:string ;
  rdfs:range "xsd:token"^^xsd:string .

<https://edi3.org/mmt/vocab#TradeTaxGuaranteeText>
  a rdf:Property ;
  rdfs:comment "The undertaking, expressed as text, given in cash, bond or as a written guarantee to ensure that an obligation will be fulfilled for this trade related tax, levy or duty."^^xsd:string ;
  rdfs:domain "mmt:TradeTax"^^xsd:string ;
  rdfs:label "guaranteeText"^^xsd:string ;
  rdfs:range "xsd:string"^^xsd:string .

<https://edi3.org/mmt/vocab#TradeTaxJurisdictionText>
  a rdf:Property ;
  rdfs:comment "A jurisdiction, expressed as text, to which this trade related tax, levy or duty applies."^^xsd:string ;
  rdfs:domain "mmt:TradeTax"^^xsd:string ;
  rdfs:label "jurisdictionText"^^xsd:string ;
  rdfs:range "xsd:string"^^xsd:string .

<https://edi3.org/mmt/vocab#TradeTaxLineTotalBasisAmount>
  a rdf:Property ;
  rdfs:comment "A monetary value used as the line total basis on which this trade related tax, levy or duty is calculated."^^xsd:string ;
  rdfs:domain "mmt:TradeTax"^^xsd:string ;
  rdfs:label "lineTotalBasisAmount"^^xsd:string ;
  rdfs:range "http://schema.org/amount"^^xsd:string .

<https://edi3.org/mmt/vocab#TradeTaxPaymentID>
  a rdf:Property ;
  rdfs:comment "The unique identifier of the payment of this trade related tax, levy or duty."^^xsd:string ;
  rdfs:domain "mmt:TradeTax"^^xsd:string ;
  rdfs:label "paymentID"^^xsd:string ;
  rdfs:range "xsd:ID"^^xsd:string .

<https://edi3.org/mmt/vocab#TradeTaxPaymentMethodCode>
  a rdf:Property ;
  rdfs:comment "The code specifying the payment method for this trade related tax, levy or duty."^^xsd:string ;
  rdfs:domain "mmt:TradeTax"^^xsd:string ;
  rdfs:label "paymentMethodCode"^^xsd:string ;
  rdfs:range "PaymentMethodType_Сode"^^xsd:string .

<https://edi3.org/mmt/vocab#TradeTaxPercent>
  a rdf:Property ;
  rdfs:comment "The percent of trade tax applicable, such as to an object or an activity."^^xsd:string ;
  rdfs:domain "mmt:TradeTax"^^xsd:string ;
  rdfs:label "percent"^^xsd:string ;
  rdfs:range "xsd:decimal"^^xsd:string .

<https://edi3.org/mmt/vocab#TradeTaxRateCode>
  a rdf:Property ;
  rdfs:comment "The code specifying the rate for this trade related tax, levy or duty."^^xsd:string ;
  rdfs:domain "mmt:TradeTax"^^xsd:string ;
  rdfs:label "rateCode"^^xsd:string ;
  rdfs:range "xsd:token"^^xsd:string .

<https://edi3.org/mmt/vocab#TradeTaxRefundAmount>
  a rdf:Property ;
  rdfs:comment "A monetary value of the refund of this trade related tax, levy or duty."^^xsd:string ;
  rdfs:domain "mmt:TradeTax"^^xsd:string ;
  rdfs:label "refundAmount"^^xsd:string ;
  rdfs:range "http://schema.org/amount"^^xsd:string .

<https://edi3.org/mmt/vocab#TradeTaxRegimeTypeCode>
  a rdf:Property ;
  rdfs:comment "The code specifying a type of regime applicable to the assessment or calculation of this trade related tax, levy or duty, such as a preferential duty rate."^^xsd:string ;
  rdfs:domain "mmt:TradeTax"^^xsd:string ;
  rdfs:label "regimeTypeCode"^^xsd:string ;
  rdfs:range "CustomsDutyRegimeType_Сode"^^xsd:string .

<https://edi3.org/mmt/vocab#TradeTaxSelfAssessedBasisAmount>
  a rdf:Property ;
  rdfs:comment "A monetary value of the amount on which this trade related tax, levy or duty has been calculated on a self-assessment basis."^^xsd:string ;
  rdfs:domain "mmt:TradeTax"^^xsd:string ;
  rdfs:label "selfAssessedBasisAmount"^^xsd:string ;
  rdfs:range "http://schema.org/amount"^^xsd:string .

<https://edi3.org/mmt/vocab#TradeTaxSelfAssessedBasisQuantity>
  a rdf:Property ;
  rdfs:comment "The quantity on which this trade related tax, levy or duty has been calculated on a self-assessment basis."^^xsd:string ;
  rdfs:domain "mmt:TradeTax"^^xsd:string ;
  rdfs:label "selfAssessedBasisQuantity"^^xsd:string ;
  rdfs:range "xsd:decimal"^^xsd:string .

<https://edi3.org/mmt/vocab#TradeTaxSelfAssessedCalculatedAmount>
  a rdf:Property ;
  rdfs:comment "A monetary value of the self-assessed calculated amount of this trade related tax, levy or duty."^^xsd:string ;
  rdfs:domain "mmt:TradeTax"^^xsd:string ;
  rdfs:label "selfAssessedCalculatedAmount"^^xsd:string ;
  rdfs:range "http://schema.org/amount"^^xsd:string .

<https://edi3.org/mmt/vocab#TradeTaxTariffDeductionQuantity>
  a rdf:Property ;
  rdfs:comment "A quantity to be deducted from the tariff quantity for the calculation of this trade related tax, duty or levy."^^xsd:string ;
  rdfs:domain "mmt:TradeTax"^^xsd:string ;
  rdfs:label "tariffDeductionQuantity"^^xsd:string ;
  rdfs:range "xsd:decimal"^^xsd:string .

<https://edi3.org/mmt/vocab#TradeTaxTaxExemptionAuthorityID>
  a rdf:Property ;
  rdfs:comment "The unique tax exemption authority identifier for this trade tax."^^xsd:string ;
  rdfs:domain "mmt:TradeTax"^^xsd:string ;
  rdfs:label "taxExemptionAuthorityID"^^xsd:string ;
  rdfs:range "xsd:ID"^^xsd:string .

<https://edi3.org/mmt/vocab#TradeTaxTaxPointDate>
  a rdf:Property ;
  rdfs:comment "The date of the tax point when this trade related tax, levy or duty becomes applicable."^^xsd:string ;
  rdfs:domain "mmt:TradeTax"^^xsd:string ;
  rdfs:label "taxPointDate"^^xsd:string ;
  rdfs:range "xsd:date"^^xsd:string .

<https://edi3.org/mmt/vocab#TradeTaxTypeCode>
  a rdf:Property ;
  rdfs:comment "The code specifying the type of trade related tax, levy or duty, such as a code for a Value Added Tax (VAT) [Reference United Nations Code List (UNCL) 5153]."^^xsd:string ;
  rdfs:domain "mmt:TradeTax"^^xsd:string ;
  rdfs:label "typeCode"^^xsd:string ;
  rdfs:range "DutyTaxFeeType_Сode"^^xsd:string .

<https://edi3.org/mmt/vocab#TradeTaxTypeText>
  a rdf:Property ;
  rdfs:comment "The type, expressed as text, of this trade related tax, levy or duty."^^xsd:string ;
  rdfs:domain "mmt:TradeTax"^^xsd:string ;
  rdfs:label "typeText"^^xsd:string ;
  rdfs:range "xsd:string"^^xsd:string .

<https://edi3.org/mmt/vocab#TradeTaxUnitBasisAmount>
  a rdf:Property ;
  rdfs:comment "A monetary value that constitutes the per unit basis on which this trade related tax, levy or duty is calculated."^^xsd:string ;
  rdfs:domain "mmt:TradeTax"^^xsd:string ;
  rdfs:label "unitBasisAmount"^^xsd:string ;
  rdfs:range "http://schema.org/amount"^^xsd:string .

<https://edi3.org/mmt/vocab#TransportServiceLocation>
  a rdfs:Class ;
  rdfs:comment "A location where a transport service takes place."^^xsd:string ;
  rdfs:label "TransportServiceLocation"^^xsd:string .

<https://edi3.org/mmt/vocab#TransportServiceLocationID>
  a rdf:Property ;
  rdfs:comment "An identifier for this transport service location, such as a United Nations Location Code (UNLOCODE) or GS1 Global Location Number (GLN)."^^xsd:string ;
  rdfs:domain "mmt:TransportServiceLocation"^^xsd:string ;
  rdfs:label "iD"^^xsd:string ;
  rdfs:range "xsd:ID"^^xsd:string .

<https://edi3.org/mmt/vocab#TransportServiceLocationName>
  a rdf:Property ;
  rdfs:comment "A name, expressed as text, of this transport service location."^^xsd:string ;
  rdfs:domain "mmt:TransportServiceLocation"^^xsd:string ;
  rdfs:label "name"^^xsd:string ;
  rdfs:range "xsd:string"^^xsd:string .

<https://edi3.org/mmt/vocab#TransportServiceLocationTypeCode>
  a rdf:Property ;
  rdfs:comment "A code specifying the type of transport service location."^^xsd:string ;
  rdfs:domain "mmt:TransportServiceLocation"^^xsd:string ;
  rdfs:label "typeCode"^^xsd:string ;
  rdfs:range "xsd:token"^^xsd:string .

<https://edi3.org/mmt/vocab#TransportSettingTemperature>
  a rdfs:Class ;
  rdfs:comment "Temperature settings for a transport movement, such as a required storage temperature range."^^xsd:string ;
  rdfs:label "TransportSettingTemperature"^^xsd:string .

<https://edi3.org/mmt/vocab#TransportSettingTemperatureMaximumValue>
  a rdf:Property ;
  rdfs:comment "The measure of the highest value of this transport setting temperature, such as a maximum temperature value of fourteen degrees Celsius."^^xsd:string ;
  rdfs:domain "mmt:TransportSettingTemperature"^^xsd:string ;
  rdfs:label "maximumValue"^^xsd:string ;
  rdfs:range "xsd:decimal"^^xsd:string .

<https://edi3.org/mmt/vocab#TransportSettingTemperatureMinimumValue>
  a rdf:Property ;
  rdfs:comment "The measure of the lowest value of this transport setting temperature, such as a minimum temperature value of four degrees Celsius."^^xsd:string ;
  rdfs:domain "mmt:TransportSettingTemperature"^^xsd:string ;
  rdfs:label "minimumValue"^^xsd:string ;
  rdfs:range "xsd:decimal"^^xsd:string .

<https://edi3.org/mmt/vocab#TransportSettingTemperatureTypeCode>
  a rdf:Property ;
  rdfs:comment "The code specifying the type of transport setting temperature [Reference United Nations Code List (UNCL) 6245]."^^xsd:string ;
  rdfs:domain "mmt:TransportSettingTemperature"^^xsd:string ;
  rdfs:label "typeCode"^^xsd:string ;
  rdfs:range "TemperatureType_Сode"^^xsd:string .

<https://edi3.org/mmt/vocab#TransportSettingTemperatureValue>
  a rdf:Property ;
  rdfs:comment "The measure of the value of this transport setting temperature, such as a temperature value of ten degrees Celsius."^^xsd:string ;
  rdfs:domain "mmt:TransportSettingTemperature"^^xsd:string ;
  rdfs:label "value"^^xsd:string ;
  rdfs:range "xsd:decimal"^^xsd:string .

<https://edi3.org/mmt/vocab#TransportCargo>
  a rdfs:Class ;
  rdfs:comment "Information about goods being transported identifying their nature for customs, statistical or transport purposes."^^xsd:string ;
  rdfs:label "TransportCargo"^^xsd:string .

<https://edi3.org/mmt/vocab#TransportCargoIdentificationText>
  a rdf:Property ;
  rdfs:comment "The identification, expressed as text, of this transport cargo that is sufficient to identify it for customs, statistical or transport purposes."^^xsd:string ;
  rdfs:domain "mmt:TransportCargo"^^xsd:string ;
  rdfs:label "identificationText"^^xsd:string ;
  rdfs:range "xsd:string"^^xsd:string .

<https://edi3.org/mmt/vocab#TransportCargoOperationalCategoryCode>
  a rdf:Property ;
  rdfs:comment "The code specifying the operational category for this transport cargo, such as obnoxious or military."^^xsd:string ;
  rdfs:domain "mmt:TransportCargo"^^xsd:string ;
  rdfs:label "operationalCategoryCode"^^xsd:string ;
  rdfs:range "CargoOperationalCategoryType_Сode"^^xsd:string .

<https://edi3.org/mmt/vocab#TransportCargoStatisticalClassificationCode>
  a rdf:Property ;
  rdfs:comment "The code specifying a statistical classification for this transport cargo."^^xsd:string ;
  rdfs:domain "mmt:TransportCargo"^^xsd:string ;
  rdfs:label "statisticalClassificationCode"^^xsd:string ;
  rdfs:range "CommodityIdentificationType_Сode"^^xsd:string .

<https://edi3.org/mmt/vocab#TransportCargoTypeCode>
  a rdf:Property ;
  rdfs:comment "The code, such as UNECE Recommendation 21 single digit codes, specifying the type of transported cargo."^^xsd:string ;
  rdfs:domain "mmt:TransportCargo"^^xsd:string ;
  rdfs:label "typeCode"^^xsd:string ;
  rdfs:range "CargoType_Сode"^^xsd:string .

<https://edi3.org/mmt/vocab#TransportCargoInsurance>
  a rdfs:Class ;
  rdfs:comment "Insurance coverage for cargo during transport movements."^^xsd:string ;
  rdfs:label "TransportCargoInsurance"^^xsd:string .

<https://edi3.org/mmt/vocab#TransportCargoInsuranceContractGeneralConditionsText>
  a rdf:Property ;
  rdfs:comment "The contract general conditions, expressed as text, for this transport cargo insurance."^^xsd:string ;
  rdfs:domain "mmt:TransportCargoInsurance"^^xsd:string ;
  rdfs:label "contractGeneralConditionsText"^^xsd:string ;
  rdfs:range "xsd:string"^^xsd:string .

<https://edi3.org/mmt/vocab#TransportCargoInsuranceCoverageCode>
  a rdf:Property ;
  rdfs:comment "The code specifying the coverage of this transport cargo insurance."^^xsd:string ;
  rdfs:domain "mmt:TransportCargoInsurance"^^xsd:string ;
  rdfs:label "coverageCode"^^xsd:string ;
  rdfs:range "xsd:token"^^xsd:string .

<https://edi3.org/mmt/vocab#TransportCargoInsuranceCoverageDescription>
  a rdf:Property ;
  rdfs:comment "The textual description of the coverage of this transport cargo insurance."^^xsd:string ;
  rdfs:domain "mmt:TransportCargoInsurance"^^xsd:string ;
  rdfs:label "coverageDescription"^^xsd:string ;
  rdfs:range "xsd:string"^^xsd:string .

<https://edi3.org/mmt/vocab#TransportDangerousGoods>
  a rdfs:Class ;
  rdfs:comment "Goods which may contain a substance which poses risks to people and/or the environment during transportation which is regulated by dangerous goods regulations."^^xsd:string ;
  rdfs:label "TransportDangerousGoods"^^xsd:string .

<https://edi3.org/mmt/vocab#TransportDangerousGoodsAdditionalHazardClassificationID>
  a rdf:Property ;
  rdfs:comment "The unique identifier of an additional hazard class applicable to these transported dangerous goods."^^xsd:string ;
  rdfs:domain "mmt:TransportDangerousGoods"^^xsd:string ;
  rdfs:label "additionalHazardClassificationID"^^xsd:string ;
  rdfs:range "xsd:ID"^^xsd:string .

<https://edi3.org/mmt/vocab#TransportDangerousGoodsAircraftLimitationInformation>
  a rdf:Property ;
  rdfs:comment "Aircraft limitation information, expressed as text, for these transported dangerous goods."^^xsd:string ;
  rdfs:domain "mmt:TransportDangerousGoods"^^xsd:string ;
  rdfs:label "aircraftLimitationInformation"^^xsd:string ;
  rdfs:range "xsd:string"^^xsd:string .

<https://edi3.org/mmt/vocab#TransportDangerousGoodsAllPackedInOneInformation>
  a rdf:Property ;
  rdfs:comment "All packed in one information, expressed as text, for these transported dangerous goods."^^xsd:string ;
  rdfs:domain "mmt:TransportDangerousGoods"^^xsd:string ;
  rdfs:label "allPackedInOneInformation"^^xsd:string ;
  rdfs:range "xsd:string"^^xsd:string .

<https://edi3.org/mmt/vocab#TransportDangerousGoodsAuthorizationInformation>
  a rdf:Property ;
  rdfs:comment "Authorization information, expressed as text, for these transported dangerous goods."^^xsd:string ;
  rdfs:domain "mmt:TransportDangerousGoods"^^xsd:string ;
  rdfs:label "authorizationInformation"^^xsd:string ;
  rdfs:range "xsd:string"^^xsd:string .

<https://edi3.org/mmt/vocab#TransportDangerousGoodsComplianceDeclarationInformation>
  a rdf:Property ;
  rdfs:comment "Compliance declaration information, expressed as text, for these transported dangerous goods."^^xsd:string ;
  rdfs:domain "mmt:TransportDangerousGoods"^^xsd:string ;
  rdfs:label "complianceDeclarationInformation"^^xsd:string ;
  rdfs:range "xsd:string"^^xsd:string .

<https://edi3.org/mmt/vocab#TransportDangerousGoodsEMSID>
  a rdf:Property ;
  rdfs:comment "The unique transport emergency procedure (EMS) identifier applicable for these transported dangerous goods."^^xsd:string ;
  rdfs:domain "mmt:TransportDangerousGoods"^^xsd:string ;
  rdfs:label "eMSID"^^xsd:string ;
  rdfs:range "xsd:ID"^^xsd:string .

<https://edi3.org/mmt/vocab#TransportDangerousGoodsExplosiveCargoNetWeight>
  a rdf:Property ;
  rdfs:comment "The measure of the explosive cargo weight applicable to these transported dangerous goods."^^xsd:string ;
  rdfs:domain "mmt:TransportDangerousGoods"^^xsd:string ;
  rdfs:label "explosiveCargoNetWeight"^^xsd:string ;
  rdfs:range "xsd:decimal"^^xsd:string .

<https://edi3.org/mmt/vocab#TransportDangerousGoodsExplosiveCompatibilityGroupCode>
  a rdf:Property ;
  rdfs:comment "The code specifying the explosive compatibility group for these transported dangerous goods."^^xsd:string ;
  rdfs:domain "mmt:TransportDangerousGoods"^^xsd:string ;
  rdfs:label "explosiveCompatibilityGroupCode"^^xsd:string ;
  rdfs:range "xsd:token"^^xsd:string .

<https://edi3.org/mmt/vocab#TransportDangerousGoodsGrossVolume>
  a rdf:Property ;
  rdfs:comment "The measure of the gross volume, normally calculated by multiplying the maximum length, width and height dimensions of these transported dangerous goods."^^xsd:string ;
  rdfs:domain "mmt:TransportDangerousGoods"^^xsd:string ;
  rdfs:label "grossVolume"^^xsd:string ;
  rdfs:range "xsd:decimal"^^xsd:string .

<https://edi3.org/mmt/vocab#TransportDangerousGoodsGrossWeight>
  a rdf:Property ;
  rdfs:comment "The measure of the weight (mass) of these transported dangerous goods including packaging but excluding the transport equipment."^^xsd:string ;
  rdfs:domain "mmt:TransportDangerousGoods"^^xsd:string ;
  rdfs:label "grossWeight"^^xsd:string ;
  rdfs:range "xsd:decimal"^^xsd:string .

<https://edi3.org/mmt/vocab#TransportDangerousGoodsHazardCategoryCode>
  a rdf:Property ;
  rdfs:comment "The code specifying the hazard category for these transported dangerous goods."^^xsd:string ;
  rdfs:domain "mmt:TransportDangerousGoods"^^xsd:string ;
  rdfs:label "hazardCategoryCode"^^xsd:string ;
  rdfs:range "xsd:token"^^xsd:string .

<https://edi3.org/mmt/vocab#TransportDangerousGoodsHazardClassVersionID>
  a rdf:Property ;
  rdfs:comment "The unique identifier of the version of a hazard class for these transported dangerous goods."^^xsd:string ;
  rdfs:domain "mmt:TransportDangerousGoods"^^xsd:string ;
  rdfs:label "hazardClassVersionID"^^xsd:string ;
  rdfs:range "xsd:ID"^^xsd:string .

<https://edi3.org/mmt/vocab#TransportDangerousGoodsHazardClassificationID>
  a rdf:Property ;
  rdfs:comment "The unique identifier of a hazard class applicable to these transported dangerous goods as defined by the relevant governing regulation authority."^^xsd:string ;
  rdfs:domain "mmt:TransportDangerousGoods"^^xsd:string ;
  rdfs:label "hazardClassificationID"^^xsd:string ;
  rdfs:range "xsd:ID"^^xsd:string .

<https://edi3.org/mmt/vocab#TransportDangerousGoodsHazardTypeCode>
  a rdf:Property ;
  rdfs:comment "A code specifying the type of hazard for these transported dangerous goods."^^xsd:string ;
  rdfs:domain "mmt:TransportDangerousGoods"^^xsd:string ;
  rdfs:label "hazardTypeCode"^^xsd:string ;
  rdfs:range "xsd:token"^^xsd:string .

<https://edi3.org/mmt/vocab#TransportDangerousGoodsIMDGSegregationGroupCode>
  a rdf:Property ;
  rdfs:comment "The code specifying the IMDG (International Maritime Dangerous Goods regulation) segregation group for these transported dangerous goods."^^xsd:string ;
  rdfs:domain "mmt:TransportDangerousGoods"^^xsd:string ;
  rdfs:label "iMDGSegregationGroupCode"^^xsd:string ;
  rdfs:range "xsd:token"^^xsd:string .

<https://edi3.org/mmt/vocab#TransportDangerousGoodsInformation>
  a rdf:Property ;
  rdfs:comment "Information, expressed as text, concerning the transport of these dangerous goods."^^xsd:string ;
  rdfs:domain "mmt:TransportDangerousGoods"^^xsd:string ;
  rdfs:label "information"^^xsd:string ;
  rdfs:range "xsd:string"^^xsd:string .

<https://edi3.org/mmt/vocab#TransportDangerousGoodsLimitedQuantityCode>
  a rdf:Property ;
  rdfs:comment "A code specifying facilitations for transport of limited quantities of these transported dangerous goods."^^xsd:string ;
  rdfs:domain "mmt:TransportDangerousGoods"^^xsd:string ;
  rdfs:label "limitedQuantityCode"^^xsd:string ;
  rdfs:range "xsd:token"^^xsd:string .

<https://edi3.org/mmt/vocab#TransportDangerousGoodsLowerPartOrangeHazardPlacardID>
  a rdf:Property ;
  rdfs:comment "The unique lower part of the orange hazard placard identifier for these transported dangerous goods."^^xsd:string ;
  rdfs:domain "mmt:TransportDangerousGoods"^^xsd:string ;
  rdfs:label "lowerPartOrangeHazardPlacardID"^^xsd:string ;
  rdfs:range "xsd:ID"^^xsd:string .

<https://edi3.org/mmt/vocab#TransportDangerousGoodsMFAGID>
  a rdf:Property ;
  rdfs:comment "The unique Medical First Aid Guide (MFAG) identifier for these transported dangerous goods."^^xsd:string ;
  rdfs:domain "mmt:TransportDangerousGoods"^^xsd:string ;
  rdfs:label "mFAGID"^^xsd:string ;
  rdfs:range "xsd:ID"^^xsd:string .

<https://edi3.org/mmt/vocab#TransportDangerousGoodsMarinePollutantIndicator>
  a rdf:Property ;
  rdfs:comment "The indication of whether or not these transported dangerous goods have a marine pollutant content."^^xsd:string ;
  rdfs:domain "mmt:TransportDangerousGoods"^^xsd:string ;
  rdfs:label "marinePollutantIndicator"^^xsd:string ;
  rdfs:range "xsd:boolean"^^xsd:string .

<https://edi3.org/mmt/vocab#TransportDangerousGoodsMarkingText>
  a rdf:Property ;
  rdfs:comment "Marking, expressed as text, for these transported dangerous goods."^^xsd:string ;
  rdfs:domain "mmt:TransportDangerousGoods"^^xsd:string ;
  rdfs:label "markingText"^^xsd:string ;
  rdfs:range "xsd:string"^^xsd:string .

<https://edi3.org/mmt/vocab#TransportDangerousGoodsNetWeight>
  a rdf:Property ;
  rdfs:comment "The measure of the net weight (mass) of these transported dangerous goods."^^xsd:string ;
  rdfs:domain "mmt:TransportDangerousGoods"^^xsd:string ;
  rdfs:label "netWeight"^^xsd:string ;
  rdfs:range "xsd:decimal"^^xsd:string .

<https://edi3.org/mmt/vocab#TransportDangerousGoodsOverpackInformation>
  a rdf:Property ;
  rdfs:comment "Overpack information, expressed as text, for these transported dangerous goods."^^xsd:string ;
  rdfs:domain "mmt:TransportDangerousGoods"^^xsd:string ;
  rdfs:label "overpackInformation"^^xsd:string ;
  rdfs:range "xsd:string"^^xsd:string .

<https://edi3.org/mmt/vocab#TransportDangerousGoodsPackageTypeCode>
  a rdf:Property ;
  rdfs:comment "The code specifying the package type for the transported dangerous goods."^^xsd:string ;
  rdfs:domain "mmt:TransportDangerousGoods"^^xsd:string ;
  rdfs:label "packageTypeCode"^^xsd:string ;
  rdfs:range "PackageType_Сode"^^xsd:string .

<https://edi3.org/mmt/vocab#TransportDangerousGoodsPackagingDangerLevelCode>
  a rdf:Property ;
  rdfs:comment "The code specifying the level of danger that the packaging of these dangerous goods must cover for transport purposes."^^xsd:string ;
  rdfs:domain "mmt:TransportDangerousGoods"^^xsd:string ;
  rdfs:label "packagingDangerLevelCode"^^xsd:string ;
  rdfs:range "DangerousGoodsPackingType_Сode"^^xsd:string .

<https://edi3.org/mmt/vocab#TransportDangerousGoodsPackingInstructionTypeCode>
  a rdf:Property ;
  rdfs:comment "The code specifying a type of packing instruction for these transported dangerous goods."^^xsd:string ;
  rdfs:domain "mmt:TransportDangerousGoods"^^xsd:string ;
  rdfs:label "packingInstructionTypeCode"^^xsd:string ;
  rdfs:range "xsd:token"^^xsd:string .

<https://edi3.org/mmt/vocab#TransportDangerousGoodsPollutantIndicator>
  a rdf:Property ;
  rdfs:comment "The indication of whether or not these transported dangerous goods have a pollutant content."^^xsd:string ;
  rdfs:domain "mmt:TransportDangerousGoods"^^xsd:string ;
  rdfs:label "pollutantIndicator"^^xsd:string ;
  rdfs:range "xsd:boolean"^^xsd:string .

<https://edi3.org/mmt/vocab#TransportDangerousGoodsPollutantLevelCode>
  a rdf:Property ;
  rdfs:comment "The code specifying the level of pollution of these transported dangerous goods."^^xsd:string ;
  rdfs:domain "mmt:TransportDangerousGoods"^^xsd:string ;
  rdfs:label "pollutantLevelCode"^^xsd:string ;
  rdfs:range "xsd:token"^^xsd:string .

<https://edi3.org/mmt/vocab#TransportDangerousGoodsProperShippingName>
  a rdf:Property ;
  rdfs:comment "The proper shipping name, expressed as text, for these transported dangerous goods."^^xsd:string ;
  rdfs:domain "mmt:TransportDangerousGoods"^^xsd:string ;
  rdfs:label "properShippingName"^^xsd:string ;
  rdfs:range "xsd:string"^^xsd:string .

<https://edi3.org/mmt/vocab#TransportDangerousGoodsQValueNumber>
  a rdf:Property ;
  rdfs:comment "The number of the Q-Value for these transported dangerous goods."^^xsd:string ;
  rdfs:domain "mmt:TransportDangerousGoods"^^xsd:string ;
  rdfs:label "qValueNumber"^^xsd:string ;
  rdfs:range "xsd:decimal"^^xsd:string .

<https://edi3.org/mmt/vocab#TransportDangerousGoodsRegulationCode>
  a rdf:Property ;
  rdfs:comment "The code specifying a regulation applicable to these transported dangerous goods."^^xsd:string ;
  rdfs:domain "mmt:TransportDangerousGoods"^^xsd:string ;
  rdfs:label "regulationCode"^^xsd:string ;
  rdfs:range "DangerousGoodsRegulationType_Сode"^^xsd:string .

<https://edi3.org/mmt/vocab#TransportDangerousGoodsRegulationName>
  a rdf:Property ;
  rdfs:comment "A name, expressed as text, for a regulation of these transported dangerous goods."^^xsd:string ;
  rdfs:domain "mmt:TransportDangerousGoods"^^xsd:string ;
  rdfs:label "regulationName"^^xsd:string ;
  rdfs:range "xsd:string"^^xsd:string .

<https://edi3.org/mmt/vocab#TransportDangerousGoodsRegulatoryAuthorityName>
  a rdf:Property ;
  rdfs:comment "The name, expressed as text, for the regulatory authority for these transported dangerous goods."^^xsd:string ;
  rdfs:domain "mmt:TransportDangerousGoods"^^xsd:string ;
  rdfs:label "regulatoryAuthorityName"^^xsd:string ;
  rdfs:range "xsd:string"^^xsd:string .

<https://edi3.org/mmt/vocab#TransportDangerousGoodsReportableQuantity>
  a rdf:Property ;
  rdfs:comment "The reportable quantity for these transported dangerous goods."^^xsd:string ;
  rdfs:domain "mmt:TransportDangerousGoods"^^xsd:string ;
  rdfs:label "reportableQuantity"^^xsd:string ;
  rdfs:range "xsd:decimal"^^xsd:string .

<https://edi3.org/mmt/vocab#TransportDangerousGoodsShipperDeclarationInformation>
  a rdf:Property ;
  rdfs:comment "Shipper declaration information, expressed as text, for these transported dangerous goods."^^xsd:string ;
  rdfs:domain "mmt:TransportDangerousGoods"^^xsd:string ;
  rdfs:label "shipperDeclarationInformation"^^xsd:string ;
  rdfs:range "xsd:string"^^xsd:string .

<https://edi3.org/mmt/vocab#TransportDangerousGoodsSpecialProvisionID>
  a rdf:Property ;
  rdfs:comment "The unique identifier of the special provision for these transported dangerous goods."^^xsd:string ;
  rdfs:domain "mmt:TransportDangerousGoods"^^xsd:string ;
  rdfs:label "specialProvisionID"^^xsd:string ;
  rdfs:range "xsd:ID"^^xsd:string .

<https://edi3.org/mmt/vocab#TransportDangerousGoodsSupplementaryInformation>
  a rdf:Property ;
  rdfs:comment "Supplementary information, expressed as text, concerning the transport of these dangerous goods."^^xsd:string ;
  rdfs:domain "mmt:TransportDangerousGoods"^^xsd:string ;
  rdfs:label "supplementaryInformation"^^xsd:string ;
  rdfs:range "xsd:string"^^xsd:string .

<https://edi3.org/mmt/vocab#TransportDangerousGoodsTREMID>
  a rdf:Property ;
  rdfs:comment "The unique TRansport EMergency (TREM) card identifier for these transported dangerous goods."^^xsd:string ;
  rdfs:domain "mmt:TransportDangerousGoods"^^xsd:string ;
  rdfs:label "tREMID"^^xsd:string ;
  rdfs:range "xsd:ID"^^xsd:string .

<https://edi3.org/mmt/vocab#TransportDangerousGoodsTechnicalName>
  a rdf:Property ;
  rdfs:comment "A technical name, expressed as text, for these transported dangerous goods."^^xsd:string ;
  rdfs:domain "mmt:TransportDangerousGoods"^^xsd:string ;
  rdfs:label "technicalName"^^xsd:string ;
  rdfs:range "xsd:string"^^xsd:string .

<https://edi3.org/mmt/vocab#TransportDangerousGoodsTunnelRestrictionCode>
  a rdf:Property ;
  rdfs:comment "The code specifying the tunnel restriction for these transported dangerous goods."^^xsd:string ;
  rdfs:domain "mmt:TransportDangerousGoods"^^xsd:string ;
  rdfs:label "tunnelRestrictionCode"^^xsd:string ;
  rdfs:range "xsd:token"^^xsd:string .

<https://edi3.org/mmt/vocab#TransportDangerousGoodsUNDGID>
  a rdf:Property ;
  rdfs:comment "The code specifying the unique United Nations Dangerous Goods (UNDG) number assigned to these transported dangerous goods."^^xsd:string ;
  rdfs:domain "mmt:TransportDangerousGoods"^^xsd:string ;
  rdfs:label "uNDGID"^^xsd:string ;
  rdfs:range "xsd:token"^^xsd:string .

<https://edi3.org/mmt/vocab#TransportDangerousGoodsUpperPartOrangeHazardPlacardID>
  a rdf:Property ;
  rdfs:comment "The unique upper part of the orange hazard placard identifier for these transported dangerous goods."^^xsd:string ;
  rdfs:domain "mmt:TransportDangerousGoods"^^xsd:string ;
  rdfs:label "upperPartOrangeHazardPlacardID"^^xsd:string ;
  rdfs:range "xsd:ID"^^xsd:string .

<https://edi3.org/mmt/vocab#TransportEvent>
  a rdfs:Class ;
  rdfs:comment "A significant occurrence or happening during transport."^^xsd:string ;
  rdfs:label "TransportEvent"^^xsd:string .

<https://edi3.org/mmt/vocab#TransportEventActualArrivalDateTime>
  a rdf:Property ;
  rdfs:comment "The date, time, date time or other date time value of the actual arrival related to this transport event."^^xsd:string ;
  rdfs:domain "mmt:TransportEvent"^^xsd:string ;
  rdfs:label "actualArrivalDateTime"^^xsd:string ;
  rdfs:range "xsd:datetime"^^xsd:string .

<https://edi3.org/mmt/vocab#TransportEventActualDepartureDateTime>
  a rdf:Property ;
  rdfs:comment "The date, time, date time or other date time value of the actual departure related to this transport event."^^xsd:string ;
  rdfs:domain "mmt:TransportEvent"^^xsd:string ;
  rdfs:label "actualDepartureDateTime"^^xsd:string ;
  rdfs:range "xsd:datetime"^^xsd:string .

<https://edi3.org/mmt/vocab#TransportEventActualOccurrenceDateTime>
  a rdf:Property ;
  rdfs:comment "The actual date, time, date time, or other date time value of the occurrence of this transport event."^^xsd:string ;
  rdfs:domain "mmt:TransportEvent"^^xsd:string ;
  rdfs:label "actualOccurrenceDateTime"^^xsd:string ;
  rdfs:range "xsd:datetime"^^xsd:string .

<https://edi3.org/mmt/vocab#TransportEventArrivalDateTime>
  a rdf:Property ;
  rdfs:comment "An arrival date, time, date time, or other date time value related to this transport event."^^xsd:string ;
  rdfs:domain "mmt:TransportEvent"^^xsd:string ;
  rdfs:label "arrivalDateTime"^^xsd:string ;
  rdfs:range "xsd:datetime"^^xsd:string .

<https://edi3.org/mmt/vocab#TransportEventDepartureDateTime>
  a rdf:Property ;
  rdfs:comment "A departure date, time, date time, or other date time value related to this transport event."^^xsd:string ;
  rdfs:domain "mmt:TransportEvent"^^xsd:string ;
  rdfs:label "departureDateTime"^^xsd:string ;
  rdfs:range "xsd:datetime"^^xsd:string .

<https://edi3.org/mmt/vocab#TransportEventDescription>
  a rdf:Property ;
  rdfs:comment "The textual description of this transport event."^^xsd:string ;
  rdfs:domain "mmt:TransportEvent"^^xsd:string ;
  rdfs:label "description"^^xsd:string ;
  rdfs:range "xsd:string"^^xsd:string .

<https://edi3.org/mmt/vocab#TransportEventEstimatedOccurrenceDateTime>
  a rdf:Property ;
  rdfs:comment "The estimated date, time, date time, or other date time value of the occurrence of this transport event."^^xsd:string ;
  rdfs:domain "mmt:TransportEvent"^^xsd:string ;
  rdfs:label "estimatedOccurrenceDateTime"^^xsd:string ;
  rdfs:range "xsd:datetime"^^xsd:string .

<https://edi3.org/mmt/vocab#TransportEventEstimatedTransportMeansArrivalOccurrenceDateTime>
  a rdf:Property ;
  rdfs:comment "The date, time, date time, or other date time value when the arrival of a means of transport at the location of this transport event is estimated to occur."^^xsd:string ;
  rdfs:domain "mmt:TransportEvent"^^xsd:string ;
  rdfs:label "estimatedTransportMeansArrivalOccurrenceDateTime"^^xsd:string ;
  rdfs:range "xsd:datetime"^^xsd:string .

<https://edi3.org/mmt/vocab#TransportEventID>
  a rdf:Property ;
  rdfs:comment "The unique identifier for this transport event."^^xsd:string ;
  rdfs:domain "mmt:TransportEvent"^^xsd:string ;
  rdfs:label "iD"^^xsd:string ;
  rdfs:range "xsd:ID"^^xsd:string .

<https://edi3.org/mmt/vocab#TransportEventRequestedOccurrenceDateTime>
  a rdf:Property ;
  rdfs:comment "The requested date, time, date time, or other date time value of the occurrence of this transport event."^^xsd:string ;
  rdfs:domain "mmt:TransportEvent"^^xsd:string ;
  rdfs:label "requestedOccurrenceDateTime"^^xsd:string ;
  rdfs:range "xsd:datetime"^^xsd:string .

<https://edi3.org/mmt/vocab#TransportEventScheduledArrivalDateTime>
  a rdf:Property ;
  rdfs:comment "The date, time, date time or other date time value of the scheduled arrival related to this transport event."^^xsd:string ;
  rdfs:domain "mmt:TransportEvent"^^xsd:string ;
  rdfs:label "scheduledArrivalDateTime"^^xsd:string ;
  rdfs:range "xsd:datetime"^^xsd:string .

<https://edi3.org/mmt/vocab#TransportEventScheduledDepartureDateTime>
  a rdf:Property ;
  rdfs:comment "The date, time, date time or other date time value of the scheduled departure related to this transport event."^^xsd:string ;
  rdfs:domain "mmt:TransportEvent"^^xsd:string ;
  rdfs:label "scheduledDepartureDateTime"^^xsd:string ;
  rdfs:range "xsd:datetime"^^xsd:string .

<https://edi3.org/mmt/vocab#TransportEventScheduledOccurrenceDateTime>
  a rdf:Property ;
  rdfs:comment "The scheduled date, time, date time, or other date time value of the occurrence of this transport event."^^xsd:string ;
  rdfs:domain "mmt:TransportEvent"^^xsd:string ;
  rdfs:label "scheduledOccurrenceDateTime"^^xsd:string ;
  rdfs:range "xsd:datetime"^^xsd:string .

<https://edi3.org/mmt/vocab#TransportEventTypeCode>
  a rdf:Property ;
  rdfs:comment "The code specifying the type of transport event."^^xsd:string ;
  rdfs:domain "mmt:TransportEvent"^^xsd:string ;
  rdfs:label "typeCode"^^xsd:string ;
  rdfs:range "xsd:token"^^xsd:string .

<https://edi3.org/mmt/vocab#TransportEventUnitQuantity>
  a rdf:Property ;
  rdfs:comment "The number of units for this transport event."^^xsd:string ;
  rdfs:domain "mmt:TransportEvent"^^xsd:string ;
  rdfs:label "unitQuantity"^^xsd:string ;
  rdfs:range "xsd:decimal"^^xsd:string .

<https://edi3.org/mmt/vocab#TransportInstructions>
  a rdfs:Class ;
  rdfs:comment "Transport information of an instructive nature."^^xsd:string ;
  rdfs:label "TransportInstructions"^^xsd:string .

<https://edi3.org/mmt/vocab#TransportInstructionsDescription>
  a rdf:Property ;
  rdfs:comment "A textual description of these transport instructions."^^xsd:string ;
  rdfs:domain "mmt:TransportInstructions"^^xsd:string ;
  rdfs:label "description"^^xsd:string ;
  rdfs:range "xsd:string"^^xsd:string .

<https://edi3.org/mmt/vocab#TransportInstructionsDescriptionCode>
  a rdf:Property ;
  rdfs:comment "The code specifying a description of these transport instructions."^^xsd:string ;
  rdfs:domain "mmt:TransportInstructions"^^xsd:string ;
  rdfs:label "descriptionCode"^^xsd:string ;
  rdfs:range "xsd:token"^^xsd:string .

<https://edi3.org/mmt/vocab#TransportPerson>
  a rdfs:Class ;
  rdfs:comment "A transport related person, such as a member of a crew or a passenger."^^xsd:string ;
  rdfs:label "TransportPerson"^^xsd:string .

<https://edi3.org/mmt/vocab#TransportPersonBirthDateTime>
  a rdf:Property ;
  rdfs:comment "The birth date of this transport person."^^xsd:string ;
  rdfs:domain "mmt:TransportPerson"^^xsd:string ;
  rdfs:label "birthDateTime"^^xsd:string ;
  rdfs:range "xsd:datetime"^^xsd:string .

<https://edi3.org/mmt/vocab#TransportPersonID>
  a rdf:Property ;
  rdfs:comment "The unique identifier for this transport person."^^xsd:string ;
  rdfs:domain "mmt:TransportPerson"^^xsd:string ;
  rdfs:label "iD"^^xsd:string ;
  rdfs:range "xsd:ID"^^xsd:string .

<https://edi3.org/mmt/vocab#TransportPersonLanguageCode>
  a rdf:Property ;
  rdfs:comment "A unique identifier of a language related to this transport person, such as their spoken or correspondence language."^^xsd:string ;
  rdfs:domain "mmt:TransportPerson"^^xsd:string ;
  rdfs:label "languageCode"^^xsd:string ;
  rdfs:range "ISO639_Code"^^xsd:string .

<https://edi3.org/mmt/vocab#TransportPersonName>
  a rdf:Property ;
  rdfs:comment "The name or set of names, expressed as text, by which this transport person is known."^^xsd:string ;
  rdfs:domain "mmt:TransportPerson"^^xsd:string ;
  rdfs:label "name"^^xsd:string ;
  rdfs:range "xsd:string"^^xsd:string .

<https://edi3.org/mmt/vocab#TransportPersonRoleText>
  a rdf:Property ;
  rdfs:comment "A role, expressed as text, of this transport person."^^xsd:string ;
  rdfs:domain "mmt:TransportPerson"^^xsd:string ;
  rdfs:label "roleText"^^xsd:string ;
  rdfs:range "xsd:string"^^xsd:string .

<https://edi3.org/mmt/vocab#TransportRoute>
  a rdfs:Class ;
  rdfs:comment "A way or course taken from one location to another for the purpose of transporting cargo and or passengers."^^xsd:string ;
  rdfs:label "TransportRoute"^^xsd:string .

<https://edi3.org/mmt/vocab#TransportRouteDeparturePointText>
  a rdf:Property ;
  rdfs:comment "A departure point, expressed as text, for this transport route."^^xsd:string ;
  rdfs:domain "mmt:TransportRoute"^^xsd:string ;
  rdfs:label "departurePointText"^^xsd:string ;
  rdfs:range "xsd:string"^^xsd:string .

<https://edi3.org/mmt/vocab#TransportRouteDescription>
  a rdf:Property ;
  rdfs:comment "The textual description of this transport route."^^xsd:string ;
  rdfs:domain "mmt:TransportRoute"^^xsd:string ;
  rdfs:label "description"^^xsd:string ;
  rdfs:range "xsd:string"^^xsd:string .

<https://edi3.org/mmt/vocab#TransportRouteFrequencyTypeCode>
  a rdf:Property ;
  rdfs:comment "The code specifying the type of frequency for this transport route, such as weekly, bi-monthly or daily."^^xsd:string ;
  rdfs:domain "mmt:TransportRoute"^^xsd:string ;
  rdfs:label "frequencyTypeCode"^^xsd:string ;
  rdfs:range "xsd:token"^^xsd:string .

<https://edi3.org/mmt/vocab#TransportRouteID>
  a rdf:Property ;
  rdfs:comment "The unique identifier of this transport route."^^xsd:string ;
  rdfs:domain "mmt:TransportRoute"^^xsd:string ;
  rdfs:label "iD"^^xsd:string ;
  rdfs:range "xsd:ID"^^xsd:string .

<https://edi3.org/mmt/vocab#TransportRouteMapBinaryObject>
  a rdf:Property ;
  rdfs:comment "Binary object data that is the map of this transport route."^^xsd:string ;
  rdfs:domain "mmt:TransportRoute"^^xsd:string ;
  rdfs:label "mapBinaryObject"^^xsd:string ;
  rdfs:range "xsd:base64Binary"^^xsd:string .

<https://edi3.org/mmt/vocab#TransportRouteStatusCode>
  a rdf:Property ;
  rdfs:comment "The code specifying a status for a transport route, such as planned or actual."^^xsd:string ;
  rdfs:domain "mmt:TransportRoute"^^xsd:string ;
  rdfs:label "statusCode"^^xsd:string ;
  rdfs:range "StatusType_Сode"^^xsd:string .

<https://edi3.org/mmt/vocab#TransportRouteTransportMeansText>
  a rdf:Property ;
  rdfs:comment "A means of transport, expressed as text, for this transport route."^^xsd:string ;
  rdfs:domain "mmt:TransportRoute"^^xsd:string ;
  rdfs:label "transportMeansText"^^xsd:string ;
  rdfs:range "xsd:string"^^xsd:string .

<https://edi3.org/mmt/vocab#TransportService>
  a rdfs:Class ;
  rdfs:comment "A service associated with a transport movement."^^xsd:string ;
  rdfs:label "TransportService"^^xsd:string .

<https://edi3.org/mmt/vocab#TransportServiceCategoryTypeCode>
  a rdf:Property ;
  rdfs:comment "A code specifying a type of category for this transport service."^^xsd:string ;
  rdfs:domain "mmt:TransportService"^^xsd:string ;
  rdfs:label "categoryTypeCode"^^xsd:string ;
  rdfs:range "xsd:token"^^xsd:string .

<https://edi3.org/mmt/vocab#TransportServiceChargeAmount>
  a rdf:Property ;
  rdfs:comment "The monetary value of the charge for this transport service."^^xsd:string ;
  rdfs:domain "mmt:TransportService"^^xsd:string ;
  rdfs:label "chargeAmount"^^xsd:string ;
  rdfs:range "http://schema.org/amount"^^xsd:string .

<https://edi3.org/mmt/vocab#TransportServiceConditionTypeCode>
  a rdf:Property ;
  rdfs:comment "A code specifying a type of condition for this transport service, such as a contract or carriage condition."^^xsd:string ;
  rdfs:domain "mmt:TransportService"^^xsd:string ;
  rdfs:label "conditionTypeCode"^^xsd:string ;
  rdfs:range "TransportServiceConditionType_Сode"^^xsd:string .

<https://edi3.org/mmt/vocab#TransportServiceDescription>
  a rdf:Property ;
  rdfs:comment "The textual description of this transport service."^^xsd:string ;
  rdfs:domain "mmt:TransportService"^^xsd:string ;
  rdfs:label "description"^^xsd:string ;
  rdfs:range "xsd:string"^^xsd:string .

<https://edi3.org/mmt/vocab#TransportServiceID>
  a rdf:Property ;
  rdfs:comment "The unique identifier of this transport service."^^xsd:string ;
  rdfs:domain "mmt:TransportService"^^xsd:string ;
  rdfs:label "iD"^^xsd:string ;
  rdfs:range "xsd:ID"^^xsd:string .

<https://edi3.org/mmt/vocab#TransportServiceInformationText>
  a rdf:Property ;
  rdfs:comment "Information, expressed as text, for this transport service."^^xsd:string ;
  rdfs:domain "mmt:TransportService"^^xsd:string ;
  rdfs:label "informationText"^^xsd:string ;
  rdfs:range "xsd:string"^^xsd:string .

<https://edi3.org/mmt/vocab#TransportServiceName>
  a rdf:Property ;
  rdfs:comment "The name, expressed as text, of this transport service."^^xsd:string ;
  rdfs:domain "mmt:TransportService"^^xsd:string ;
  rdfs:label "name"^^xsd:string ;
  rdfs:range "xsd:string"^^xsd:string .

<https://edi3.org/mmt/vocab#TransportServicePaymentArrangementCode>
  a rdf:Property ;
  rdfs:comment "The code specifying the payment arrangement for this transport service."^^xsd:string ;
  rdfs:domain "mmt:TransportService"^^xsd:string ;
  rdfs:label "paymentArrangementCode"^^xsd:string ;
  rdfs:range "TransportPaymentArrangementType_Сode"^^xsd:string .

<https://edi3.org/mmt/vocab#TransportServicePriorityCode>
  a rdf:Property ;
  rdfs:comment "The code specifying the priority of this transport service."^^xsd:string ;
  rdfs:domain "mmt:TransportService"^^xsd:string ;
  rdfs:label "priorityCode"^^xsd:string ;
  rdfs:range "TransportServicePriorityType_Сode"^^xsd:string .

<https://edi3.org/mmt/vocab#TransportServiceServiceRequirementCode>
  a rdf:Property ;
  rdfs:comment "A code specifying a service requirement for this transport service."^^xsd:string ;
  rdfs:domain "mmt:TransportService"^^xsd:string ;
  rdfs:label "serviceRequirementCode"^^xsd:string ;
  rdfs:range "TransportServiceRequirementType_Сode"^^xsd:string .

<https://edi3.org/mmt/vocab#UniversalCommunication>
  a rdfs:Class ;
  rdfs:comment "The exchange of thoughts, messages, or information, as universally exchanged by speech, signals, writing, or behaviour between persons and/or organizations."^^xsd:string ;
  rdfs:label "UniversalCommunication"^^xsd:string .

<https://edi3.org/mmt/vocab#UniversalCommunicationChannelCode>
  a rdf:Property ;
  rdfs:comment "The code specifying the channel or manner in which a universal communication can be made, such as telephone or email."^^xsd:string ;
  rdfs:domain "mmt:UniversalCommunication"^^xsd:string ;
  rdfs:label "channelCode"^^xsd:string ;
  rdfs:range "CommunicationMeansType_Сode"^^xsd:string .

<https://edi3.org/mmt/vocab#UniversalCommunicationCompleteNumber>
  a rdf:Property ;
  rdfs:comment "The text string of characters that make up the complete number for this universal communication."^^xsd:string ;
  rdfs:domain "mmt:UniversalCommunication"^^xsd:string ;
  rdfs:label "completeNumber"^^xsd:string ;
  rdfs:range "xsd:string"^^xsd:string .

<https://edi3.org/mmt/vocab#UniversalCommunicationURI>
  a rdf:Property ;
  rdfs:comment "The Uniform Resource Identifier (URI), such as a web or an email address, for this universal communication."^^xsd:string ;
  rdfs:domain "mmt:UniversalCommunication"^^xsd:string ;
  rdfs:label "uRI"^^xsd:string ;
  rdfs:range "xsd:ID"^^xsd:string .

